# baseURI: http://ies.data.gov.uk/ontology/ies4
@prefix owl: <http://www.w3.org/2002/07/owl#> .
@prefix rdf: <http://www.w3.org/1999/02/22-rdf-syntax-ns#> .
@prefix rdfs: <http://www.w3.org/2000/01/rdf-schema#> .
@prefix xsd: <http://www.w3.org/2001/XMLSchema#> .
@prefix dc: <http://purl.org/dc/elements/1.1/> .
@prefix sh: <http://www.w3.org/ns/shacl#> .
@prefix sparx: <http://data.sparxsystems.com#> .
@prefix ies: <http://ies.data.gov.uk/ontology/ies4#> .
<http://ies.data.gov.uk/ontology/ies4> rdf:type owl:Ontology . 
ies:Accent rdf:type rdfs:Class . 
ies:Accent sparx:guid "{63409D9A-1779-444a-BF04-23C03B3B2F72}" . 
ies:Accent rdfs:comment "An Characteristic whose members are people who all share the same national or regional accent" . 
ies:Accent rdfs:subClassOf ies:Characteristic . 
ies:Account rdf:type rdfs:Class . 
ies:Account sparx:guid "{31BFE794-924E-44e3-942E-ADC9ED19FBA1}" . 
ies:Account rdfs:comment "An Entity that is the collection of all transactions between a provider and a customer" . 
ies:Account rdfs:subClassOf ies:Entity . 
ies:Account rdfs:subClassOf ies:AccountState . 
ies:AccountAdminEvent rdf:type rdfs:Class . 
ies:AccountAdminEvent sparx:guid "{19E90CA4-F0EB-4245-826E-EDC278642B41}" . 
ies:AccountAdminEvent rdfs:comment "A BusinessEvent that an Account participates in" . 
ies:AccountAdminEvent rdfs:subClassOf ies:BusinessEvent . 
ies:accountForCard rdf:type owl:ObjectProperty . 
ies:accountForCard sparx:guid "{7891E893-56DB-4d47-80B4-C78A667767F6}" . 
ies:accountForCard rdfs:comment "Relates a BankCard to the FinancialAccount which the card is issued against." . 
ies:accountForCard rdfs:subPropertyOf ies:relationship . 
ies:accountForCard rdfs:domain ies:BankCard . 
ies:accountForCard rdfs:range ies:FinancialAccount . 
ies:AccountHolder rdf:type rdfs:Class . 
ies:AccountHolder sparx:guid "{C93379F2-6B01-4100-ABFA-BD26098AC1CB}" . 
ies:AccountHolder rdfs:comment "A PersonState when they hold an Account" . 
ies:AccountHolder rdfs:subClassOf ies:ResponsibleActorState . 
ies:AccountInCommunication rdf:type rdfs:Class . 
ies:AccountInCommunication sparx:guid "{942FBF46-A7EF-432b-99DD-1E0E3E874C21}" . 
ies:AccountInCommunication rdfs:comment "An AccountState (and an EventParticipant) when an Account is involved in communicating. " . 
ies:AccountInCommunication rdfs:subClassOf ies:EventParticipant . 
ies:AccountInCommunication rdfs:subClassOf ies:CommunicationsAccountState . 
ies:AccountNumber rdf:type rdfs:Class . 
ies:AccountNumber sparx:guid "{A72F0FF1-88F2-4b36-A2C4-26B4B0698A2C}" . 
ies:AccountNumber rdfs:comment "The account number for the respective FinancialAccount." . 
ies:AccountNumber rdfs:subClassOf ies:Identifier . 
ies:accountProvider rdf:type owl:ObjectProperty . 
ies:accountProvider sparx:guid "{0F9244C3-B2F5-4b8a-AED2-54B7FDAB9578}" . 
ies:accountProvider rdfs:comment "The Organisation that provides the FinancialAccount" . 
ies:accountProvider rdfs:subPropertyOf ies:relationship . 
ies:accountProvider rdfs:range ies:Organisation . 
ies:accountProvider rdfs:domain ies:Account . 
ies:AccountState rdf:type rdfs:Class . 
ies:AccountState sparx:guid "{0BCDB801-1F3B-4496-B04B-95EF545E9445}" . 
ies:AccountState rdfs:comment "A temporal state of an Account" . 
ies:AccountState rdfs:subClassOf ies:State . 
ies:Accused rdf:type rdfs:Class . 
ies:Accused sparx:guid "{A4D8A62A-DC98-410c-80D2-57C98C1E95C0}" . 
ies:Accused rdfs:comment "A ResponsibleActors role as the accused in a Prosecution" . 
ies:Accused rdfs:subClassOf ies:ActiveEventParticipant . 
ies:Accused rdfs:subClassOf ies:ResponsibleActorState . 
ies:aCopyOf rdf:type owl:ObjectProperty . 
ies:aCopyOf sparx:guid "{22D9054C-AE5C-4afe-99D9-3C9D65C86CB9}" . 
ies:aCopyOf rdfs:comment "An rdf:type relationship that asserts a Document is a copy of WorkOfDocumentationNote: Document instances are individual physical documents whereas WorkOfDocumentation is the general case of a document - e.g. War and Peace vs my copy of War and Peace" . 
ies:aCopyOf rdfs:subPropertyOf rdf:type . 
ies:aCopyOf rdfs:domain ies:IndividualDocument . 
ies:aCopyOf rdfs:range ies:WorkOfDocumentation . 
ies:ActiveEventParticipant rdf:type rdfs:Class . 
ies:ActiveEventParticipant sparx:guid "{3360DCC9-D39B-4280-8872-2FE122240407}" . 
ies:ActiveEventParticipant rdfs:comment "An EventParticipant where the participant is actively engaged in the Event.Note: In BORO, EventParticipant would be Involvement and ActiveEventParticipant would be Participation." . 
ies:ActiveEventParticipant rdfs:subClassOf ies:EventParticipant . 
ies:Actor rdf:type rdfs:Class . 
ies:Actor sparx:guid "{B2B15802-9CE9-4a9d-9DE0-8289D8474E9B}" . 
ies:Actor rdfs:comment "An Entity that is capable of performing functions - i.e. actively participating in an Event." . 
ies:Actor rdfs:subClassOf ies:Entity . 
ies:Actor rdfs:subClassOf ies:ActorState . 
ies:ActorState rdf:type rdfs:Class . 
ies:ActorState sparx:guid "{7ED8BC7C-A85F-4ed5-AC6F-D640F2DF4B7B}" . 
ies:ActorState rdfs:comment "A temporal state of an Actor" . 
ies:ActorState rdfs:subClassOf ies:State . 
ies:Address rdf:type rdfs:Class . 
ies:Address sparx:guid "{C90267B5-77A3-4b79-BD0D-7C50C3F4C333}" . 
ies:Address rdfs:comment "A Location that can be specified by a postal address" . 
ies:Address rdfs:subClassOf ies:RealEstate . 
ies:addressRegion rdf:type owl:ObjectProperty . 
ies:addressRegion sparx:guid "{3E452516-2523-4a86-974D-1D2251057E6E}" . 
ies:addressRegion rdfs:comment "An inLocation relationship to indicate an Address is in a RegionOfCountry" . 
ies:addressRegion rdfs:subPropertyOf ies:inLocation . 
ies:addressRegion rdfs:domain ies:Address . 
ies:addressRegion rdfs:range ies:RegionOfCountry . 
ies:AdministeredAccount rdf:type rdfs:Class . 
ies:AdministeredAccount sparx:guid "{D779F547-C1FB-4d48-9BB8-CB37B9D2F82C}" . 
ies:AdministeredAccount rdfs:comment "An EventParticipant where a FinancialAccount is administered" . 
ies:AdministeredAccount rdfs:subClassOf ies:EventParticipant . 
ies:after rdf:type owl:ObjectProperty . 
ies:after sparx:guid "{FA4DDF04-16DA-4b5c-AE9A-6AB8CD07DCDB}" . 
ies:after rdfs:comment "A relationship linking two Elements where one ends before the other starts" . 
ies:after rdfs:subPropertyOf ies:relationship . 
ies:after rdfs:domain ies:Element . 
ies:after rdfs:range ies:Element . 
ies:AgreementExecution rdf:type rdfs:Class . 
ies:AgreementExecution sparx:guid "{93F71FAF-AEF4-4e41-8CEB-FC6447B20428}" . 
ies:AgreementExecution rdfs:comment "An AgreementStage which includes all the ongoing activities that conform to the agreement reached" . 
ies:AgreementExecution rdfs:subClassOf ies:AgreementStage . 
ies:AgreementName rdf:type rdfs:Class . 
ies:AgreementName sparx:guid "{7A750064-E711-4871-AFC3-39057342FB9E}" . 
ies:AgreementName rdfs:comment "A Name that is used to refer to an EndToEndAgreement." . 
ies:AgreementName rdfs:subClassOf ies:Name . 
ies:AgreementStage rdf:type rdfs:Class . 
ies:AgreementStage sparx:guid "{422B4F1C-DA90-400b-8FFD-43C90B4F10F4}" . 
ies:AgreementStage rdfs:comment "An Event which is part of an EndToEndAgreement" . 
ies:AgreementStage rdfs:subClassOf ies:Event . 
ies:Aircraft rdf:type rdfs:Class . 
ies:Aircraft sparx:guid "{01A64A84-7A14-45a5-AAF2-F1AA614D5F30}" . 
ies:Aircraft rdfs:comment "A Vehicle that travels by air" . 
ies:Aircraft rdfs:subClassOf ies:Vehicle . 
ies:Airport rdf:type rdfs:Class . 
ies:Airport sparx:guid "{82E3793F-D0D1-40ca-927C-7A6FEF913503}" . 
ies:Airport rdfs:comment "A Port used for air travel" . 
ies:Airport rdfs:subClassOf ies:Port . 
ies:allAuthorisedAgainst rdf:type owl:ObjectProperty . 
ies:allAuthorisedAgainst sparx:guid "{97E2E16A-5D4C-41bd-AF32-8DF2057A35BA}" . 
ies:allAuthorisedAgainst rdfs:comment "A relationship linking an AuthorisedEventClass to a Entity to assert that all instances of the AuthorisedEventClass were Events acting upon the Entity.Note: this is generally a law-enforcement concern where a warrant (EndToEndAuthorisation) is granted against people, devices, etc. (GrantOfAuthority)." . 
ies:allAuthorisedAgainst rdfs:subPropertyOf ies:relationship . 
ies:allAuthorisedAgainst rdfs:domain ies:AuthorisedEventClass . 
ies:allAuthorisedAgainst rdfs:range ies:Entity . 
ies:allHaveCharacteristic rdf:type owl:ObjectProperty . 
ies:allHaveCharacteristic sparx:guid "{81A1E70D-6ADB-4843-BCA6-C0A710E7716B}" . 
ies:allHaveCharacteristic rdfs:comment "An rdfs:subClassOf relationship that asserts that all instances of a ClassOfElement share a particular Characteristic or Measuree.g. all London buses being red, all heavyweight boxers weighing more than 200lbs" . 
ies:allHaveCharacteristic rdfs:subPropertyOf ies:relationship . 
ies:allHaveCharacteristic rdfs:subPropertyOf rdfs:subClassOf . 
ies:allHaveCharacteristic rdfs:domain ies:ClassOfElement . 
ies:allHaveCharacteristic rdfs:range ies:Characteristic . 
ies:allHaveDisposition rdf:type owl:ObjectProperty . 
ies:allHaveDisposition sparx:guid "{6F8504E0-E03C-43fa-AA81-C3341CA551E3}" . 
ies:allHaveDisposition rdfs:comment "An rdfs:subClassOf relationship that asserts that all instances of a ClassOfElement share a dispositione.g. all Eurofighters being cable of Mach 2" . 
ies:allHaveDisposition rdfs:subPropertyOf ies:relationship . 
ies:allHaveDisposition rdfs:subPropertyOf rdfs:subClassOf . 
ies:allHaveDisposition rdfs:range ies:DispositionalClass . 
ies:allHaveDisposition rdfs:domain ies:Element . 
ies:Alliance rdf:type rdfs:Class . 
ies:Alliance sparx:guid "{3D83E15F-ACA8-48e4-8C7B-84580807E06F}" . 
ies:Alliance rdfs:comment "An Organisation made up of allies - these could be people or organisations, and the alliance may be quite loose." . 
ies:Alliance rdfs:subClassOf ies:Organisation . 
ies:alliedTo rdf:type owl:ObjectProperty . 
ies:alliedTo sparx:guid "{7F818F57-2C3B-4629-8EEC-F5F8310AE655}" . 
ies:alliedTo rdfs:comment "A Relationship between two ResponsibleActor Entities where one is allied to the other." . 
ies:alliedTo rdfs:subPropertyOf ies:relationship . 
ies:alliedTo rdfs:range ies:Alliance . 
ies:alliedTo rdfs:domain ies:ResponsibleActorState . 
ies:allocatedSeatNumber rdf:type owl:DatatypeProperty . 
ies:allocatedSeatNumber sparx:guid "{518E9B39-58C0-4e89-831D-B6099C3B9892}" . 
ies:allocatedSeatNumber rdfs:comment "The seat number associated with the ticket" . 
ies:allocatedSeatNumber rdfs:subPropertyOf ies:attribute . 
ies:allocatedSeatNumber rdfs:domain ies:Ticket . 
ies:Altitude rdf:type rdfs:Class . 
ies:Altitude sparx:guid "{51B6F4C5-0DA3-437d-9507-38514BC2ABCD}" . 
ies:Altitude rdfs:comment "The Length that is the distance above (or below in the case of negative numbers) the surface of the WGS84 spheroid of the respective Location " . 
ies:Altitude rdfs:subClassOf ies:Length . 
ies:AmountOfMoney rdf:type rdfs:Class . 
ies:AmountOfMoney sparx:guid "{0DF94DE5-68B7-45b4-A106-A11CE06C31B8}" . 
ies:AmountOfMoney rdfs:comment "A specific amount of a given currency" . 
ies:AmountOfMoney rdfs:subClassOf ies:Asset . 
ies:AmountOfSubstance rdf:type rdfs:Class . 
ies:AmountOfSubstance sparx:guid "{324D0329-1299-45cc-92A5-270134E66512}" . 
ies:AmountOfSubstance rdfs:comment "The Measure of the stoichiometric quantity of substance (usually measured in moles)" . 
ies:AmountOfSubstance rdfs:subClassOf ies:StandardMeasure . 
ies:ancestorOf rdf:type owl:ObjectProperty . 
ies:ancestorOf sparx:guid "{15388C46-262D-4f70-8F65-83758A5AEAF5}" . 
ies:ancestorOf rdfs:comment "A Relationship between two Person Entities that indicates one is and ancestor of the otherNote: was called relative of in IES 3.x, but was really only about ancestry, so is changed here. " . 
ies:ancestorOf rdfs:domain ies:Person . 
ies:ancestorOf rdfs:range ies:Person . 
ies:ancestorOf rdfs:subPropertyOf ies:familiallyRelatedTo . 
ies:andGroup rdf:type owl:DatatypeProperty . 
ies:andGroup sparx:guid "{1326576A-6240-47b0-AED7-5F3FC4E3884D}" . 
ies:andGroup rdfs:comment "The groups (if any) which the requesting user must be a member of in order to access the item. See the EDH specification for further details.Allowable Values:See EDH Standard" . 
ies:andGroup rdfs:domain ies:SecurityLabel . 
ies:ArbitraryOverlap rdf:type rdfs:Class . 
ies:ArbitraryOverlap sparx:guid "{F8FABF60-63D3-42ae-BA6A-54CFD0C036BF}" . 
ies:ArbitraryOverlap rdfs:comment "An Element whose extent is defined by being the shared overlap of two or more Elements" . 
ies:ArbitraryOverlap rdfs:subClassOf ies:Element . 
ies:ArbitraryPeriod rdf:type rdfs:Class . 
ies:ArbitraryPeriod sparx:guid "{68BA678C-DCA8-453e-BFCC-D9FB48339D99}" . 
ies:ArbitraryPeriod rdfs:comment "A PeriodOfTime for which is not delineated by a particular clock period - e.g. not a year, not a month, not a day, not an hour, etc. Instead it is one which is most clearly specified in terms of start and end that are ParticularPeriods." . 
ies:ArbitraryPeriod rdfs:subClassOf ies:PeriodOfTime . 
ies:areaOfCoverage rdf:type owl:ObjectProperty . 
ies:areaOfCoverage sparx:guid "{C6BA7464-C00E-4ff6-AE7B-9CE9D4E08FDF}" . 
ies:areaOfCoverage rdfs:comment "The area over which the TravelCard is valid Examples:London  Zone 1London  All Zones" . 
ies:areaOfCoverage rdfs:subPropertyOf ies:relationship . 
ies:areaOfCoverage rdfs:domain ies:TravelCard . 
ies:areaOfCoverage rdfs:range ies:Location . 
ies:Arrest rdf:type rdfs:Class . 
ies:Arrest sparx:guid "{D8D7184C-2F7B-4a5d-AA8F-7EE7B5A04F94}" . 
ies:Arrest rdfs:comment "A LawEnforcement Event where a Person is arrested" . 
ies:Arrest rdfs:subClassOf ies:LawEnforcement . 
ies:Arrest rdfs:subClassOf ies:OperationalEvent . 
ies:Arrested rdf:type rdfs:Class . 
ies:Arrested sparx:guid "{B870A3B5-32FA-4aaf-86F1-7DB674585F3A}" . 
ies:Arrested rdfs:comment "A Persons role when arrested" . 
ies:Arrested rdfs:subClassOf ies:ActiveEventParticipant . 
ies:Arrested rdfs:subClassOf ies:PersonState . 
ies:ArrestingOfficer rdf:type rdfs:Class . 
ies:ArrestingOfficer sparx:guid "{5B3F41C3-91CC-442f-A4F8-615E77751734}" . 
ies:ArrestingOfficer rdfs:comment "A Persons role as arresting officer" . 
ies:ArrestingOfficer rdfs:subClassOf ies:ActiveEventParticipant . 
ies:ArrestingOfficer rdfs:subClassOf ies:PersonState . 
ies:Arrival rdf:type rdfs:Class . 
ies:Arrival sparx:guid "{F2C03DA3-B554-4bde-A0DE-EFB5BEE19C56}" . 
ies:Arrival rdfs:comment "A BoundingState that marks the end of a Movement eventThe date/time of the arrival can be specified using the inPeriod relationship. " . 
ies:Arrival rdfs:subClassOf ies:BoundingState . 
ies:assessed rdf:type owl:ObjectProperty . 
ies:assessed sparx:guid "{669E3CD0-CD9D-496c-A711-ECDE3F589012}" . 
ies:assessed rdfs:comment "An owl:objectProperty that links an AssesToBeTrue to the rdfs:Resource that is assessed to be true." . 
ies:assessed rdfs:domain ies:AssessToBeTrue . 
ies:assessed rdfs:range rdfs:Resource . 
ies:assessedToBeTheSameAs rdf:type owl:ObjectProperty . 
ies:assessedToBeTheSameAs sparx:guid "{6A1C6C65-D671-4ea3-9184-044AE2A802CF}" . 
ies:assessedToBeTheSameAs rdfs:comment "A relationship that asserts two ExchangedItems that may have been previously judged to be different are in fact the same thing. WARNING:  by the same we mean they occupy the same space for the same period of time - i.e. not two different things in the same place at different times, and not the same physical item at two different periods of time. The Identifier and State patterns should do most of what is needed here, and it is extremely rare that this would ever be needed. Do not use unless absolutely necessary. " . 
ies:assessedToBeTheSameAs rdfs:subPropertyOf ies:relationship . 
ies:Assessor rdf:type rdfs:Class . 
ies:Assessor sparx:guid "{80F9B97D-2C7F-4978-83A3-BE934DD4E1FF}" . 
ies:Assessor rdfs:comment "An EventParticipant where an Actor assesses something to be true." . 
ies:Assessor rdfs:subClassOf ies:ActiveEventParticipant . 
ies:AssessToBeTrue rdf:type rdfs:Class . 
ies:AssessToBeTrue sparx:guid "{7150208D-A02E-45ed-8279-44843F4DA897}" . 
ies:AssessToBeTrue rdfs:comment "An Event where a fact is assessed to be true by a Actor (i.e. a Person or Device)An AssessToBeTrue shall have one and only one hmlConfidence attribute (i.e. this is mandatory)" . 
ies:AssessToBeTrue rdfs:subClassOf ies:Event . 
ies:Asset rdf:type rdfs:Class . 
ies:Asset sparx:guid "{40231334-5ACC-4dd4-A8C1-05012E2170E0}" . 
ies:Asset rdfs:comment "An Entity that is either man-made (or defined - see Rights) or whose extent is defined in such a way as to specify ownership - e.g. a parcel of real estate" . 
ies:Asset rdfs:subClassOf ies:Entity . 
ies:Asset rdfs:subClassOf ies:AssetState . 
ies:AssetState rdf:type rdfs:Class . 
ies:AssetState sparx:guid "{CA196722-9531-4eb4-A8CF-B9A5145CDCFD}" . 
ies:AssetState rdfs:comment "A temporal state of an Asset" . 
ies:AssetState rdfs:subClassOf ies:State . 
ies:associatedCarrier rdf:type owl:ObjectProperty . 
ies:associatedCarrier sparx:guid "{2E464C7F-FC0B-4dcc-9B1C-5DCA87B4CE3A}" . 
ies:associatedCarrier rdfs:comment "The Organisation that provides the transport specified on the Ticket" . 
ies:associatedCarrier rdfs:subPropertyOf ies:relationship . 
ies:associatedCarrier rdfs:domain ies:TravelTicket . 
ies:associatedCarrier rdfs:range ies:Organisation . 
ies:associatedPersonName rdf:type owl:DatatypeProperty . 
ies:associatedPersonName sparx:guid "{022535DE-2100-420b-B4BC-10465DEEEC3C}" . 
ies:associatedPersonName rdfs:comment "The name of the Person which is associated with the EntityThis may be the name of an account holder, the name printed on ID, tickets, etc.Note in 3.x, this was several different attributes:accountHolderName on FinancialAccountnameOnLicense, etc. on IdentityDocumentticketHolderName on Ticket" . 
ies:associatedPersonName rdfs:domain ies:Ticket . 
ies:associatedPersonName rdfs:domain ies:AccountState . 
ies:associatedPersonName rdfs:domain ies:IdentityDocument . 
ies:associatedPersonName rdfs:domain ies:PaymentArtefact . 
ies:associatedPersonName rdfs:subPropertyOf ies:attribute . 
ies:Attacker rdf:type rdfs:Class . 
ies:Attacker sparx:guid "{73D38C0E-3291-4de9-8920-F37980CB3A9E}" . 
ies:Attacker rdfs:comment "Relates a MilitaryAttack to the Organisation conducting the attack" . 
ies:Attacker rdfs:subClassOf ies:EventParticipant . 
ies:Attendance rdf:type rdfs:Class . 
ies:Attendance sparx:guid "{626D5F2C-9153-40f4-9F2A-393B6DB072D3}" . 
ies:Attendance rdfs:comment "A Presence where the Person is presentNote - we may not know the identity of the person, so would just create only the Attendance (EventParticipant). This allows the model to grow as more information is discovered without recourse to using sameAs relationships." . 
ies:Attendance rdfs:subClassOf ies:Presence . 
ies:Attendance rdfs:subClassOf ies:PersonState . 
ies:Attendance rdfs:subClassOf ies:ActiveEventParticipant . 
ies:attribute rdf:type owl:DatatypeProperty . 
ies:attribute sparx:guid "{4A8E5877-32DF-428f-9A60-6AC3D083FFCA}" . 
ies:attribute rdfs:comment "A feature or property of an ExchangedItemNote: In IES4 it is important to distinguish between names and attributes - attribute should never be used to identify or name something - for that, use Name or Identifier." . 
ies:attribute rdfs:domain ies:ExchangedItem . 
ies:AtWar rdf:type rdfs:Class . 
ies:AtWar sparx:guid "{89953404-8A71-46ef-8F7B-90C12EE286FD}" . 
ies:AtWar rdfs:comment "An InDisagreement where the parties have declared war" . 
ies:AtWar rdfs:subClassOf ies:InDisagreement . 
ies:AuthorisationDocument rdf:type rdfs:Class . 
ies:AuthorisationDocument sparx:guid "{8177A2FB-CA54-4dc5-9884-33FBA660B174}" . 
ies:AuthorisationDocument rdfs:comment "A WorkOfDocumentation that provides permission" . 
ies:AuthorisationDocument rdfs:subClassOf ies:WorkOfDocumentation . 
ies:AuthorisationRequest rdf:type rdfs:Class . 
ies:AuthorisationRequest sparx:guid "{1D6BAE08-B8F1-4eee-928E-991B3B46EADF}" . 
ies:AuthorisationRequest rdfs:comment "An AuthorisationStage where a ResponsibleActor requests authorisation to act from another ResponsibleActor" . 
ies:AuthorisationRequest rdfs:subClassOf ies:AuthorisationStage . 
ies:AuthorisationRequester rdf:type rdfs:Class . 
ies:AuthorisationRequester sparx:guid "{81BF6EA6-996D-4148-8F5D-8B41156637F6}" . 
ies:AuthorisationRequester rdfs:comment "An ActiveEventParticipant where a ResponsibleActor requests authority to act " . 
ies:AuthorisationRequester rdfs:subClassOf ies:ActiveEventParticipant . 
ies:AuthorisationReviewer rdf:type rdfs:Class . 
ies:AuthorisationReviewer sparx:guid "{8E4CC036-C4C5-4222-8532-9B6C53EEC56E}" . 
ies:AuthorisationReviewer rdfs:comment "An ActiveEventParticipant where a ResponsibleActor reviews an AuthorisationRequest" . 
ies:AuthorisationReviewer rdfs:subClassOf ies:ActiveEventParticipant . 
ies:AuthorisationStage rdf:type rdfs:Class . 
ies:AuthorisationStage sparx:guid "{2D5069F2-FE77-477f-A607-FA6458E64173}" . 
ies:AuthorisationStage rdfs:comment "An Event which is part of an EndToEndAuthorisation" . 
ies:AuthorisationStage rdfs:subClassOf ies:Event . 
ies:AuthorisedActor rdf:type rdfs:Class . 
ies:AuthorisedActor sparx:guid "{F69279D2-BA11-4a31-8739-0D91EF5B9BEF}" . 
ies:AuthorisedActor rdfs:comment "An ActiveEventParticipant where a ResponsibleActor is granted authority to act in a GrantOfAuthority " . 
ies:AuthorisedActor rdfs:subClassOf ies:ActiveEventParticipant . 
ies:AuthorisedEventClass rdf:type rdfs:Class . 
ies:AuthorisedEventClass sparx:guid "{057C04F9-EB8A-4e21-9CF8-2D98038570FB}" . 
ies:AuthorisedEventClass rdfs:comment "A ClassOfEvent where the type activity described is either authorised or required to be authorised.An instance of an AuthorisedEventClass will most often also be a TimeBoundedClass as it is rare to see requests or grants of authority with no time limit. An AuthorisedEventClass will usually be of the form of Event type A against Entity X = e.g. Arrest of John Smith, Surveillance of 23 Acacia Gardens. The link from this class to the entity involved is via the allAuthorisedAgainst relationship." . 
ies:AuthorisedEventClass rdfs:subClassOf ies:ClassOfEvent . 
ies:Authoriser rdf:type rdfs:Class . 
ies:Authoriser sparx:guid "{466DCDFB-B642-468b-A47A-E83291A86C6B}" . 
ies:Authoriser rdfs:comment "An ActiveEventParticipant where a ResponsibleActor acts as the authoriser (sign off) in a GrantOfAuthority " . 
ies:Authoriser rdfs:subClassOf ies:ActiveEventParticipant . 
ies:authorisesAccessTo rdf:type owl:ObjectProperty . 
ies:authorisesAccessTo sparx:guid "{A2DA918D-843C-43c9-A974-4795601E9D65}" . 
ies:authorisesAccessTo rdfs:comment "The Event for which the respective Ticket applies." . 
ies:authorisesAccessTo rdfs:subPropertyOf ies:relationship . 
ies:authorisesAccessTo rdfs:domain ies:Ticket . 
ies:authorisesAccessTo rdfs:range ies:Event . 
ies:Bank rdf:type rdfs:Class . 
ies:Bank sparx:guid "{4E10343E-8350-4354-B3DB-A7F74B4535EF}" . 
ies:Bank rdfs:comment "An Organisation that holds a banking license and can conduct financial transactions on behalf of customers" . 
ies:Bank rdfs:subClassOf ies:Organisation . 
ies:BankBranch rdf:type rdfs:Class . 
ies:BankBranch sparx:guid "{02E3C3B8-8650-4867-8390-823E4B3360E6}" . 
ies:BankBranch rdfs:comment "An operating division of a Bank, usually a high street branch, but might also be the online arm of a Bank" . 
ies:BankBranch rdfs:subClassOf ies:Organisation . 
ies:BankCard rdf:type rdfs:Class . 
ies:BankCard sparx:guid "{848A9E0F-F3B4-47c3-AA7E-2FF6BE92170C}" . 
ies:BankCard rdfs:comment "A PaymentArtefact that is a physical card used for making financial transactions.Note: when used online, the accompanying Fan" . 
ies:BankCard rdfs:subClassOf ies:PaymentArtefact . 
ies:beginBoundOfClass rdf:type owl:ObjectProperty . 
ies:beginBoundOfClass sparx:guid "{2C441F0A-635D-41ef-B8CC-96AA07958F8E}" . 
ies:beginBoundOfClass rdfs:comment "A relationship linking a TimeBoundedClass to the ParticularPeriod that marks the beginning bound date of its instances" . 
ies:beginBoundOfClass rdfs:subPropertyOf ies:relationship . 
ies:beginBoundOfClass rdfs:domain ies:TimeBoundedClass . 
ies:beginBoundOfClass rdfs:range ies:ParticularPeriod . 
ies:BirthCertificate rdf:type rdfs:Class . 
ies:BirthCertificate sparx:guid "{4457E8AF-EDBD-4ef1-B62B-59037829B961}" . 
ies:BirthCertificate rdfs:comment "An IdentityDocument issued to prove the data and place of birth of a Person" . 
ies:BirthCertificate rdfs:subClassOf ies:IdentityDocument . 
ies:BirthState rdf:type rdfs:Class . 
ies:BirthState sparx:guid "{CFE53096-32FC-47c8-98BA-950EE6F988CB}" . 
ies:BirthState rdfs:comment "A BoundingState that marks the beginning of a Persons life.The location of the birth can be specified using inLocationThe date/time of the birth can be specified using the inPeriod relationship. " . 
ies:BirthState rdfs:subClassOf ies:BoundingState . 
ies:BirthState rdfs:subClassOf ies:PersonState . 
ies:BoardingCardNumber rdf:type rdfs:Class . 
ies:BoardingCardNumber sparx:guid "{683E5B90-2514-4342-AE34-894D2DAC2AF0}" . 
ies:BoardingCardNumber rdfs:comment "The number of the boarding card issued to the Passenger. " . 
ies:BoardingCardNumber rdfs:subClassOf ies:Identifier . 
ies:Book rdf:type rdfs:Class . 
ies:Book sparx:guid "{22AB6EA2-B088-4ef6-AE3A-5843FBA5C8AE}" . 
ies:Book rdfs:comment "A WorkOfDocumentation that is a published book" . 
ies:Book rdfs:subClassOf ies:WorkOfDocumentation . 
ies:BookedPassenger rdf:type rdfs:Class . 
ies:BookedPassenger sparx:guid "{53C6BCA9-4D66-4bac-B946-0A8541CF510A}" . 
ies:BookedPassenger rdfs:comment "A Persons involvement as a booked traveller in a TravelBooking" . 
ies:BookedPassenger rdfs:subClassOf ies:EventParticipant . 
ies:BookedPassenger rdfs:subClassOf ies:ResponsibleActorState . 
ies:BookingAgent rdf:type rdfs:Class . 
ies:BookingAgent sparx:guid "{0AF87601-5B3E-4c5e-8149-D0D3C0073C42}" . 
ies:BookingAgent rdfs:comment "A ResponsibleActors involvement as the facilitator of a TravelBooking" . 
ies:BookingAgent rdfs:subClassOf ies:EventParticipant . 
ies:BookingAgent rdfs:subClassOf ies:ResponsibleActorState . 
ies:BookingPayment rdf:type rdfs:Class . 
ies:BookingPayment sparx:guid "{61BDEBA6-BE87-44e3-A1C7-246D0CE60ADC}" . 
ies:BookingPayment rdfs:comment "An EventParticipant where an AmountOfMoney in cash is used as payment in a TravelBooking.When neither card nor cash is used, there will be an accompanying MoneyTransfer" . 
ies:BookingPayment rdfs:subClassOf ies:EventParticipant . 
ies:BookingReference rdf:type rdfs:Class . 
ies:BookingReference sparx:guid "{D31E959A-6354-40e7-8370-1FE5246624AD}" . 
ies:BookingReference rdfs:comment "An Identifier that is  notionally unique number that is allocated to a TravelBooking.Note that Booking Reference Numbers are recycled and so are not unique in their own right. When combined with the BookingDate it is potentially possible to identify a specific booking." . 
ies:BookingReference rdfs:subClassOf ies:Identifier . 
ies:bookingType rdf:type owl:ObjectProperty . 
ies:bookingType sparx:guid "{C52879E4-919A-4dee-82EB-3CB11DD69E56}" . 
ies:bookingType rdfs:comment "Relates a TravelBooking to a ClassOfTravelBooking to indicate the method of booking" . 
ies:bookingType rdfs:subPropertyOf ies:relationship . 
ies:bookingType rdfs:subPropertyOf rdf:type . 
ies:bookingType rdfs:domain ies:TravelBooking . 
ies:bookingType rdfs:range ies:ClassOfTravelBooking . 
ies:BoundingState rdf:type rdfs:Class . 
ies:BoundingState sparx:guid "{892345CD-9FA7-4982-978D-B6D3ABAE839C}" . 
ies:BoundingState rdfs:comment "A ContinuousState that occurs at the beginning or end of an Element The date/time of the state can be specified using the inPeriod relationship. " . 
ies:BoundingState rdfs:subClassOf ies:ContinuousState . 
ies:BranchCode rdf:type rdfs:Class . 
ies:BranchCode sparx:guid "{012F7F29-4F8E-4263-8224-126050EE175F}" . 
ies:BranchCode rdfs:comment "In identifier for a BankBranch - In the UK this is often referred to as the Sort Code." . 
ies:BranchCode rdfs:subClassOf ies:Identifier . 
ies:branding rdf:type owl:ObjectProperty . 
ies:branding sparx:guid "{62675B63-9169-4f05-9993-E1B17540A6C1}" . 
ies:branding rdfs:comment "A brand or logo that is represented on an Entitye.g. some bank cards are branded by a car manufacturer, etc. but actually operated by a bank" . 
ies:branding rdfs:subPropertyOf ies:relationship . 
ies:branding rdfs:domain ies:PaymentArtefact . 
ies:branding rdfs:range ies:Organisation . 
ies:BusinessEvent rdf:type rdfs:Class . 
ies:BusinessEvent sparx:guid "{94CEDBD1-8E3D-4cb4-8155-FBD621DA6A0D}" . 
ies:BusinessEvent rdfs:comment "An Event that is commercial or administrative in nature" . 
ies:BusinessEvent rdfs:subClassOf ies:Event . 
ies:Callee rdf:type rdfs:Class . 
ies:Callee sparx:guid "{F50BAD6D-EBE0-4fd8-B54C-3E24A62491A6}" . 
ies:Callee rdfs:comment "An PartyInCommunication where the communicating party is called in an InteractiveCommunication" . 
ies:Callee rdfs:subClassOf ies:PartyInCommunication . 
ies:Caller rdf:type rdfs:Class . 
ies:Caller sparx:guid "{03DDC2F5-F961-47c2-B8F8-B27A752AEC34}" . 
ies:Caller rdfs:comment "An PartyInCommunication where the communicating party is the caller in an InteractiveCommunication" . 
ies:Caller rdfs:subClassOf ies:PartyInCommunication . 
ies:Callsign rdf:type rdfs:Class . 
ies:Callsign sparx:guid "{25F4F685-3931-4cdc-AF43-1A9194BBE15D}" . 
ies:Callsign rdfs:comment "In broadcasting and radio communications, a call sign (also known as a call name or call letters � and historically as a call signal) is a unique designation for a transmitting station." . 
ies:Callsign rdfs:subClassOf ies:CommunicationsIdentifier . 
ies:Capability rdf:type rdfs:Class . 
ies:Capability sparx:guid "{91D62F08-ED05-4558-9321-368712A34A30}" . 
ies:Capability rdfs:comment "A DispositionalClass where all the instances share the same capabilityExample: Vehicles capable of Mach 2" . 
ies:Capability rdfs:subClassOf ies:DispositionalClass . 
ies:CardNumber rdf:type rdfs:Class . 
ies:CardNumber sparx:guid "{087F3453-B1D7-41e6-B79F-31B123ED0D68}" . 
ies:CardNumber rdfs:comment "An Identifier that is the long number on the face of the card (PaymentArtefact)" . 
ies:CardNumber rdfs:subClassOf ies:Identifier . 
ies:cardType rdf:type owl:ObjectProperty . 
ies:cardType sparx:guid "{CF6B72ED-DF58-42e1-A72A-1F047287B80D}" . 
ies:cardType rdfs:comment "The type of a PaymentArtefact" . 
ies:cardType rdfs:subPropertyOf ies:relationship . 
ies:cardType rdfs:domain ies:PaymentArtefact . 
ies:cardType rdfs:range ies:ClassOfPaymentArtefact . 
ies:cardType rdfs:subPropertyOf rdf:type . 
ies:CardUsed rdf:type rdfs:Class . 
ies:CardUsed sparx:guid "{1B9C8EB0-69A7-4fe7-8358-0F6067439C42}" . 
ies:CardUsed rdfs:comment "An EventParticipant where a PaymentArtefact is participant in a TradeEvent" . 
ies:CardUsed rdfs:subClassOf ies:EventParticipant . 
ies:Carrier rdf:type rdfs:Class . 
ies:Carrier sparx:guid "{91DC18F6-3E35-411c-814D-5ACEE83BE316}" . 
ies:Carrier rdfs:comment "An EventParticipant where a ResponsibleActor participates in a Delivery as a carrier" . 
ies:Carrier rdfs:subClassOf ies:EventParticipant . 
ies:carrierService rdf:type owl:ObjectProperty . 
ies:carrierService sparx:guid "{76C31798-780C-41b0-A985-0AE3B1C3A478}" . 
ies:carrierService rdfs:comment "The Organisation that provides the transport specified on the Ticket" . 
ies:carrierService rdfs:subPropertyOf ies:relationship . 
ies:carrierService rdfs:domain ies:TravelService . 
ies:carrierService rdfs:range ies:Organisation . 
ies:CarTravel rdf:type rdfs:Class . 
ies:CarTravel sparx:guid "{F5E2BCD3-4529-42f2-9ED9-95801B42ED3F}" . 
ies:CarTravel rdfs:comment "A TravelService by car" . 
ies:CarTravel rdfs:subClassOf ies:Transit . 
ies:CashPayment rdf:type rdfs:Class . 
ies:CashPayment sparx:guid "{62A9AA44-6C36-448b-805F-E13203CFB4FC}" . 
ies:CashPayment rdfs:comment "An EventParticipant where an AmountOfMoney in cash is used as payment in a Purchase.When neither card nor cash is used, there will be an accompanying MoneyTransfer" . 
ies:CashPayment rdfs:subClassOf ies:EventParticipant . 
ies:Casualty rdf:type rdfs:Class . 
ies:Casualty sparx:guid "{61D00F47-977E-43f6-BD30-77CBAAA74CC1}" . 
ies:Casualty rdfs:comment "Relates a MilitaryAttack to a Person who was injured or killed in the attack" . 
ies:Casualty rdfs:subClassOf ies:EventParticipant . 
ies:CBRadioHandset rdf:type rdfs:Class . 
ies:CBRadioHandset sparx:guid "{18EB7B22-5927-4b0e-98A8-638D28BDCF87}" . 
ies:CBRadioHandset rdfs:comment "A CommunicationsDevice used to hold radio conversations on frequencies allocated as Citizen Band" . 
ies:CBRadioHandset rdfs:subClassOf ies:CommunicationsDevice . 
ies:CellularBaseStation rdf:type rdfs:Class . 
ies:CellularBaseStation sparx:guid "{9D4A1395-8687-4f0b-BC5D-61A756210B4D}" . 
ies:CellularBaseStation rdfs:comment "A RadioMast that is used for cellular communication" . 
ies:CellularBaseStation rdfs:subClassOf ies:RadioMast . 
ies:CellularBaseStation rdfs:subClassOf ies:SystemState . 
ies:ChangeOfGovernment rdf:type rdfs:Class . 
ies:ChangeOfGovernment sparx:guid "{7FA15F56-86C4-47f4-9032-999C17703368}" . 
ies:ChangeOfGovernment rdfs:comment "A PoliticalEvent where one Government is replaced by another." . 
ies:ChangeOfGovernment rdfs:subClassOf ies:PoliticalEvent . 
ies:Characteristic rdf:type rdfs:Class . 
ies:Characteristic sparx:guid "{A7F266E8-B1CB-4b9b-8AF1-1EF2A7D8F5EE}" . 
ies:Characteristic rdfs:comment "A ClassOfElement whose instances all share a common property - e.g. they are all the same colour, mass, etc. " . 
ies:Characteristic rdfs:subClassOf ies:ClassOfElement . 
ies:charters rdf:type owl:ObjectProperty . 
ies:charters sparx:guid "{48223A62-12E6-4953-8F80-8C7A48151825}" . 
ies:charters rdfs:comment "A Relationship between a ResponsibleActor and the Transit they have chartered." . 
ies:charters rdfs:subPropertyOf ies:relationship . 
ies:charters rdfs:domain ies:ResponsibleActor . 
ies:charters rdfs:range ies:Transit . 
ies:CheckIn rdf:type rdfs:Class . 
ies:CheckIn sparx:guid "{87308A03-5C79-4d94-99E1-660042AC7929}" . 
ies:CheckIn rdfs:comment "An Event where a Person checks in to a hotel or Transit. This also includes swiping tickets to use public transportThe location of the CheckIn is specified using a happensIn relationship.The CheckIn may be part of another Event - e.g. an EntertainmentEvent or Transit event. Simply use the isPartOf relationship to specify this." . 
ies:CheckIn rdfs:subClassOf ies:Event . 
ies:CinemaTicket rdf:type rdfs:Class . 
ies:CinemaTicket sparx:guid "{7E0C25C9-DD3A-463e-A481-7CA4EA4AC8C5}" . 
ies:CinemaTicket rdfs:comment "An EntertainmentTicket that permits attendance at a cinema" . 
ies:CinemaTicket rdfs:subClassOf ies:EntertainmentTicket . 
ies:ClassOfAccount rdf:type rdfs:Class . 
ies:ClassOfAccount sparx:guid "{0077DA88-19EF-4c4c-B6C0-D418D5D77256}" . 
ies:ClassOfAccount rdfs:comment "The powertype of Account" . 
ies:ClassOfAccount rdfs:subClassOf ies:ClassOfEntity . 
ies:ClassOfAmountOfMoney rdf:type rdfs:Class . 
ies:ClassOfAmountOfMoney sparx:guid "{E5C27DA8-7DF1-49ea-A9EC-ABE17AFD2047}" . 
ies:ClassOfAmountOfMoney rdfs:comment "The powertype of AmountOfMoney" . 
ies:ClassOfAmountOfMoney rdfs:subClassOf ies:ClassOfAsset . 
ies:ClassOfAsset rdf:type rdfs:Class . 
ies:ClassOfAsset sparx:guid "{F999F59A-7C7B-40f3-8F86-5B2592889E95}" . 
ies:ClassOfAsset rdfs:comment "The powertype of Asset- i.e. a ClassOfEntity whose instances are classes of AssetExamples:* Vauxhall Insignia, VW Golf* Smartphone* Apple iPhone 6S" . 
ies:ClassOfAsset rdfs:subClassOf ies:ClassOfEntity . 
ies:ClassOfClassOfElement rdf:type rdfs:Class . 
ies:ClassOfClassOfElement sparx:guid "{85305668-DE1A-454a-87EE-346A221E846C}" . 
ies:ClassOfClassOfElement rdfs:comment "An rdfs:Class and an ExchangedItem whose instances are classes of classes of Element" . 
ies:ClassOfClassOfElement rdfs:subClassOf ies:ExchangedItem . 
ies:ClassOfClassOfElement rdfs:subClassOf rdfs:Class . 
ies:ClassOfClassOfEntity rdf:type rdfs:Class . 
ies:ClassOfClassOfEntity sparx:guid "{1F9AC8FE-3862-48d6-A3DC-E429B08D2B26}" . 
ies:ClassOfClassOfEntity rdfs:comment "The powertype of ClassOfEntity" . 
ies:ClassOfClassOfEntity rdfs:subClassOf ies:ClassOfClassOfElement . 
ies:ClassOfCriminalActivity rdf:type rdfs:Class . 
ies:ClassOfCriminalActivity sparx:guid "{69868D83-C3BD-4877-AB5C-374B4C6F4A7E}" . 
ies:ClassOfCriminalActivity rdfs:comment "The powertype of CriminalActivityExample instances:* Burglary* Fraud* Murder* Driving sheep across London Bridge if not a freeman of the City* Being Welsh inside the walls of Chester outside daylight hours" . 
ies:ClassOfCriminalActivity rdfs:subClassOf ies:ClassOfEvent . 
ies:ClassOfDevice rdf:type rdfs:Class . 
ies:ClassOfDevice sparx:guid "{09F9136C-9069-47ec-A58E-FC26CF9BA55E}" . 
ies:ClassOfDevice rdfs:comment "The powertype of Device- i.e. a ClassOfEntity whose instances are classes of DeviceExamples:* Smartphone* Apple iPhone 6S" . 
ies:ClassOfDevice rdfs:subClassOf ies:ClassOfElement . 
ies:ClassOfDevice rdfs:subClassOf ies:ClassOfAsset . 
ies:ClassOfElement rdf:type rdfs:Class . 
ies:ClassOfElement sparx:guid "{3C13E07D-5796-4d03-9EBC-C75277E87CA4}" . 
ies:ClassOfElement rdfs:comment "An rdfs:Class and an ExchangedItem whose instances are classes of ElementExamples:	Human groupings (e.g. Nigerian Women, British Men, Righthanded people, English Speakers);	Political Ideologies	Weapons	Days of the week	Standard procedures	etc." . 
ies:ClassOfElement rdfs:subClassOf ies:ExchangedItem . 
ies:ClassOfElement rdfs:subClassOf rdfs:Class . 
ies:ClassOfEntity rdf:type rdfs:Class . 
ies:ClassOfEntity sparx:guid "{D1B2FB30-36CA-4012-B85F-514E270BF541}" . 
ies:ClassOfEntity rdfs:comment "The powertype of Entity - i.e. a ClassOfElement whose instances are classes of EntityExamples:� Human groupings (e.g. Nigerian Women, British Men, Righthanded people, English Speakers);� Weapons� Etc." . 
ies:ClassOfEntity rdfs:subClassOf ies:ClassOfElement . 
ies:ClassOfEntity ies:powertype ies:ClassOfClassOfEntity . 
ies:ClassOfEvent rdf:type rdfs:Class . 
ies:ClassOfEvent sparx:guid "{4EA194C6-BBF9-45ab-85DE-5802D8C3A531}" . 
ies:ClassOfEvent rdfs:comment "An ClassOfElement whose instances are classes of Event. This is the powertype of Event.Examples:* Conference* Football Match* Annual General Meeting" . 
ies:ClassOfEvent rdfs:subClassOf ies:ClassOfElement . 
ies:ClassOfFinancialAccount rdf:type rdfs:Class . 
ies:ClassOfFinancialAccount sparx:guid "{901334E9-238C-4d05-8F85-FE9A8E537BA1}" . 
ies:ClassOfFinancialAccount rdfs:comment "The powertype of FinancialAccountExamples:* Savings Account* Current Account* Credit Card Account" . 
ies:ClassOfFinancialAccount rdfs:subClassOf ies:ClassOfAccount . 
ies:ClassOfIndividualDocument rdf:type rdfs:Class . 
ies:ClassOfIndividualDocument sparx:guid "{CCC8FA06-CDA8-491d-BFFC-0A88D6A565B1}" . 
ies:ClassOfIndividualDocument rdfs:comment "The powertype of IndividualDocument" . 
ies:ClassOfIndividualDocument rdfs:subClassOf ies:Representation . 
ies:ClassOfMeasureValue rdf:type rdfs:Class . 
ies:ClassOfMeasureValue sparx:guid "{4520A91C-D956-46c1-9A81-93C4C0B12880}" . 
ies:ClassOfMeasureValue rdfs:comment "A ClassOfRepresentation that is the powertype of MeasureValue" . 
ies:ClassOfMeasureValue rdfs:subClassOf ies:ClassOfRepresentation . 
ies:ClassOfMoneyTransfer rdf:type rdfs:Class . 
ies:ClassOfMoneyTransfer sparx:guid "{F1AACA77-BA24-41cb-9AB8-7AF9C1B9971D}" . 
ies:ClassOfMoneyTransfer rdfs:comment "The powertype of MoneyTransferExamples:* BACS* CHAPS* Paypal payment" . 
ies:ClassOfMoneyTransfer rdfs:subClassOf ies:ClassOfEvent . 
ies:ClassOfOnlineService rdf:type rdfs:Class . 
ies:ClassOfOnlineService sparx:guid "{FBE0CFC1-43C4-47e2-9EFE-20E291A1697C}" . 
ies:ClassOfOnlineService rdfs:comment "The powertype of OnlineService" . 
ies:ClassOfOnlineService rdfs:subClassOf ies:ClassOfWebResource . 
ies:ClassOfOperationalEvent rdf:type rdfs:Class . 
ies:ClassOfOperationalEvent sparx:guid "{64CE6FEA-7B05-4813-BD55-D56C02A54486}" . 
ies:ClassOfOperationalEvent rdfs:comment "The powertype of OperationalEventExamples:* Counter-Narcotics Operation* Murder Investigation" . 
ies:ClassOfOperationalEvent rdfs:subClassOf ies:ClassOfEvent . 
ies:ClassOfOrganisation rdf:type rdfs:Class . 
ies:ClassOfOrganisation sparx:guid "{5B21F148-72C1-45e6-A3E3-F2D8B33729D3}" . 
ies:ClassOfOrganisation rdfs:comment "The powertype of OrganisationNote: care should be exercised when using ClassOfOrganisation - it should only be used for classifications that apply to the whole life of the organisation." . 
ies:ClassOfOrganisation rdfs:subClassOf ies:ClassOfResponsibleActor . 
ies:ClassOfPaymentArtefact rdf:type rdfs:Class . 
ies:ClassOfPaymentArtefact sparx:guid "{46144D4F-5A9F-432b-B533-26C0399DBB34}" . 
ies:ClassOfPaymentArtefact rdfs:comment "The powertype of PaymentArtefactExamples:* Visa* Oyster* Selfridges Store Card" . 
ies:ClassOfPaymentArtefact rdfs:subClassOf ies:ClassOfElement . 
ies:ClassOfPaymentArtefact rdfs:subClassOf ies:ClassOfAsset . 
ies:ClassOfPerson rdf:type rdfs:Class . 
ies:ClassOfPerson sparx:guid "{2A62C672-1757-4a2d-874B-C099C9DEC416}" . 
ies:ClassOfPerson rdfs:comment "The powertype of Person" . 
ies:ClassOfPerson rdfs:subClassOf ies:ClassOfResponsibleActor . 
ies:ClassOfPersonState rdf:type rdfs:Class . 
ies:ClassOfPersonState sparx:guid "{92CDC810-9DFA-476b-A2E7-33121F65905B}" . 
ies:ClassOfPersonState rdfs:comment "The powertype of PersonState" . 
ies:ClassOfPersonState rdfs:subClassOf ies:ClassOfResponsibleActorState . 
ies:ClassOfRepresentation rdf:type rdfs:Class . 
ies:ClassOfRepresentation sparx:guid "{4FFEB84D-B823-4829-9A3A-ADE51EF0F0F5}" . 
ies:ClassOfRepresentation rdfs:comment "The powertype of Representation" . 
ies:ClassOfRepresentation rdfs:subClassOf ies:ClassOfClassOfEntity . 
ies:ClassOfResponsibleActor rdf:type rdfs:Class . 
ies:ClassOfResponsibleActor sparx:guid "{9FC2431D-63A4-4e1b-8D31-2BCD125853D9}" . 
ies:ClassOfResponsibleActor rdfs:comment "The powertype of ResponsibleActor " . 
ies:ClassOfResponsibleActor rdfs:subClassOf ies:ClassOfEntity . 
ies:ClassOfResponsibleActorState rdf:type rdfs:Class . 
ies:ClassOfResponsibleActorState sparx:guid "{9CEF4F29-5619-4d8f-A9DE-8CB43270C7F5}" . 
ies:ClassOfResponsibleActorState rdfs:comment "A ClassOfState that is the powertype of ResponsibleActorState " . 
ies:ClassOfResponsibleActorState rdfs:subClassOf ies:ClassOfState . 
ies:ClassOfState rdf:type rdfs:Class . 
ies:ClassOfState sparx:guid "{0358DDAB-D22C-4ee5-8F9A-CF18F3E432BD}" . 
ies:ClassOfState rdfs:comment "A ClassOfElement whose instances are classes of States. This is the powertype of State.Examples:* Roles" . 
ies:ClassOfState rdfs:subClassOf ies:ClassOfElement . 
ies:ClassOfTravelBooking rdf:type rdfs:Class . 
ies:ClassOfTravelBooking sparx:guid "{44D4DD7C-201A-447d-8BCE-C8B3E3E6A890}" . 
ies:ClassOfTravelBooking rdfs:comment "The powertype of TravelBookingExamples:INTERNET BookingTELEPHONE Booking" . 
ies:ClassOfTravelBooking rdfs:subClassOf ies:ClassOfEvent . 
ies:ClassOfTravelVisa rdf:type rdfs:Class . 
ies:ClassOfTravelVisa sparx:guid "{2BADCB50-7A19-4d7b-A46E-8369F8B00D57}" . 
ies:ClassOfTravelVisa rdfs:comment "The powertype of TravelVisa" . 
ies:ClassOfTravelVisa rdfs:subClassOf ies:ClassOfIndividualDocument . 
ies:ClassOfWebResource rdf:type rdfs:Class . 
ies:ClassOfWebResource sparx:guid "{B1AAE4CA-CAB0-475f-B7D3-8CED404B1FC6}" . 
ies:ClassOfWebResource rdfs:comment "The powertype of WebResource" . 
ies:ClassOfWebResource rdfs:subClassOf ies:ClassOfEntity . 
ies:CloseAccount rdf:type rdfs:Class . 
ies:CloseAccount sparx:guid "{2A5450A7-5B26-4605-A109-5CB26DD9A70F}" . 
ies:CloseAccount rdfs:comment "An AccountAdminEvent where an Account is shut down." . 
ies:CloseAccount rdfs:subClassOf ies:AccountAdminEvent . 
ies:coercedBy rdf:type owl:ObjectProperty . 
ies:coercedBy sparx:guid "{9E413787-42C8-4cd4-B7B1-63E38F6A02D9}" . 
ies:coercedBy rdfs:comment "A Relationship between two ResponsibleActor Entities where one (range) coerces the other (domain)." . 
ies:coercedBy rdfs:subPropertyOf ies:relationship . 
ies:coercedBy rdfs:range ies:ResponsibleActor . 
ies:coercedBy rdfs:domain ies:ResponsibleActorState . 
ies:CoLocation rdf:type rdfs:Class . 
ies:CoLocation sparx:guid "{3524D10D-D9B0-416d-ADED-D5AAEB99DD09}" . 
ies:CoLocation rdfs:comment "An Event where the activity is uncertain, but it is known that some Entities were presentNote: whilst colocation can be easily inferred from data, sometimes its important to call out specific instances where entities of interest were in the same place at the same time." . 
ies:CoLocation rdfs:subClassOf ies:Event . 
ies:Colour rdf:type rdfs:Class . 
ies:Colour sparx:guid "{B10D22FB-1D6A-47c9-B1C0-E870D43A5C52}" . 
ies:Colour rdfs:comment "An Characteristic whose members all have the same colour" . 
ies:Colour rdfs:subClassOf ies:Characteristic . 
ies:CommercialOrganisation rdf:type rdfs:Class . 
ies:CommercialOrganisation sparx:guid "{1456439C-65C9-4a39-A743-09A7D0FBF248}" . 
ies:CommercialOrganisation rdfs:comment "An Organisation that is run for profit" . 
ies:CommercialOrganisation rdfs:subClassOf ies:Organisation . 
ies:Communication rdf:type rdfs:Class . 
ies:Communication sparx:guid "{6698805F-F492-4f1f-954C-E1EB3C53E148}" . 
ies:Communication rdfs:comment "An Event where two or more parties interact and exchange information" . 
ies:Communication rdfs:subClassOf ies:Event . 
ies:CommunicationsAccount rdf:type rdfs:Class . 
ies:CommunicationsAccount sparx:guid "{8300451C-1DF9-4545-9174-D8AA69C58CCD}" . 
ies:CommunicationsAccount rdfs:comment "An Account of the communications transactions provided to a customer" . 
ies:CommunicationsAccount rdfs:subClassOf ies:CommunicationsAccountState . 
ies:CommunicationsAccount rdfs:subClassOf ies:Account . 
ies:CommunicationsAccountState rdf:type rdfs:Class . 
ies:CommunicationsAccountState sparx:guid "{20BB42F0-3F2D-4bb7-88DD-F4D05377D59B}" . 
ies:CommunicationsAccountState rdfs:comment "A temporal state of a CommunicationsAccount" . 
ies:CommunicationsAccountState rdfs:subClassOf ies:AccountState . 
ies:CommunicationsDevice rdf:type rdfs:Class . 
ies:CommunicationsDevice sparx:guid "{32EB46A5-0FA4-44e9-A9E9-9424E80BDE91}" . 
ies:CommunicationsDevice rdfs:comment "A Device that provides an endpoint for communications � e.g. mobile telephone, landline, satellite phone, CB Radio, etc." . 
ies:CommunicationsDevice rdfs:subClassOf ies:Device . 
ies:CommunicationsIdentifier rdf:type rdfs:Class . 
ies:CommunicationsIdentifier sparx:guid "{A82378B9-9774-46b9-9845-CC75BE882F06}" . 
ies:CommunicationsIdentifier rdfs:comment "An Identifier for the end-point of a communication " . 
ies:CommunicationsIdentifier rdfs:subClassOf ies:Identifier . 
ies:CommunicationsIdentifierRange rdf:type rdfs:Class . 
ies:CommunicationsIdentifierRange sparx:guid "{DF388418-F296-46a5-A2A3-4297F084DD07}" . 
ies:CommunicationsIdentifierRange rdfs:comment "A specified range of identifiers for the end-points of a communication." . 
ies:CommunicationsIdentifierRange rdfs:subClassOf ies:CommunicationsIdentifier . 
ies:Competition rdf:type rdfs:Class . 
ies:Competition sparx:guid "{98421510-0A8A-4942-9743-191EA0DCA9E6}" . 
ies:Competition rdfs:comment "An Event where the participants are competing with each other" . 
ies:Competition rdfs:subClassOf ies:Event . 
ies:Competitor rdf:type rdfs:Class . 
ies:Competitor sparx:guid "{763C82F1-5CE0-4652-8A93-D56D93DE1544}" . 
ies:Competitor rdfs:comment "An EventParticipant where a ResponsibleActor is in competition" . 
ies:Competitor rdfs:subClassOf ies:EventParticipant . 
ies:Competitor rdfs:subClassOf ies:ResponsibleActorState . 
ies:ConcertTicket rdf:type rdfs:Class . 
ies:ConcertTicket sparx:guid "{8FF9DE7F-137B-4a03-AB24-7D84FCFB99C0}" . 
ies:ConcertTicket rdfs:comment "An EntertainmentTicket where the Event is a concert" . 
ies:ConcertTicket rdfs:subClassOf ies:EntertainmentTicket . 
ies:ConferenceHost rdf:type rdfs:Class . 
ies:ConferenceHost sparx:guid "{B59AB165-6D9C-423f-9CB2-85B4E1B37D93}" . 
ies:ConferenceHost rdfs:comment "A ConferenceParticipant that is in the role of host" . 
ies:ConferenceHost rdfs:subClassOf ies:ConferenceParticipant . 
ies:ConferenceParticipant rdf:type rdfs:Class . 
ies:ConferenceParticipant sparx:guid "{5C76FE3F-FE06-4abc-B495-0D4F35FB5252}" . 
ies:ConferenceParticipant rdfs:comment "An PartyInCommunication that is a participant in a TeleConference" . 
ies:ConferenceParticipant rdfs:subClassOf ies:PartyInCommunication . 
ies:confidence rdf:type owl:DatatypeProperty . 
ies:confidence sparx:guid "{45FE24B3-B146-4199-B760-C1150CEF9AB2}" . 
ies:confidence rdfs:comment "A qualitative or quantitative indication of the confidence of an AssessToBeTrue " . 
ies:confidence rdfs:subPropertyOf ies:attribute . 
ies:confidence rdfs:domain ies:AssessToBeTrue . 
ies:contactDetailsOnBooking rdf:type owl:DatatypeProperty . 
ies:contactDetailsOnBooking sparx:guid "{B54BB629-E007-4099-BC01-B512894F1E89}" . 
ies:contactDetailsOnBooking rdfs:comment "The contact details of the Person making the booking as recorded on the actual Travel Booking.Note that if these details can be parsed to identify the contact telephone number, contact email address etc. then they should be mapped as instances of relationship to the respective CommunicationsIdentifier (TelephoneNumber, EmailAddress, etc.)." . 
ies:contactDetailsOnBooking rdfs:subPropertyOf ies:attribute . 
ies:contactDetailsOnBooking rdfs:domain ies:TravelBooking . 
ies:ContentCategory rdf:type rdfs:Class . 
ies:ContentCategory sparx:guid "{8CA5551A-EAEB-4145-A75F-2E7D7DAD5A57}" . 
ies:ContentCategory rdfs:comment "An ClassOfClassOfEntity whose instances collect together all Representations that have similar content.Examples:* Fiction* Non-Fiction* Financial Information* Extremist Media" . 
ies:ContentCategory rdfs:subClassOf ies:ClassOfRepresentation . 
ies:ContinuousState rdf:type rdfs:Class . 
ies:ContinuousState sparx:guid "{6E5AF4BB-BB7F-4387-A7BB-476B81FEC103}" . 
ies:ContinuousState rdfs:comment "A State that is temporally continuous - i.e. it is not a DiscontinuousState" . 
ies:ContinuousState rdfs:subClassOf ies:State . 
ies:contractedTo rdf:type owl:ObjectProperty . 
ies:contractedTo sparx:guid "{0876AE1F-7202-41d9-A00F-208B118BBF79}" . 
ies:contractedTo rdfs:comment "A worksFor relationship where a ResponsibleActor (domain) is contracted to another ResponsibleActor (range)." . 
ies:contractedTo rdfs:subPropertyOf ies:worksFor . 
ies:Cookie rdf:type rdfs:Class . 
ies:Cookie sparx:guid "{C81B6EAD-8494-45ca-928C-21CB6D395C39}" . 
ies:Cookie rdfs:comment "An OnlineArtefact that is stored on a Device to enable continuity of session, log-in, or simply to track activity online.Cookies tend to be ephemeral, an unique to a device, so no states are required. Simply use cookieOnDevice relationship mark the stand and end BoundingStates of the Cookie. " . 
ies:Cookie rdfs:subClassOf ies:OnlineArtefact . 
ies:cookieOnDevice rdf:type owl:ObjectProperty . 
ies:cookieOnDevice sparx:guid "{76D8EA41-E338-4db5-BB30-D642CF0F90EB}" . 
ies:cookieOnDevice rdfs:comment "Relates a Cookie to the Device it is installed on.Note: there is usually no need for states here as the Cookie itself has begin and end times." . 
ies:cookieOnDevice rdfs:subPropertyOf ies:relationship . 
ies:cookieOnDevice rdfs:domain ies:Cookie . 
ies:cookieOnDevice rdfs:range ies:Device . 
ies:cookieOriginSite rdf:type owl:ObjectProperty . 
ies:cookieOriginSite sparx:guid "{24E8B958-284F-4be2-AACD-A7B2A94B97D4}" . 
ies:cookieOriginSite rdfs:comment "Relates a Cookie to the Webpage from which it originated." . 
ies:cookieOriginSite rdfs:subPropertyOf ies:relationship . 
ies:cookieOriginSite rdfs:domain ies:Cookie . 
ies:cookieOriginSite rdfs:range ies:Webpage . 
ies:Cooperation rdf:type rdfs:Class . 
ies:Cooperation sparx:guid "{F650B9E3-2669-455e-B20C-92737CFD9A08}" . 
ies:Cooperation rdfs:comment "An Event where the participants are cooperating with each other" . 
ies:Cooperation rdfs:subClassOf ies:Event . 
ies:Cooperator rdf:type rdfs:Class . 
ies:Cooperator sparx:guid "{2B96182A-9363-4c6a-BE62-132B072A7520}" . 
ies:Cooperator rdfs:comment "An EventParticipant where a ResponsibleActor is in Cooperation" . 
ies:Cooperator rdfs:subClassOf ies:EventParticipant . 
ies:Cooperator rdfs:subClassOf ies:ResponsibleActorState . 
ies:Country rdf:type rdfs:Class . 
ies:Country sparx:guid "{92EBA9B9-48C2-4082-9FE5-603977BD6846}" . 
ies:Country rdfs:comment "A Location whose land extent / borders are recognised as a Country by the International Standards Organisation (ISO)Note: this is simply the land, any buildings on it, and the airspace and ground beneath as recognised by the ISO definition. It does not include the nationals of the Country, its Government, etc. " . 
ies:Country rdfs:subClassOf ies:Location . 
ies:countryOfRegistration rdf:type owl:ObjectProperty . 
ies:countryOfRegistration sparx:guid "{D33498ED-B6A0-41ea-864F-CE95E2B1E010}" . 
ies:countryOfRegistration rdfs:comment "The Country in which the respective Entity is registered / recognised." . 
ies:countryOfRegistration rdfs:domain ies:Account . 
ies:countryOfRegistration rdfs:domain ies:Organisation . 
ies:countryOfRegistration rdfs:range ies:Country . 
ies:countryOfRegistration rdfs:subPropertyOf ies:relationship . 
ies:countryOfRegistration rdfs:domain ies:Vehicle . 
ies:countryUsingDialCode rdf:type owl:ObjectProperty . 
ies:countryUsingDialCode sparx:guid "{8C3F2C71-C7A2-414a-85C2-DFCD2D91D8E5}" . 
ies:countryUsingDialCode rdfs:comment "A relationship between a TelephoneCountryCode and a Country that uses that code.Note:  more than one Country may use the same code, and in rare cases a given Country may have more than one code." . 
ies:countryUsingDialCode rdfs:subPropertyOf ies:relationship . 
ies:countryUsingDialCode rdfs:domain ies:TelephoneCountryCode . 
ies:countryUsingDialCode rdfs:range ies:Country . 
ies:cousinOf rdf:type owl:ObjectProperty . 
ies:cousinOf sparx:guid "{32A625FA-3159-4b36-B551-3742BA11C7A8}" . 
ies:cousinOf rdfs:comment "A Relationship between two Person Entities that indicates one is the cousin of the other" . 
ies:cousinOf rdfs:subPropertyOf ies:familiallyRelatedTo . 
ies:cousinOf rdfs:domain ies:Person . 
ies:cousinOf rdfs:range ies:Person . 
ies:Create rdf:type rdfs:Class . 
ies:Create sparx:guid "{AF60517B-E4EF-48ca-BE0F-56E0A89660FD}" . 
ies:Create rdfs:comment "A LifecycleEvent where an Entity is brought into existence." . 
ies:Create rdfs:subClassOf ies:LifecycleEvent . 
ies:Created rdf:type rdfs:Class . 
ies:Created sparx:guid "{46DE5D1F-B3CE-4858-A6D1-64A0B891A00F}" . 
ies:Created rdfs:comment "An EventParticipant where an Entity is createdThe date/time of the creation can be specified using the inPeriod relationship. " . 
ies:Created rdfs:subClassOf ies:EventParticipant . 
ies:Created rdfs:subClassOf ies:BoundingState . 
ies:CreatedContent rdf:type rdfs:Class . 
ies:CreatedContent sparx:guid "{1EBC6375-B26C-4506-B4DE-85B74E476362}" . 
ies:CreatedContent rdfs:comment "A Create EventParticipant where online content is created" . 
ies:CreatedContent rdfs:subClassOf ies:Created . 
ies:Creator rdf:type rdfs:Class . 
ies:Creator sparx:guid "{850DB6D5-C8E8-4aa8-87A0-4E7680FF854A}" . 
ies:Creator rdfs:comment "An EventParticipant where a ResponsibleActor participates in a Create event as a creator" . 
ies:Creator rdfs:subClassOf ies:ActiveEventParticipant . 
ies:CreditCard rdf:type rdfs:Class . 
ies:CreditCard sparx:guid "{C2174205-C96F-4427-A401-19C1DEF0E4AF}" . 
ies:CreditCard rdfs:comment "A BankCard that allows the customer to carry a line of credit" . 
ies:CreditCard rdfs:subClassOf ies:BankCard . 
ies:CriminalActivity rdf:type rdfs:Class . 
ies:CriminalActivity sparx:guid "{43E58528-16E4-48b3-8F13-10500879EA83}" . 
ies:CriminalActivity rdfs:comment "An Event which is illegal within the laws of the jurisdiction in which it takes place.Note: If the CriminalActivity falls into one of the Home Office Offence Classification Index codes, then this should be provided using the offenceCode attribute." . 
ies:CriminalActivity rdfs:subClassOf ies:Event . 
ies:CriminalOrganisation rdf:type rdfs:Class . 
ies:CriminalOrganisation sparx:guid "{3CEFB37C-D5EE-4c9d-848D-C8E2DB206482}" . 
ies:CriminalOrganisation rdfs:comment "An OrganisationState that is assessed to be breaking the law in an organised manner" . 
ies:CriminalOrganisation rdfs:subClassOf ies:OrganisationState . 
ies:Crossing rdf:type rdfs:Class . 
ies:Crossing sparx:guid "{B85F065A-6A18-433e-9195-7B6BCBB91C7C}" . 
ies:Crossing rdfs:comment "A Location and an ArbitraryOverlap whose extent is defined by the shared overlap of two or more Locations" . 
ies:Crossing rdfs:subClassOf ies:Location . 
ies:Crossing rdfs:subClassOf ies:ArbitraryOverlap . 
ies:crossingOf rdf:type owl:ObjectProperty . 
ies:crossingOf sparx:guid "{5A0E8F10-EE46-49bd-8E25-A67040D4A40B}" . 
ies:crossingOf rdfs:comment "A partOf relationship to indicate a Location (range) has a Crossing (domain)" . 
ies:crossingOf rdfs:subPropertyOf ies:isPartOf . 
ies:crossingOf rdfs:domain ies:Crossing . 
ies:crossingOf rdfs:range ies:Location . 
ies:Currency rdf:type rdfs:Class . 
ies:Currency sparx:guid "{A06EE74F-9A66-4b63-8DC3-3B1C2B362862}" . 
ies:Currency rdfs:comment "A ClassOfAmountOfMoney that is the denomination as currency.The identifier should be specified as an ISO4217 three-letter code (e.g. USD, GBP, EUR, etc.)" . 
ies:Currency rdfs:subClassOf ies:ClassOfAmountOfMoney . 
ies:currencyAmount rdf:type owl:DatatypeProperty . 
ies:currencyAmount sparx:guid "{C53F62D0-0817-404b-9624-95A89D94F9A2}" . 
ies:currencyAmount rdfs:comment "A number that represents the amount of currency. Note: sometimes the number and/or the currency may be unknown and therefore not instantiated" . 
ies:currencyAmount rdfs:subPropertyOf ies:attribute . 
ies:currencyAmount rdfs:domain ies:AmountOfMoney . 
ies:currencyDenomination rdf:type owl:ObjectProperty . 
ies:currencyDenomination sparx:guid "{AE8A5533-9C08-46e7-8131-E3D119F6AAE3}" . 
ies:currencyDenomination rdfs:comment "The currency in which the AmountOfMoney is denominated" . 
ies:currencyDenomination rdfs:subPropertyOf ies:relationship . 
ies:currencyDenomination rdfs:domain ies:AmountOfMoney . 
ies:currencyDenomination rdfs:range ies:Currency . 
ies:currencyDenomination rdfs:subPropertyOf rdf:type . 
ies:Customer rdf:type rdfs:Class . 
ies:Customer sparx:guid "{76689446-5969-49d3-8E7E-A92C86C244D5}" . 
ies:Customer rdfs:comment "An EventParticipant where a ResponsibleActor is the customer for the Event - i.e. the Event has been conducted as a service to them, or in production of goods for them." . 
ies:Customer rdfs:subClassOf ies:ActiveEventParticipant . 
ies:CustomerIdentifier rdf:type rdfs:Class . 
ies:CustomerIdentifier sparx:guid "{43560C95-66A3-4d69-A743-F0A166DE51FC}" . 
ies:CustomerIdentifier rdfs:comment "The customer identifier associated with the Financial Account.A single Customer Identity could be associated with more than one Financial Account managed by the same provider." . 
ies:CustomerIdentifier rdfs:subClassOf ies:Identifier . 
ies:CyberStalking rdf:type rdfs:Class . 
ies:CyberStalking sparx:guid "{8CF52FB7-69F2-4ef2-8074-FB90EE924139}" . 
ies:CyberStalking rdfs:comment "A form of Stalking which takes place online." . 
ies:CyberStalking rdfs:subClassOf ies:Stalking . 
ies:Database rdf:type rdfs:Class . 
ies:Database sparx:guid "{3099B032-4B0A-4aec-ABCD-3E862C4C1979}" . 
ies:Database rdfs:comment "A DataObject that is the contents of an entire database (note this is still a class, as there may be many copies of the database)" . 
ies:Database rdfs:subClassOf ies:DataObject . 
ies:DatabaseItem rdf:type rdfs:Class . 
ies:DatabaseItem sparx:guid "{73F8D96C-A9EC-4301-9968-0F7BF9826C45}" . 
ies:DatabaseItem rdfs:comment "A DataObject that is part of the data in a DatabaseExamples:* A table, row, column in RDBMS* A document in a document db* a key-value pair in KVDB* named graph in a graph db" . 
ies:DatabaseItem rdfs:subClassOf ies:DataObject . 
ies:DatabaseRow rdf:type rdfs:Class . 
ies:DatabaseRow sparx:guid "{1F23EB62-323B-402d-84BD-B4D417ED1A73}" . 
ies:DatabaseRow rdfs:comment "A DataObject that is an entire row of a table in a database (note this is still a class, as there may be many copies of the database)" . 
ies:DatabaseRow rdfs:subClassOf ies:DatabaseItem . 
ies:DatabaseTable rdf:type rdfs:Class . 
ies:DatabaseTable sparx:guid "{D9E56CAA-4668-4248-B087-C041363816DD}" . 
ies:DatabaseTable rdfs:comment "A DataObject that is the entire contents of a table in a database (note this is still a class, as there may be many copies of the database)" . 
ies:DatabaseTable rdfs:subClassOf ies:DatabaseItem . 
ies:DataKey rdf:type rdfs:Class . 
ies:DataKey sparx:guid "{2D88DE83-F87F-48ad-A485-9FFA79ED90D8}" . 
ies:DataKey rdfs:comment "A unique key (usually only unique within a Database, though it could be a GUID) that identifies a DataObject" . 
ies:DataKey rdfs:subClassOf ies:Identifier . 
ies:DataObject rdf:type rdfs:Class . 
ies:DataObject sparx:guid "{CAC97EB4-E0E8-4576-9637-1FBED5F9FEF2}" . 
ies:DataObject rdfs:comment "A Representation which might contain internal structure that can be exploited using bespoke tools and/or applications. Data objects might be geoobjects, video files, audio files, etc." . 
ies:DataObject rdfs:subClassOf ies:Representation . 
ies:DeathState rdf:type rdfs:Class . 
ies:DeathState sparx:guid "{F6173D27-D86D-40f8-A5B0-36DCCF85D396}" . 
ies:DeathState rdfs:comment "A BoundingState that marks the end of a Persons lifeThe location of the death can be specified using inLocationThe date/time of the death can be specified using the inPeriod relationship. " . 
ies:DeathState rdfs:subClassOf ies:BoundingState . 
ies:DeathState rdfs:subClassOf ies:PersonState . 
ies:DebitCard rdf:type rdfs:Class . 
ies:DebitCard sparx:guid "{F0C846E7-76B9-4ab6-988E-3694C95818E7}" . 
ies:DebitCard rdfs:comment "A BankCard where transactions debit from a bank account" . 
ies:DebitCard rdfs:subClassOf ies:BankCard . 
ies:DeclarationOfWar rdf:type rdfs:Class . 
ies:DeclarationOfWar sparx:guid "{5E25DC95-E376-420f-9991-F5175476B386}" . 
ies:DeclarationOfWar rdfs:comment "A PoliticalAnnouncement marking the start of a War" . 
ies:DeclarationOfWar rdfs:subClassOf ies:PoliticalAnnouncement . 
ies:DeclaredTarget rdf:type rdfs:Class . 
ies:DeclaredTarget sparx:guid "{19B808BB-348E-4ea3-B62E-ED6356F7D4A0}" . 
ies:DeclaredTarget rdfs:comment "The Organisation against which War has been declared" . 
ies:DeclaredTarget rdfs:subClassOf ies:EventParticipant . 
ies:DeclaringParty rdf:type rdfs:Class . 
ies:DeclaringParty sparx:guid "{82139547-0CA1-448d-997F-3386EFDF049C}" . 
ies:DeclaringParty rdfs:comment "An EventParticipant where a ResponsibleActor makes an AnnouncementNote: this also covers GoverningParty from IES 3.2" . 
ies:DeclaringParty rdfs:subClassOf ies:EventParticipant . 
ies:Delivery rdf:type rdfs:Class . 
ies:Delivery sparx:guid "{F428ADA5-2349-4cd0-815F-8F768B08C6E6}" . 
ies:Delivery rdfs:comment "A TradeEvent where one or more Entities are delivered to the receiving party" . 
ies:Delivery rdfs:subClassOf ies:TradeEvent . 
ies:DeliveryAddress rdf:type rdfs:Class . 
ies:DeliveryAddress sparx:guid "{096F83D3-F25E-4d48-96E8-566731C06DB1}" . 
ies:DeliveryAddress rdfs:comment "An EventParticipant where an Address participates in a Delivery as a the location to which the delivery is made" . 
ies:DeliveryAddress rdfs:subClassOf ies:EventParticipant . 
ies:DeliveryRecipient rdf:type rdfs:Class . 
ies:DeliveryRecipient sparx:guid "{63289363-A4D6-4abf-BE19-6DCDDCF9B28F}" . 
ies:DeliveryRecipient rdfs:comment "An EventParticipant where a ResponsibleActor participates in a Delivery as a recipient" . 
ies:DeliveryRecipient rdfs:subClassOf ies:EventParticipant . 
ies:DemocraticChangeOfGovernment rdf:type rdfs:Class . 
ies:DemocraticChangeOfGovernment sparx:guid "{33C68A39-AF9C-4f37-97EA-1DE4BAC4F7FB}" . 
ies:DemocraticChangeOfGovernment rdfs:comment "A ChangeOfGovernment that comes about by democratic means" . 
ies:DemocraticChangeOfGovernment rdfs:subClassOf ies:ChangeOfGovernment . 
ies:Department rdf:type rdfs:Class . 
ies:Department sparx:guid "{6C7891C7-E095-41f4-A894-AA0C6A22F5D2}" . 
ies:Department rdfs:comment "An Organisation that is part of another Organisation - usually part of a CommercialOrganisation, though other Organisations have departments" . 
ies:Department rdfs:subClassOf ies:Organisation . 
ies:Departure rdf:type rdfs:Class . 
ies:Departure sparx:guid "{0FCBDA68-1B1C-40e1-9C5B-0E225CA827DB}" . 
ies:Departure rdfs:comment "An EventParticipant and a BoundingState that marks the start of a Travel eventThe date/time of the departure can be specified using the inPeriod relationship. " . 
ies:Departure rdfs:subClassOf ies:BoundingState . 
ies:Destroy rdf:type rdfs:Class . 
ies:Destroy sparx:guid "{27000BBA-F3F9-4355-B466-92CE04477C9B}" . 
ies:Destroy rdfs:comment "A LifecycleEvent where an Entity is destroyed" . 
ies:Destroy rdfs:subClassOf ies:LifecycleEvent . 
ies:Destroyed rdf:type rdfs:Class . 
ies:Destroyed sparx:guid "{E70CA8CD-51DC-4f77-982C-C233F9493FF9}" . 
ies:Destroyed rdfs:comment "An EventParticipant where an Entity is destroyed" . 
ies:Destroyed rdfs:subClassOf ies:EventParticipant . 
ies:Destroyer rdf:type rdfs:Class . 
ies:Destroyer sparx:guid "{C029299D-5946-48dd-94CB-80EC23A56300}" . 
ies:Destroyer rdfs:comment "An EventParticipant where a ResponsibleActor participates in a Destroy event as a destroyer" . 
ies:Destroyer rdfs:subClassOf ies:ActiveEventParticipant . 
ies:Device rdf:type rdfs:Class . 
ies:Device sparx:guid "{115F2F9B-21F3-4903-8EAA-AB3AEFE97461}" . 
ies:Device rdfs:comment "An Asset that is man-made and performs one or more functions - i.e. it is also an Actor" . 
ies:Device rdfs:subClassOf ies:Asset . 
ies:Device rdfs:subClassOf ies:DeviceState . 
ies:Device rdfs:subClassOf ies:Actor . 
ies:DeviceInCommunication rdf:type rdfs:Class . 
ies:DeviceInCommunication sparx:guid "{0073BD83-64CB-433c-BF4D-A6BB01862F14}" . 
ies:DeviceInCommunication rdfs:comment "A DeviceState (and an EventParticipant) when a Device is communicating. " . 
ies:DeviceInCommunication rdfs:subClassOf ies:EventParticipant . 
ies:DeviceInCommunication rdfs:subClassOf ies:DeviceState . 
ies:DeviceOnline rdf:type rdfs:Class . 
ies:DeviceOnline sparx:guid "{700BC564-35E1-4921-8759-5DAFA51B4E83}" . 
ies:DeviceOnline rdfs:comment "An EventParticipant where a Device participates in an OnlineEvent" . 
ies:DeviceOnline rdfs:subClassOf ies:EventParticipant . 
ies:DeviceOnline rdfs:subClassOf ies:DeviceState . 
ies:DeviceState rdf:type rdfs:Class . 
ies:DeviceState sparx:guid "{6107EEA5-1A13-46e4-83FB-14740437B814}" . 
ies:DeviceState rdfs:comment "A temporalState of a Device" . 
ies:DeviceState rdfs:subClassOf ies:AssetState . 
ies:dialInNumber rdf:type owl:DatatypeProperty . 
ies:dialInNumber sparx:guid "{73F2438B-77F5-49ee-B70D-84D5D50B378F}" . 
ies:dialInNumber rdfs:comment "The number dialed to take part in the TeleConference" . 
ies:dialInNumber rdfs:subPropertyOf ies:attribute . 
ies:dialInNumber rdfs:domain ies:TeleConference . 
ies:Disagreement rdf:type rdfs:Class . 
ies:Disagreement sparx:guid "{E73C74A9-B356-40a4-BDBB-40567592BBD0}" . 
ies:Disagreement rdfs:comment "An Event that covers the end-to-end disagreement between parties" . 
ies:Disagreement rdfs:subClassOf ies:Event . 
ies:DiscontinuousState rdf:type rdfs:Class . 
ies:DiscontinuousState sparx:guid "{52DB371E-71AC-4812-B3CF-0FD7D73F1BB0}" . 
ies:DiscontinuousState rdfs:comment "A State that is temporally dissected - i.e. it is not a continuous state, but in fact a fusion of states (which may or may not be specified)This is used for managing situations where something happens from time to time, and we dont always know when it happens. For example, if a vehicle is usually parked in a street, we would use a DiscontinuousState of the vehicle that would be inLocation." . 
ies:DiscontinuousState rdfs:subClassOf ies:State . 
ies:Dislikes rdf:type rdfs:Class . 
ies:Dislikes sparx:guid "{30A0F2DA-DB31-40fd-8723-88A24B2F8448}" . 
ies:Dislikes rdfs:comment "A Interested state where a ResponsibleActor dislikes something" . 
ies:Dislikes rdfs:subClassOf ies:Interested . 
ies:DispositionalClass rdf:type rdfs:Class . 
ies:DispositionalClass sparx:guid "{2855AF50-EEE4-4ced-B499-AE42423A4DE3}" . 
ies:DispositionalClass rdfs:comment "A ClassOfElement whose instances all share the same disposition - e.g. capability or tendencyExample: Vehicles capable of Mach 2" . 
ies:DispositionalClass rdfs:subClassOf ies:ClassOfElement . 
ies:disrespectfulOf rdf:type owl:ObjectProperty . 
ies:disrespectfulOf sparx:guid "{369D2CA7-BFFD-4bc3-941F-47262C3DBF1F}" . 
ies:disrespectfulOf rdfs:comment "A Relationship between two ResponsibleActor Entities where one is disrespectful of the other.Note: this should not be considered a bi-directional relationship. Just because one person disrespects another person does not necessarily mean the feeling is reciprocated. " . 
ies:disrespectfulOf rdfs:subPropertyOf ies:relationship . 
ies:disrespectfulOf rdfs:range ies:ResponsibleActor . 
ies:disrespectfulOf rdfs:domain ies:ResponsibleActorState . 
ies:distrusts rdf:type owl:ObjectProperty . 
ies:distrusts sparx:guid "{3499FB8A-AA42-4367-BBBC-79A69338BD70}" . 
ies:distrusts rdfs:comment "A Relationship between two ResponsibleActor Entities where one distrusts the other.Note: this should not be considered a bi-directional relationship. Just because one person distrusts another person does not necessarily mean the feeling is reciprocated. " . 
ies:distrusts rdfs:subPropertyOf ies:relationship . 
ies:distrusts rdfs:range ies:ResponsibleActor . 
ies:distrusts rdfs:domain ies:ResponsibleActorState . 
ies:documentedBy rdf:type owl:ObjectProperty . 
ies:documentedBy sparx:guid "{AC7C948A-F19C-4296-AC38-0FEE6A4C5E90}" . 
ies:documentedBy rdfs:comment "An isRepresentedAs relationship that asserts a WorkOfDocumentation is about an ExchangedItem" . 
ies:documentedBy rdfs:subPropertyOf ies:isRepresentedAs . 
ies:documentedBy rdfs:domain ies:ExchangedItem . 
ies:documentedBy rdfs:range ies:WorkOfDocumentation . 
ies:DocumentFormat rdf:type rdfs:Class . 
ies:DocumentFormat sparx:guid "{ACB44E46-7A30-4911-A9F0-3D5412FB3725}" . 
ies:DocumentFormat rdfs:comment "A ClassOfIndividualDocument whose members are all of the same document format - e.g.PDFMS Word" . 
ies:DocumentFormat rdfs:subClassOf ies:ClassOfIndividualDocument . 
ies:documentIdentifies rdf:type owl:ObjectProperty . 
ies:documentIdentifies sparx:guid "{2F8738A6-5EBA-4d80-980B-AA9E6F28B81A}" . 
ies:documentIdentifies rdfs:comment "Links an IdentityDocument to the Person it identifies.Note: was Is associated with in IES3" . 
ies:documentIdentifies rdfs:subPropertyOf ies:relationship . 
ies:documentIdentifies rdfs:domain ies:IdentityDocument . 
ies:documentIdentifies rdfs:range ies:Person . 
ies:DomainName rdf:type rdfs:Class . 
ies:DomainName sparx:guid "{42FFB9AC-2D28-453a-80A0-2A271DA32EB5}" . 
ies:DomainName rdfs:comment "A CommunicationsIdentifierRange that defines a realm of administrative autonomy, authority or control within the internet.  [from wikipedia]" . 
ies:DomainName rdfs:subClassOf ies:CommunicationsIdentifierRange . 
ies:DrivingLicence rdf:type rdfs:Class . 
ies:DrivingLicence sparx:guid "{44C1DD59-354B-405a-9755-417240802DE4}" . 
ies:DrivingLicence rdfs:comment "An IdentityDocument that permits a Person to drive a Vehicle in the Country of issue. " . 
ies:DrivingLicence rdfs:subClassOf ies:IdentityDocument . 
ies:Duration rdf:type rdfs:Class . 
ies:Duration sparx:guid "{7852A5E5-8684-49f2-82AE-3368032163B1}" . 
ies:Duration rdfs:comment "The Measure of an Elements temporal extent" . 
ies:Duration rdfs:subClassOf ies:StandardMeasure . 
ies:Easting rdf:type rdfs:Class . 
ies:Easting sparx:guid "{A4502460-54B7-446b-A9AA-003B49F9682B}" . 
ies:Easting rdfs:comment "The GeoIdentity that is a representation of the eastward componrnent of cartesian point on a map - i.e. on a 2D projection of the globe such as a mercator projection." . 
ies:Easting rdfs:subClassOf ies:GeoIdentity . 
ies:EducationalOrganisation rdf:type rdfs:Class . 
ies:EducationalOrganisation sparx:guid "{F30D350C-848D-4b02-AEA5-86575CEEEFB3}" . 
ies:EducationalOrganisation rdfs:comment "An Organisation that provides education" . 
ies:EducationalOrganisation rdfs:subClassOf ies:Organisation . 
ies:Election rdf:type rdfs:Class . 
ies:Election sparx:guid "{7D9E328D-345E-43f5-8163-9657E4D016BD}" . 
ies:Election rdfs:comment "A PoliticalEvent where the population vote for their preferred ElectoralCandidate to become their representative. " . 
ies:Election rdfs:subClassOf ies:PoliticalEvent . 
ies:ElectoralCandidate rdf:type rdfs:Class . 
ies:ElectoralCandidate sparx:guid "{E035D766-CB68-49c3-AC69-A56F3487C625}" . 
ies:ElectoralCandidate rdfs:comment "A Person standing for elected office" . 
ies:ElectoralCandidate rdfs:subClassOf ies:EventParticipant . 
ies:ElectoralRegion rdf:type rdfs:Class . 
ies:ElectoralRegion sparx:guid "{515468C2-B4D9-449d-8AC4-575973EFBF6B}" . 
ies:ElectoralRegion rdfs:comment "The RegionalConstituency being decided in an Election" . 
ies:ElectoralRegion rdfs:subClassOf ies:EventParticipant . 
ies:ElectricCurrent rdf:type rdfs:Class . 
ies:ElectricCurrent sparx:guid "{9442C4E6-A52B-4c93-B942-8B93D90B3B14}" . 
ies:ElectricCurrent rdfs:comment "The Measure of the flow of electric chargeNote: whilst this is a tricky Measure in a 4D ontology, it should be used in a niaive manner - i.e. a measure of a State of an Entity when the current is flowing through it." . 
ies:ElectricCurrent rdfs:subClassOf ies:StandardMeasure . 
ies:Element rdf:type rdfs:Class . 
ies:Element sparx:guid "{97EDC90F-3B36-4da8-AE77-D5FDBDEA2B21}" . 
ies:Element rdfs:comment "An ExchangedItem that has a spatial extent and can have start and end dates" . 
ies:Element rdfs:subClassOf ies:ExchangedItem . 
ies:EmailAccount rdf:type rdfs:Class . 
ies:EmailAccount sparx:guid "{FCBB35B9-704B-46c1-8054-10B7DA7EB8F8}" . 
ies:EmailAccount rdfs:comment "A CommunicationsAccount that is used to administer the use of one or more e-mail addresses." . 
ies:EmailAccount rdfs:subClassOf ies:CommunicationsAccount . 
ies:EmailAccount rdfs:subClassOf ies:OnlineAccount . 
ies:EmailAddress rdf:type rdfs:Class . 
ies:EmailAddress sparx:guid "{36F61EDF-6E6E-4d8d-9E75-275A820F6D96}" . 
ies:EmailAddress rdfs:comment "A CommunicationsIdentifier that uniquely identifiers an email account.Format: local-part@domain" . 
ies:EmailAddress rdfs:subClassOf ies:CommunicationsIdentifier . 
ies:employedBy rdf:type owl:ObjectProperty . 
ies:employedBy sparx:guid "{74721DF1-18D6-4c1b-93CC-71C888C6D405}" . 
ies:employedBy rdfs:comment "A worksFor relationship where the worker is employed." . 
ies:employedBy rdfs:subPropertyOf ies:worksFor . 
ies:employedBy rdfs:domain ies:PersonState . 
ies:endBoundOfClass rdf:type owl:ObjectProperty . 
ies:endBoundOfClass sparx:guid "{F8109922-1CB1-490d-BBB5-FD5B76E19FD1}" . 
ies:endBoundOfClass rdfs:comment "A relationship linking a TimeBoundedClass to the ParticularPeriod that marks the end bound date of its instances" . 
ies:endBoundOfClass rdfs:subPropertyOf ies:relationship . 
ies:endBoundOfClass rdfs:domain ies:TimeBoundedClass . 
ies:endBoundOfClass rdfs:range ies:ParticularPeriod . 
ies:endsIn rdf:type owl:DatatypeProperty . 
ies:endsIn sparx:guid "{6767DFCD-3FCB-42cc-BEE3-9FA9A324DF0B}" . 
ies:endsIn rdfs:comment "An xsd:DateTime for the end of the period" . 
ies:endsIn rdfs:subPropertyOf ies:attribute . 
ies:endsIn rdfs:domain ies:ArbitraryPeriod . 
ies:EndToEndActivity rdf:type rdfs:Class . 
ies:EndToEndActivity sparx:guid "{A88ABE99-1D6C-4843-A2E4-7531626D3859}" . 
ies:EndToEndActivity rdfs:comment "An Event (usually of long duration) that is composed of a number of other Events." . 
ies:EndToEndActivity rdfs:subClassOf ies:Event . 
ies:EndToEndAgreement rdf:type rdfs:Class . 
ies:EndToEndAgreement sparx:guid "{1B39630B-B00F-4def-9C65-48082C4AD2E0}" . 
ies:EndToEndAgreement rdfs:comment "An EndToEndActivity which is the overall process of agreeing something, including all the events that take place under that agreement, such as the negotiation, signing, delivery of service, etc." . 
ies:EndToEndAgreement rdfs:subClassOf ies:EndToEndActivity . 
ies:EndToEndAuthorisation rdf:type rdfs:Class . 
ies:EndToEndAuthorisation sparx:guid "{D75F18D1-95D6-481b-84D5-F8D7F3A5A389}" . 
ies:EndToEndAuthorisation rdfs:comment "An EndToEndActivity which is the overall process of requesting, receiving authority to act, and the conduct of activities under that authorisation until the period of authorisation ends. " . 
ies:EndToEndAuthorisation rdfs:subClassOf ies:EndToEndActivity . 
ies:EndToEndTransaction rdf:type rdfs:Class . 
ies:EndToEndTransaction sparx:guid "{911EB3DE-A001-493d-850D-3CF5A848791D}" . 
ies:EndToEndTransaction rdfs:comment "An EndToEndActivity covering the lifecycle of the trade" . 
ies:EndToEndTransaction rdfs:subClassOf ies:IntelligenceOperation . 
ies:EndToEndTransaction rdfs:subClassOf ies:EndToEndActivity . 
ies:enemyOf rdf:type owl:ObjectProperty . 
ies:enemyOf sparx:guid "{7F1A6A06-5223-4bf9-B903-1061A127D62C}" . 
ies:enemyOf rdfs:comment "A Relationship between two ResponsibleActor Entities where one is the enemy of the other.Note: this should not be considered a bi-directional relationship. Just because one person considers another person their enemy does not necessarily mean the feeling is reciprocated. " . 
ies:enemyOf rdfs:subPropertyOf ies:relationship . 
ies:enemyOf rdfs:domain ies:ResponsibleActorState . 
ies:enemyOf rdfs:range ies:ResponsibleActor . 
ies:EntertainmentEvent rdf:type rdfs:Class . 
ies:EntertainmentEvent sparx:guid "{78C33499-CD14-43cb-82AE-93A0F8CF022B}" . 
ies:EntertainmentEvent rdfs:comment "An Event where entertainment (sporting, music, theatre, etc.) is provided" . 
ies:EntertainmentEvent rdfs:subClassOf ies:Event . 
ies:EntertainmentTicket rdf:type rdfs:Class . 
ies:EntertainmentTicket sparx:guid "{96989C30-99CC-4606-A8D4-DFD9421F0E34}" . 
ies:EntertainmentTicket rdfs:comment "A Ticket to an EntertainmentEvent" . 
ies:EntertainmentTicket rdfs:subClassOf ies:Ticket . 
ies:Entity rdf:type rdfs:Class . 
ies:Entity sparx:guid "{F4EDE167-6F5A-417d-9984-0221CCDF752C}" . 
ies:Entity rdfs:comment "An Entity typically represents a tangible thing like a Person, a Communications Device, or a Location." . 
ies:Entity rdfs:subClassOf ies:Element . 
ies:Entity ies:powertype ies:ClassOfEntity . 
ies:EntityInTransit rdf:type rdfs:Class . 
ies:EntityInTransit sparx:guid "{74169219-A47C-48ce-A25F-3948E7E873B6}" . 
ies:EntityInTransit rdfs:comment "A TravelLeg where an Entity is moving in Transit" . 
ies:EntityInTransit rdfs:subClassOf ies:TravelLeg . 
ies:Ethnicity rdf:type rdfs:Class . 
ies:Ethnicity sparx:guid "{8AC946A4-4C03-463c-9F32-37EA8593988A}" . 
ies:Ethnicity rdfs:comment "A ClassOfPerson whose members all share the same ethnicity" . 
ies:Ethnicity rdfs:subClassOf ies:ClassOfPerson . 
ies:Event rdf:type rdfs:Class . 
ies:Event sparx:guid "{B376370E-F5E8-4287-A3EC-AC35532919B1}" . 
ies:Event rdfs:comment "An Event represents an activity or incident, involving one or more participating entities, that occurred/started at a specific point in time � e.g. a meeting, or a telephone call." . 
ies:Event rdfs:subClassOf ies:Element . 
ies:Event ies:powertype ies:ClassOfEvent . 
ies:eventDateTime rdf:type owl:ObjectProperty . 
ies:eventDateTime sparx:guid "{07DCD4FC-938C-438d-ABE6-F7F64E66A255}" . 
ies:eventDateTime rdfs:comment "The date/time of the performance to which the ticket is valid." . 
ies:eventDateTime rdfs:subPropertyOf ies:relationship . 
ies:eventDateTime rdfs:domain ies:EntertainmentTicket . 
ies:eventDateTime rdfs:range ies:ParticularPeriod . 
ies:EventParticipant rdf:type rdfs:Class . 
ies:EventParticipant sparx:guid "{C5AB420C-1AB6-479a-97E1-4F2FD37725CB}" . 
ies:EventParticipant rdfs:comment "A State which is the participating role of an Entity in an Event.Note: this includes inactive participation (e.g. something that is being repaired). If the participation is known to be active then ActiveEventPartipant (or one of its subtypes) should be used. In BORO, EventParticipant would be Involvement and ActiveEventParticipant would be Participation." . 
ies:EventParticipant rdfs:subClassOf ies:State . 
ies:EventState rdf:type rdfs:Class . 
ies:EventState sparx:guid "{FE668C24-D25C-4273-872A-EB77CB09341D}" . 
ies:EventState rdfs:comment "A temporal state of an EventNote: care must be taken with using this in a 4D, extensional model such as IES. States such as Ended would not be appropriate, for example - in such a case, the temporal extent of the Event or the presence of a BoundingState to end it would be correct. " . 
ies:EventState rdfs:subClassOf ies:State . 
ies:EvidentialPhotograph rdf:type rdfs:Class . 
ies:EvidentialPhotograph sparx:guid "{AFFFF30F-B274-4466-B0F2-D2A6A78E1832}" . 
ies:EvidentialPhotograph rdfs:comment "Relates a Surveillance Event to a Document that is the evidence resulting from the Surveillance" . 
ies:EvidentialPhotograph rdfs:subClassOf ies:EventParticipant . 
ies:ExchangedItem rdf:type rdfs:Class . 
ies:ExchangedItem sparx:guid "{485CBF1A-04FF-4741-8471-46A03D28C406}" . 
ies:ExchangedItem rdfs:comment "An ExchangedItem is a real world �thing� about which a sender might retain specific knowledge, some or all of which is needed to be shared (exchanged) with one or more recipients." . 
ies:ExchangedItem rdfs:subClassOf rdfs:Resource . 
ies:ExchangedItem rdfs:label "Exchanged Item" .
ies:ExchangePayload rdf:type rdfs:Class . 
ies:ExchangePayload sparx:guid "{749B002E-37B1-4754-B3B2-96642B3CF4A7}" . 
ies:ExchangePayload rdfs:comment "A marker object that shall be present in all IES exchange files. This object is the domain for all meta-data about the file.Wherever possible, Dublin-Core meta-data tags should be used on an ExchangePayload. If locally defined properties are needed, then these may also be defined and included in the exchange file. " . 
ies:excludedFrom rdf:type owl:ObjectProperty . 
ies:excludedFrom sparx:guid "{883B5479-62DD-47a4-BC14-9A11835D820B}" . 
ies:excludedFrom rdfs:comment "A Relationship between a ResponsibleActorState and a Location they are not allowed to enter.Note: any additional information about how or why the exclusion is in place should be added to the state" . 
ies:excludedFrom rdfs:subPropertyOf ies:relationship . 
ies:excludedFrom rdfs:domain ies:ResponsibleActorState . 
ies:excludedFrom rdfs:range ies:Location . 
ies:Facility rdf:type rdfs:Class . 
ies:Facility sparx:guid "{9CD2C1B1-85B1-4579-9376-07827AD68461}" . 
ies:Facility rdfs:comment "A Location that is man-made, but is typically larger than an Address (i.e. it may have more than one postal address)Examples:Military camps, factories, sports facilities, airports, etc." . 
ies:Facility rdfs:subClassOf ies:RealEstate . 
ies:familiallyRelatedTo rdf:type owl:ObjectProperty . 
ies:familiallyRelatedTo sparx:guid "{3AA26AC6-206D-4b6d-BDEC-C9E2B4814BE7}" . 
ies:familiallyRelatedTo rdfs:comment "A Relationship between PersonState (which may be a Person, or just a temporal state of Person) and another Person to indicate they have a familial relationship.Note:  some relationships will be temporal (e.g. spouseOf) and therefore related a state to a Person. Others will be for life (i.e. from the birth of the youngest until one of them dies) and therefore between two whole-life Person entities." . 
ies:familiallyRelatedTo rdfs:subPropertyOf ies:relationship . 
ies:familiallyRelatedTo rdfs:domain ies:PersonState . 
ies:familiallyRelatedTo rdfs:range ies:Person . 
ies:fearfulOf rdf:type owl:ObjectProperty . 
ies:fearfulOf sparx:guid "{A589F81D-DC15-4b71-80B5-BA4CD46B2E41}" . 
ies:fearfulOf rdfs:comment "A Relationship between two ResponsibleActor Entities where one is fearful of the other.Note: this should not be considered a bi-directional relationship. Just because one person considers another person a threat does not necessarily mean the feeling is reciprocated. " . 
ies:fearfulOf rdfs:subPropertyOf ies:relationship . 
ies:fearfulOf rdfs:range ies:ResponsibleActor . 
ies:fearfulOf rdfs:domain ies:ResponsibleActorState . 
ies:FerryTicket rdf:type rdfs:Class . 
ies:FerryTicket sparx:guid "{B2ED961F-245E-4e74-A32F-6B9CF1BBDF2B}" . 
ies:FerryTicket rdfs:comment "A Ticket that is used to travel by sea" . 
ies:FerryTicket rdfs:subClassOf ies:TravelTicket . 
ies:FinancialAccount rdf:type rdfs:Class . 
ies:FinancialAccount sparx:guid "{44DAC574-2A2E-44bc-ACD2-236811FA8D29}" . 
ies:FinancialAccount rdfs:comment "An Account held for financial management purposes." . 
ies:FinancialAccount rdfs:subClassOf ies:Account . 
ies:financialAccountType rdf:type owl:ObjectProperty . 
ies:financialAccountType sparx:guid "{94BC4F7F-3DC3-4e26-8E2B-26E7D9B1A760}" . 
ies:financialAccountType rdfs:comment "Relates a FinancialAccount to its type. Note, that a given FinancialAccount may have more than one ClassOfFinancialAccount - e.g. a Business Account that is also a Current Account" . 
ies:financialAccountType rdfs:subPropertyOf ies:relationship . 
ies:financialAccountType rdfs:subPropertyOf rdf:type . 
ies:financialAccountType rdfs:range ies:ClassOfFinancialAccount . 
ies:financialAccountType rdfs:domain ies:FinancialAccount . 
ies:FirstLineOfAddress rdf:type rdfs:Class . 
ies:FirstLineOfAddress sparx:guid "{8B6DD87E-3D76-4836-9201-1244B80CDC69}" . 
ies:FirstLineOfAddress rdfs:comment "The first line of the Address including the number of the dwelling and the street name." . 
ies:FirstLineOfAddress rdfs:subClassOf ies:LineOfAddress . 
ies:Flight rdf:type rdfs:Class . 
ies:Flight sparx:guid "{375B0887-712F-43f0-BBF4-5C544D75AC39}" . 
ies:Flight rdfs:comment "A TravelService by air" . 
ies:Flight rdfs:subClassOf ies:Transit . 
ies:FlightTicket rdf:type rdfs:Class . 
ies:FlightTicket sparx:guid "{3A9A1BA9-465F-4f6d-BD55-9F3F8AE40AE0}" . 
ies:FlightTicket rdfs:comment "A Ticket that is used to travel by air" . 
ies:FlightTicket rdfs:subClassOf ies:TravelTicket . 
ies:FootballMatchTicket rdf:type rdfs:Class . 
ies:FootballMatchTicket sparx:guid "{DA626F73-5748-47db-813F-E1813577F41B}" . 
ies:FootballMatchTicket rdfs:comment "An EntertainmentTicket for a football match" . 
ies:FootballMatchTicket rdfs:subClassOf ies:EntertainmentTicket . 
ies:Forgery rdf:type rdfs:Class . 
ies:Forgery sparx:guid "{78686D99-2AAC-4f5b-8EE0-456BDCC6F99E}" . 
ies:Forgery rdfs:comment "A CriminalActivity that is the creation of fake items(also a subclass of Create). " . 
ies:Forgery rdfs:subClassOf ies:Create . 
ies:Forgery rdfs:subClassOf ies:CriminalActivity . 
ies:format rdf:type owl:ObjectProperty . 
ies:format sparx:guid "{EF2C13D4-7106-4799-BB72-7CD47714F257}" . 
ies:format rdfs:comment "The format of the respective WorkOfDocumentation.Examples:PDFMS Word" . 
ies:format rdfs:subPropertyOf ies:relationship . 
ies:format rdfs:subPropertyOf rdfs:subClassOf . 
ies:format rdfs:domain ies:WorkOfDocumentation . 
ies:format rdfs:range ies:DocumentFormat . 
ies:formatOfIndividualDocument rdf:type owl:ObjectProperty . 
ies:formatOfIndividualDocument sparx:guid "{F1F94713-6D95-4928-B537-4FBA55D09E34}" . 
ies:formatOfIndividualDocument rdfs:comment "The format of the respective IndividualDocument.Examples:PDFPrinted" . 
ies:formatOfIndividualDocument rdfs:subPropertyOf ies:relationship . 
ies:formatOfIndividualDocument rdfs:domain ies:IndividualDocument . 
ies:formatOfIndividualDocument rdfs:subPropertyOf rdf:type . 
ies:formatOfIndividualDocument rdfs:range ies:DocumentFormat . 
ies:FoundOrganisation rdf:type rdfs:Class . 
ies:FoundOrganisation sparx:guid "{5054AFA3-8FC7-449d-93EE-C69B9D2AE118}" . 
ies:FoundOrganisation rdfs:comment "A Create Event where an Organisation is founded" . 
ies:FoundOrganisation rdfs:subClassOf ies:Create . 
ies:friendOf rdf:type owl:ObjectProperty . 
ies:friendOf sparx:guid "{13EB3439-497F-49ad-A7F4-DEF8A600F640}" . 
ies:friendOf rdfs:comment "A Relationship between two ResponsibleActor Entities where one is the friend of the other.Note: this should not be considered a bi-directional relationship. Just because one person considers another person their friend does not necessarily mean the feeling is reciprocated. Not that Im bitter or anything. See also Stalking if you must. " . 
ies:friendOf rdfs:subPropertyOf ies:relationship . 
ies:friendOf rdfs:range ies:ResponsibleActor . 
ies:friendOf rdfs:domain ies:ResponsibleActorState . 
ies:Gender rdf:type rdfs:Class . 
ies:Gender sparx:guid "{8B4DB18E-DF46-4419-B0ED-0159A25F2319}" . 
ies:Gender rdfs:comment "A ClassOfPerson whose members all share the same gender" . 
ies:Gender rdfs:subClassOf ies:ClassOfPerson . 
ies:GeographicFeature rdf:type rdfs:Class . 
ies:GeographicFeature sparx:guid "{7EEE1EF7-C814-4eee-85B3-F48698FD52B6}" . 
ies:GeographicFeature rdfs:comment "A Location that is a naturally occurring feature on the earth." . 
ies:GeographicFeature rdfs:subClassOf ies:Location . 
ies:GeoIdentity rdf:type rdfs:Class . 
ies:GeoIdentity sparx:guid "{87251DA1-7293-445e-987F-F13E331B6BDF}" . 
ies:GeoIdentity rdfs:comment "A unique Identifier attributed to the respective Location" . 
ies:GeoIdentity rdfs:subClassOf ies:Identifier . 
ies:GeoJSON rdf:type rdfs:Class . 
ies:GeoJSON sparx:guid "{417C1F4E-6A5D-4631-B275-8E982252791A}" . 
ies:GeoJSON rdfs:comment "GeoJSON is an open standard format designed for representing simple geographical features, along with their non-spatial attributes. It is based on JSON, the JavaScript Object Notation.GeoJSON mandates use of WGS 84 coordinate system - see IETF RFC 7946" . 
ies:GeoJSON rdfs:subClassOf ies:GeoRepresentation . 
ies:GeoObject rdf:type rdfs:Class . 
ies:GeoObject sparx:guid "{EA165884-8DF6-4aa6-848C-C682F6969D9F}" . 
ies:GeoObject rdfs:comment "A DataObject and a GeoRepresentation that contains geographical information" . 
ies:GeoObject rdfs:subClassOf ies:DataObject . 
ies:GeoObject rdfs:subClassOf ies:GeoRepresentation . 
ies:GeoPoint rdf:type rdfs:Class . 
ies:GeoPoint sparx:guid "{9A9467C3-D5FC-4964-8943-FE63ADF38914}" . 
ies:GeoPoint rdfs:comment "A Location that is a point (mathematically speaking, of vanishing volume) on, below or above the surface of the WGS84 spheroid. The distance from the spheroid surface is given by the altitudeInMetres attribute." . 
ies:GeoPoint rdfs:subClassOf ies:Location . 
ies:GeoRepresentation rdf:type rdfs:Class . 
ies:GeoRepresentation sparx:guid "{A8C07233-5D62-4ad4-B405-2D15CFC37497}" . 
ies:GeoRepresentation rdfs:comment "A Representation for a Location - e.g. a point, a polyline, etc." . 
ies:GeoRepresentation rdfs:subClassOf ies:Representation . 
ies:GivenName rdf:type rdfs:Class . 
ies:GivenName sparx:guid "{A01A5045-B09C-4bea-8C96-881C29F2EE60}" . 
ies:GivenName rdfs:comment "A PersonName that is one of the given names of a PersonNote:A GivenName will often be applied to a State of the Person, as names tend to change over time" . 
ies:GivenName rdfs:subClassOf ies:PersonName . 
ies:GML rdf:type rdfs:Class . 
ies:GML sparx:guid "{AE59CB88-3178-4bad-9F43-1276337C7944}" . 
ies:GML rdfs:comment "The Geography-Markup-Language (GML) is the XML grammar defined by the Open Geospatial Consortium (OGC) to express geographical features. GML serves as a modeling language for geographic systems as well as an open interchange format for geographic transactions on the Internet. Key to GMLs utility is its ability to integrate all forms of geographic information, including not only conventional vector or discrete objects, but coverages (see also GMLJP2) and sensor data." . 
ies:GML rdfs:subClassOf ies:GeoRepresentation . 
ies:governedPopulation rdf:type owl:ObjectProperty . 
ies:governedPopulation sparx:guid "{917C549C-259F-4850-9CFD-35E05485BF63}" . 
ies:governedPopulation rdfs:comment "Relates a Government to the RegionalPopulation that it governs. " . 
ies:governedPopulation rdfs:subPropertyOf ies:relationship . 
ies:governedPopulation rdfs:domain ies:Government . 
ies:governedPopulation rdfs:range ies:RegionalConstituency . 
ies:governedRegion rdf:type owl:ObjectProperty . 
ies:governedRegion sparx:guid "{72DC3E90-53CE-434d-A5F3-89BDCE08A201}" . 
ies:governedRegion rdfs:comment "The Location which the respective Government is in charge of.See also goverenedPopulation - sometimes Locations have no people, and sometimes people reside outside the region in which they are legally citizens.Note: A Government instance has a start and end date corresponding to its time in power. " . 
ies:governedRegion rdfs:subPropertyOf ies:relationship . 
ies:governedRegion rdfs:domain ies:Government . 
ies:governedRegion rdfs:range ies:Location . 
ies:Government rdf:type rdfs:Class . 
ies:Government sparx:guid "{D62DDBB8-53FC-405a-BC43-89CA337563A0}" . 
ies:Government rdfs:comment "An Organisation that is (usually) elected to run a governedRegion" . 
ies:Government rdfs:subClassOf ies:Organisation . 
ies:GovernmentOrganisation rdf:type rdfs:Class . 
ies:GovernmentOrganisation sparx:guid "{0D042066-06C8-48d6-8387-500CF8EE2592}" . 
ies:GovernmentOrganisation rdfs:comment "An Organisation that is part of, or controlled by a national or local Government" . 
ies:GovernmentOrganisation rdfs:subClassOf ies:Organisation . 
ies:grantedActivityType rdf:type owl:ObjectProperty . 
ies:grantedActivityType sparx:guid "{289608A2-3F9D-413a-98AB-25579C370924}" . 
ies:grantedActivityType rdfs:comment "A relationship linking an GrantOfAuthority to a AuthorisedEventClass that the authorisation grants.For example,  granting authorisation to travel" . 
ies:grantedActivityType rdfs:subPropertyOf ies:relationship . 
ies:grantedActivityType rdfs:domain ies:GrantOfAuthority . 
ies:grantedActivityType rdfs:range ies:AuthorisedEventClass . 
ies:GrantOfAuthority rdf:type rdfs:Class . 
ies:GrantOfAuthority sparx:guid "{F5EAAEEE-C0B2-469f-9048-3E0731ED8342}" . 
ies:GrantOfAuthority rdfs:comment "An AuthorisationStage where a ResponsibleActor grants another ResponsibleActor authority to act." . 
ies:GrantOfAuthority rdfs:subClassOf ies:AuthorisationStage . 
ies:groupDescription rdf:type owl:DatatypeProperty . 
ies:groupDescription sparx:guid "{2F618A01-5D5F-483c-8652-8B81196AA086}" . 
ies:groupDescription rdfs:comment "A simple text description of a GroupOfItems" . 
ies:groupDescription rdfs:domain ies:GroupOfItems . 
ies:groupName rdf:type owl:DatatypeProperty . 
ies:groupName sparx:guid "{42463865-450C-4a9a-9EF0-5322222C2B97}" . 
ies:groupName rdfs:comment "A name given to a GroupOfItems" . 
ies:groupName rdfs:domain ies:GroupOfItems . 
ies:GroupOfItems rdf:type rdfs:Class . 
ies:GroupOfItems sparx:guid "{04C2111A-D958-4a95-9271-7208B849DDD8}" . 
ies:GroupOfItems rdfs:comment "A collection of ExchangedItem that have been gathered together for a purpose. Note: The same ExchangedItem can be in more than one GroupOfItems" . 
ies:GroupOfItems rdfs:subClassOf rdfs:Resource . 
ies:Hacking rdf:type rdfs:Class . 
ies:Hacking sparx:guid "{2AC7FDAB-7BB8-41ee-B558-AEBFE01274F2}" . 
ies:Hacking rdfs:comment "A CriminalActivity where computer equipment is interfered with without the owners permission" . 
ies:Hacking rdfs:subClassOf ies:CriminalActivity . 
ies:handlingCaveat rdf:type owl:DatatypeProperty . 
ies:handlingCaveat sparx:guid "{1C02B06E-3159-48f6-9575-64B62765498B}" . 
ies:handlingCaveat rdfs:comment "A textual description of any handling caveats that must be adhered to." . 
ies:handlingCaveat rdfs:domain ies:SecurityLabel . 
ies:happensIn rdf:type owl:ObjectProperty . 
ies:happensIn sparx:guid "{60A37745-8DD5-4e4c-9A4C-6957F71AD971}" . 
ies:happensIn rdfs:comment "A partOf relationship to indicate an Event takes place within a Location" . 
ies:happensIn rdfs:subPropertyOf ies:inLocation . 
ies:happensIn rdfs:domain ies:Event . 
ies:happensIn rdfs:range ies:Location . 
ies:hasAccessTo rdf:type owl:ObjectProperty . 
ies:hasAccessTo sparx:guid "{CB7F872F-7999-4bfd-8274-2C0E0AFE22AB}" . 
ies:hasAccessTo rdfs:comment "A Relationship between a ResponsibleActorState and an Entity they have access to - e.g. a FinancialAccount, CommunicationsDevice, etc." . 
ies:hasAccessTo rdfs:subPropertyOf ies:relationship . 
ies:hasAccessTo rdfs:domain ies:ResponsibleActorState . 
ies:hasAccessTo rdfs:range ies:Entity . 
ies:hasAuthor rdf:type owl:ObjectProperty . 
ies:hasAuthor sparx:guid "{9464D864-E76F-4e09-89E1-D3B2D3E63F3B}" . 
ies:hasAuthor rdfs:comment "The author of the respective document." . 
ies:hasAuthor rdfs:subPropertyOf ies:relationship . 
ies:hasAuthor rdfs:domain ies:WorkOfDocumentation . 
ies:hasAuthor rdfs:range ies:ResponsibleActor . 
ies:hasCharacteristic rdf:type owl:ObjectProperty . 
ies:hasCharacteristic sparx:guid "{720D0AA3-81F7-4220-A7A5-34304E33B72F}" . 
ies:hasCharacteristic rdfs:comment "An rdf:type relationship that asserts an Element has a Characteristic or Measure" . 
ies:hasCharacteristic rdfs:subPropertyOf rdf:type . 
ies:hasCharacteristic rdfs:subPropertyOf ies:relationship . 
ies:hasCharacteristic rdfs:domain ies:Element . 
ies:hasCharacteristic rdfs:range ies:Characteristic . 
ies:hasCountryOfIssue rdf:type owl:ObjectProperty . 
ies:hasCountryOfIssue sparx:guid "{E7500475-8C4F-47a3-8AAB-C5679621FAE8}" . 
ies:hasCountryOfIssue rdfs:comment "The country in which the respective IdentityDocument or PaymentArtefact was issued." . 
ies:hasCountryOfIssue rdfs:subPropertyOf ies:relationship . 
ies:hasCountryOfIssue rdfs:domain ies:IdentityDocument . 
ies:hasCountryOfIssue rdfs:range ies:Country . 
ies:hasCountryOfIssue rdfs:domain ies:TravelCard . 
ies:hasEmergencyContactAddress rdf:type owl:ObjectProperty . 
ies:hasEmergencyContactAddress sparx:guid "{0AAF6757-AAC9-43c4-8B43-CB3358EADCA4}" . 
ies:hasEmergencyContactAddress rdfs:comment "The address of an emergency contact as printed on the IdentityDocument" . 
ies:hasEmergencyContactAddress rdfs:subPropertyOf ies:relationship . 
ies:hasEmergencyContactAddress rdfs:domain ies:IdentityDocument . 
ies:hasEmergencyContactAddress rdfs:range ies:Address . 
ies:hasEthnicity rdf:type owl:ObjectProperty . 
ies:hasEthnicity sparx:guid "{BC3185CE-53F4-45de-A6D4-DAC8343B4D1C}" . 
ies:hasEthnicity rdfs:comment "The ethnic group that the respective Person belongs to.The Metropolitan Police standard shall be used as the reference data standard." . 
ies:hasEthnicity rdfs:domain ies:Person . 
ies:hasEthnicity rdfs:subPropertyOf ies:relationship . 
ies:hasEthnicity rdfs:range ies:Ethnicity . 
ies:hasEthnicity rdfs:subPropertyOf rdf:type . 
ies:hasGeneticGender rdf:type owl:ObjectProperty . 
ies:hasGeneticGender sparx:guid "{8914E7DF-443B-4a3a-A945-AAD11B82A86A}" . 
ies:hasGeneticGender rdfs:comment "The gender the Person was born with (sex) and which would result from a DNA test." . 
ies:hasGeneticGender rdfs:subPropertyOf ies:relationship . 
ies:hasGeneticGender rdfs:domain ies:Person . 
ies:hasGeneticGender rdfs:range ies:Gender . 
ies:hasGeneticGender rdfs:subPropertyOf rdf:type . 
ies:hasIdentifiedGender rdf:type owl:ObjectProperty . 
ies:hasIdentifiedGender sparx:guid "{7640DBFC-B520-458c-A7C1-16651DDF217F}" . 
ies:hasIdentifiedGender rdfs:comment "The gender the Person chooses to identify as" . 
ies:hasIdentifiedGender rdfs:subPropertyOf ies:relationship . 
ies:hasIdentifiedGender rdfs:domain ies:PersonState . 
ies:hasIdentifiedGender rdfs:range ies:Gender . 
ies:hasLanguageProficiency rdf:type owl:ObjectProperty . 
ies:hasLanguageProficiency sparx:guid "{2065B9A0-DCAD-45be-9F0D-BD4398261A7F}" . 
ies:hasLanguageProficiency rdfs:comment "A language spoken by the respective Person at a stage (PersonState) in their life" . 
ies:hasLanguageProficiency rdfs:subPropertyOf ies:relationship . 
ies:hasLanguageProficiency rdfs:domain ies:PersonState . 
ies:hasLanguageProficiency rdfs:range ies:LanguageProficiency . 
ies:hasLanguageProficiency rdfs:subPropertyOf rdf:type . 
ies:hasName rdf:type owl:ObjectProperty . 
ies:hasName sparx:guid "{C3A36E36-0C73-4af7-88E3-81C9243CE456}" . 
ies:hasName rdfs:comment "An isRepresentedAs relationship that asserts an ExchangedItem is identified (albeit loosely) by a Name" . 
ies:hasName rdfs:subPropertyOf ies:isRepresentedAs . 
ies:hasName rdfs:domain ies:ExchangedItem . 
ies:hasName rdfs:range ies:Name . 
ies:hasPublisher rdf:type owl:ObjectProperty . 
ies:hasPublisher sparx:guid "{07FD1DF6-BA77-4657-B3D3-D6D579FD4608}" . 
ies:hasPublisher rdfs:comment "The publisher of the document." . 
ies:hasPublisher rdfs:subPropertyOf ies:relationship . 
ies:hasPublisher rdfs:domain ies:WorkOfDocumentation . 
ies:hasPublisher rdfs:range ies:ResponsibleActor . 
ies:hasRegisteredCommsID rdf:type owl:ObjectProperty . 
ies:hasRegisteredCommsID sparx:guid "{E076AFB8-F6F8-4b06-82B3-7ED568D1EE73}" . 
ies:hasRegisteredCommsID rdfs:comment "A relationship between a CommunicationsIdentifier and the CommunicationsAccountState of the account to which the identifier is registered" . 
ies:hasRegisteredCommsID rdfs:subPropertyOf ies:relationship . 
ies:hasRegisteredCommsID rdfs:domain ies:CommunicationsAccountState . 
ies:hasRegisteredCommsID rdfs:range ies:CommunicationsIdentifier . 
ies:hasReligion rdf:type owl:ObjectProperty . 
ies:hasReligion sparx:guid "{6D1839A4-342A-4e34-823C-BDB392483048}" . 
ies:hasReligion rdfs:comment "A relationship where a PersonState holds or follows a Religion" . 
ies:hasReligion rdfs:subPropertyOf ies:relationship . 
ies:hasReligion rdfs:domain ies:PersonState . 
ies:hasReligion rdfs:range ies:Religion . 
ies:hasRole rdf:type owl:ObjectProperty . 
ies:hasRole sparx:guid "{5C76592F-C47D-40ee-8D82-497962686D34}" . 
ies:hasRole rdfs:comment "An rdf:type relationship that asserts a State has a RoleExample - Freds time in Acme as a manager" . 
ies:hasRole rdfs:subPropertyOf rdf:type . 
ies:hasRole rdfs:range ies:Role . 
ies:hasRole rdfs:domain ies:State . 
ies:hasSourceReference rdf:type owl:ObjectProperty . 
ies:hasSourceReference sparx:guid "{16480E86-9FE4-4b37-ACFB-9E410F190664}" . 
ies:hasSourceReference rdfs:comment "A isRepresentedAs relationship that asserts a Representation is the source (information provenance) for an ExchangedItem" . 
ies:hasSourceReference rdfs:subPropertyOf ies:isRepresentedAs . 
ies:hasStatedAddress rdf:type owl:ObjectProperty . 
ies:hasStatedAddress sparx:guid "{0451B5D4-99CB-47a7-BB93-DF4DF6625837}" . 
ies:hasStatedAddress rdfs:comment "The address of the owner/user as recorded on the respective IdentityDocument or PaymentArtefact." . 
ies:hasStatedAddress rdfs:subPropertyOf ies:relationship . 
ies:hasStatedAddress rdfs:domain ies:IdentityDocument . 
ies:hasStatedAddress rdfs:range ies:Address . 
ies:hasStatedAddress rdfs:domain ies:TravelCard . 
ies:hasStatedCountryOfResidence rdf:type owl:ObjectProperty . 
ies:hasStatedCountryOfResidence sparx:guid "{9A4EB722-0BDA-4ba7-B895-7A4E273865C9}" . 
ies:hasStatedCountryOfResidence rdfs:comment "The country of residence as printed on the respective IdentityDocument " . 
ies:hasStatedCountryOfResidence rdfs:subPropertyOf ies:relationship . 
ies:hasStatedCountryOfResidence rdfs:range ies:Country . 
ies:hasStatedCountryOfResidence rdfs:domain ies:IdentityDocument . 
ies:hasStatedNationality rdf:type owl:ObjectProperty . 
ies:hasStatedNationality sparx:guid "{C8AB9A91-97ED-4868-8167-44E71F40AFE7}" . 
ies:hasStatedNationality rdfs:comment "The nationality of the identity holder as specified on the IdentityDocument." . 
ies:hasStatedNationality rdfs:subPropertyOf ies:relationship . 
ies:hasStatedNationality rdfs:domain ies:IdentityDocument . 
ies:hasStatedNationality rdfs:range ies:Nation . 
ies:hasStatedPlaceOfBirth rdf:type owl:ObjectProperty . 
ies:hasStatedPlaceOfBirth sparx:guid "{F95710A9-B0A7-4f7b-ADAA-08A2DCBD9C35}" . 
ies:hasStatedPlaceOfBirth rdfs:comment "A relationship to the place of birth as recorded on the respective IdentityDocument" . 
ies:hasStatedPlaceOfBirth rdfs:subPropertyOf ies:relationship . 
ies:hasStatedPlaceOfBirth rdfs:domain ies:IdentityDocument . 
ies:hasStatedPlaceOfBirth rdfs:range ies:RegionOfCountry . 
ies:hasStatedPlaceOfIssue rdf:type owl:ObjectProperty . 
ies:hasStatedPlaceOfIssue sparx:guid "{644B75E8-92A0-4f16-861E-3B4FDFDF572E}" . 
ies:hasStatedPlaceOfIssue rdfs:comment "A relationship to the place of issue as specified on the IdentityDocument" . 
ies:hasStatedPlaceOfIssue rdfs:subPropertyOf ies:relationship . 
ies:hasStatedPlaceOfIssue rdfs:domain ies:IdentityDocument . 
ies:hasStatedPlaceOfIssue rdfs:range ies:RegionOfCountry . 
ies:hasTheme rdf:type owl:ObjectProperty . 
ies:hasTheme sparx:guid "{654CB83B-75CF-4940-A2CF-C7820141C5AE}" . 
ies:hasTheme rdfs:comment "A relationship linking an Event (e.g. Communication, Meeting or Investigation) to an ExchangedItem that is a theme (or topic)Examples:* A Event being investigated after it occurred* A general investigation into a Location* A Meeting discussing a new project* A VoiceCall about a Vehicle" . 
ies:hasTheme rdfs:subPropertyOf ies:relationship . 
ies:hasTheme rdfs:domain ies:Investigation . 
ies:hasTheme rdfs:range ies:ExchangedItem . 
ies:hasTheme rdfs:domain ies:Meeting . 
ies:hasTheme rdfs:domain ies:Communication . 
ies:hasValue rdf:type owl:ObjectProperty . 
ies:hasValue sparx:guid "{8FD84185-A7CE-4d5d-974B-55F693C4376D}" . 
ies:hasValue rdfs:comment "An isRepresentedAs relationship that asserts a Measure has a MeasureValueNote: a given Measure may have more than one value (e.g. 1kg or 2.2lbs) in different units of measure" . 
ies:hasValue rdfs:subPropertyOf ies:isRepresentedAs . 
ies:hasValue rdfs:domain ies:Measure . 
ies:hasValue rdfs:range ies:MeasureValue . 
ies:Hates rdf:type rdfs:Class . 
ies:Hates sparx:guid "{6939AE2F-D74D-4446-8A88-5C26669689BA}" . 
ies:Hates rdfs:comment "An Interested state where a ResponsibleActor hates something" . 
ies:Hates rdfs:subClassOf ies:Interested . 
ies:HealthServiceIdentifier rdf:type rdfs:Class . 
ies:HealthServiceIdentifier sparx:guid "{FBCCD717-E163-4129-B270-966F5D404260}" . 
ies:HealthServiceIdentifier rdfs:comment "A NationalIdentityNumber used for managing a citizens through-life healthcareIn UK, this would be an NHS number, apart from Scotland where it is called a CHI number" . 
ies:HealthServiceIdentifier rdfs:subClassOf ies:NationalIdentityNumber . 
ies:hmlConfidence rdf:type owl:DatatypeProperty . 
ies:hmlConfidence sparx:guid "{04F797E7-9B5C-48c5-A50D-A14CFF7725DE}" . 
ies:hmlConfidence rdfs:comment "A confidence whose value must be one of HIGH, MEDIUM, or LOWThis is a mandatory attribute for AssessToBeTrue" . 
ies:hmlConfidence rdfs:subPropertyOf ies:confidence . 
ies:hmlConfidence rdfs:domain ies:AssessToBeTrue . 
ies:holdsAccount rdf:type owl:ObjectProperty . 
ies:holdsAccount sparx:guid "{6314A9B0-4578-42a8-A553-1FDDF35AC7F1}" . 
ies:holdsAccount rdfs:comment "Relates an AccountHolder (PersonState) to the Account they hold" . 
ies:holdsAccount rdfs:subPropertyOf ies:relationship . 
ies:holdsAccount rdfs:domain ies:AccountHolder . 
ies:holdsAccount rdfs:range ies:Account . 
ies:hostedOn rdf:type owl:ObjectProperty . 
ies:hostedOn sparx:guid "{F5C27E55-623E-4fa7-95C3-DD0A722D1035}" . 
ies:hostedOn rdfs:comment "Relates a WebResourceState to the OnlineService that hosts it" . 
ies:hostedOn rdfs:subPropertyOf ies:relationship . 
ies:hostedOn rdfs:domain ies:WebResourceState . 
ies:hostedOn rdfs:range ies:OnlineService . 
ies:IATACode rdf:type rdfs:Class . 
ies:IATACode sparx:guid "{AA530BCE-02F2-4195-A431-573D13A5B41C}" . 
ies:IATACode rdfs:comment "A GeoIdentity that is administered by the International Air Transport Associate for airport identification" . 
ies:IATACode rdfs:subClassOf ies:GeoIdentity . 
ies:IBAN rdf:type rdfs:Class . 
ies:IBAN sparx:guid "{40E59970-04CE-4961-83FC-179739C4DEC3}" . 
ies:IBAN rdfs:comment "An Identifier that is an International Bank Account NumberSee ISO 13616:2007" . 
ies:IBAN rdfs:subClassOf ies:Identifier . 
ies:ICAOCode rdf:type rdfs:Class . 
ies:ICAOCode sparx:guid "{239A3A0C-183C-432f-9147-7259C9573AA2}" . 
ies:ICAOCode rdfs:comment "A GeoIdentity that is administered by the International Civil Aviation Organisation for identifying airports" . 
ies:ICAOCode rdfs:subClassOf ies:GeoIdentity . 
ies:idAuthenticity rdf:type owl:DatatypeProperty . 
ies:idAuthenticity sparx:guid "{1185F43F-7EBB-4e38-A1B3-FF1421F3416D}" . 
ies:idAuthenticity rdfs:comment "Provides an indication of the believed authenticity of the IdentityDocumentGenuineFakeUnknown" . 
ies:idAuthenticity rdfs:subPropertyOf ies:attribute . 
ies:idAuthenticity rdfs:domain ies:IdentityDocument . 
ies:idDateOfBirth rdf:type owl:ObjectProperty . 
ies:idDateOfBirth sparx:guid "{9E77B9DE-E76A-454d-B4B5-52496358FC65}" . 
ies:idDateOfBirth rdfs:comment "The Date of Birth as specified on the respective IdentityDocument." . 
ies:idDateOfBirth rdfs:subPropertyOf ies:relationship . 
ies:idDateOfBirth rdfs:domain ies:IdentityDocument . 
ies:idDateOfBirth rdfs:range ies:ParticularPeriod . 
ies:idDateOfIssue rdf:type owl:ObjectProperty . 
ies:idDateOfIssue sparx:guid "{ACAC12AD-16C3-480d-8149-C026F8BE9F81}" . 
ies:idDateOfIssue rdfs:comment "The date that the respective Identity Document was actually issued � this is different from the ValidFromDate on EphemeralIdDocuments." . 
ies:idDateOfIssue rdfs:subPropertyOf ies:relationship . 
ies:idDateOfIssue rdfs:domain ies:IdentityDocument . 
ies:idDateOfIssue rdfs:range ies:ParticularPeriod . 
ies:idEmergencyContactName rdf:type owl:DatatypeProperty . 
ies:idEmergencyContactName sparx:guid "{96B7C774-1FE0-4307-BB62-B5899F953FF2}" . 
ies:idEmergencyContactName rdfs:comment "The name of an emergency contact as printed on the IdentityDocument" . 
ies:idEmergencyContactName rdfs:subPropertyOf ies:attribute . 
ies:idEmergencyContactName rdfs:domain ies:IdentityDocument . 
ies:idEmergencyContactTelNo rdf:type owl:DatatypeProperty . 
ies:idEmergencyContactTelNo sparx:guid "{0198C1BE-43A0-4841-925E-FA5C47991AC3}" . 
ies:idEmergencyContactTelNo rdfs:comment "The telephone number of an emergency contact as printed on the IdentityDocument" . 
ies:idEmergencyContactTelNo rdfs:subPropertyOf ies:attribute . 
ies:idEmergencyContactTelNo rdfs:domain ies:IdentityDocument . 
ies:Identifier rdf:type rdfs:Class . 
ies:Identifier sparx:guid "{315E6AD3-F2DA-4f69-864F-DA2B95121E2E}" . 
ies:Identifier rdfs:comment "A Name that is unique within the specified context" . 
ies:Identifier rdfs:subClassOf ies:Name . 
ies:IdentityDocument rdf:type rdfs:Class . 
ies:IdentityDocument sparx:guid "{BDF4EBD9-7F41-4d90-91A7-571177330C1B}" . 
ies:IdentityDocument rdfs:comment "An IndividualDocument used to confirm the identity of the bearer (and often enables a particular activity � e.g. a passport enables the bearer to travel across international borders)." . 
ies:IdentityDocument rdfs:subClassOf ies:IndividualDocument . 
ies:idFamilyName rdf:type owl:DatatypeProperty . 
ies:idFamilyName sparx:guid "{CCD1F7FE-C42A-4503-BF24-00E8805BD5DD}" . 
ies:idFamilyName rdfs:comment "The family name as printed on the IdentityDocument" . 
ies:idFamilyName rdfs:subPropertyOf ies:attribute . 
ies:idFamilyName rdfs:domain ies:IdentityDocument . 
ies:idGender rdf:type owl:ObjectProperty . 
ies:idGender sparx:guid "{D5B27630-C222-45be-87C2-5C4F8592487B}" . 
ies:idGender rdfs:comment "The gender as recorded on the respective IdentityDocument" . 
ies:idGender rdfs:subPropertyOf ies:relationship . 
ies:idGender rdfs:domain ies:IdentityDocument . 
ies:idGender rdfs:range ies:Gender . 
ies:idGivenNames rdf:type owl:DatatypeProperty . 
ies:idGivenNames sparx:guid "{77CA0C8D-71F0-4cb9-8621-407396FAC5A1}" . 
ies:idGivenNames rdfs:comment "The given names as printed on the IdentityDocument" . 
ies:idGivenNames rdfs:subPropertyOf ies:attribute . 
ies:idGivenNames rdfs:domain ies:IdentityDocument . 
ies:idLowerRange rdf:type owl:ObjectProperty . 
ies:idLowerRange sparx:guid "{6C79CE89-8E17-4ee7-ABA8-DDA5D4AFC78B}" . 
ies:idLowerRange rdfs:comment "A relationship between a CommunicationsIdentifierRange and the CommunicationsIdentifier that is the lower limit of the identifier range " . 
ies:idLowerRange rdfs:subPropertyOf ies:relationship . 
ies:idLowerRange rdfs:domain ies:CommunicationsIdentifierRange . 
ies:idLowerRange rdfs:range ies:CommunicationsIdentifier . 
ies:idOnCard rdf:type owl:ObjectProperty . 
ies:idOnCard sparx:guid "{92D9B068-F8D4-4cbc-AD57-1DA39D5CC1C7}" . 
ies:idOnCard rdfs:comment "A relationship that asserts a NationalIdentityNumber (which identifies a person) is featured on a NationalIdentityCard" . 
ies:idOnCard rdfs:subPropertyOf ies:relationship . 
ies:idOnCard rdfs:domain ies:NationalIdentityCard . 
ies:idOnCard rdfs:range ies:NationalIdentityNumber . 
ies:idUpperRange rdf:type owl:ObjectProperty . 
ies:idUpperRange sparx:guid "{7615FB07-E0C5-4734-AFC8-FD52688DD2CC}" . 
ies:idUpperRange rdfs:comment "A relationship between a CommunicationsIdentifierRange and the CommunicationsIdentifier that is the upper limit of the identifier range " . 
ies:idUpperRange rdfs:subPropertyOf ies:relationship . 
ies:idUpperRange rdfs:domain ies:CommunicationsIdentifierRange . 
ies:idUpperRange rdfs:range ies:CommunicationsIdentifier . 
ies:IdUsedInCheckIn rdf:type rdfs:Class . 
ies:IdUsedInCheckIn sparx:guid "{F481C966-058B-4caf-A427-9E492CAD0D63}" . 
ies:IdUsedInCheckIn rdfs:comment "An EventParticipant where an IdentityDocument is used in a CheckIn event" . 
ies:IdUsedInCheckIn rdfs:subClassOf ies:EventParticipant . 
ies:ilrProficiency rdf:type owl:DatatypeProperty . 
ies:ilrProficiency sparx:guid "{471CF113-1728-47fd-A763-D1FA69226FC4}" . 
ies:ilrProficiency rdfs:comment "The Proficiency qualifier is specified using the Interagency Language Roundtable (ILR) scale [E].(a) ILR Level 0 � No proficiency(b) ILR Level 1 � Elementary Proficiency(c) ILR Level 2 � Limited Working Proficiency(d) ILR Level 3 � Professional Working Proficiency(e) ILR Level 4 � Full Professional Proficiency(f) ILR Level 5 � Native or Bilingual Proficiency" . 
ies:ilrProficiency rdfs:subPropertyOf ies:attribute . 
ies:ilrProficiency rdfs:domain ies:LanguageProficiency . 
ies:IMEI rdf:type rdfs:Class . 
ies:IMEI sparx:guid "{3987794E-6E2E-4457-8BF7-47813B51B139}" . 
ies:IMEI rdfs:comment "The International Mobile Equipment Identity used to identify GSM, WCDMA and iDEN mobile phone handsets, as well as some satellite phones.Usually a 15-digit number (14 digits plus a check digit)Example Value:123456789012345" . 
ies:IMEI rdfs:subClassOf ies:CommunicationsIdentifier . 
ies:IMSI rdf:type rdfs:Class . 
ies:IMSI sparx:guid "{C817C1ED-863B-41f0-B5C1-14117E926A94}" . 
ies:IMSI rdfs:comment "The International Mobile Subscriber NumberHistorically, this is stored as a 64-bit number on the SIM Card (it is NOT identity of the SIM Card itself), but now can be a software assigned identifier to any mobile subscriber interface. An IMSI is usually presented as a 15-digit number, but it can be shorter.The first three digits are the Mobile Country Code (MCC), followed by a 2 or 3 digit Mobile Network Code (MNC) and the remaining digits are the Mobile Subscription Identification Number (MSIN).For the example shown this would be:- 404=India,- 68=MTNL Delhi- 1234567890=Subscriber ID" . 
ies:IMSI rdfs:subClassOf ies:CommunicationsIdentifier . 
ies:IncarceratingOrganisation rdf:type rdfs:Class . 
ies:IncarceratingOrganisation sparx:guid "{321CB600-140F-452f-96B7-640DE8289ECF}" . 
ies:IncarceratingOrganisation rdfs:comment "An Organisationss role in incarcerating a Person" . 
ies:IncarceratingOrganisation rdfs:subClassOf ies:ActiveEventParticipant . 
ies:IncarceratingOrganisation rdfs:subClassOf ies:PersonState . 
ies:Incarceration rdf:type rdfs:Class . 
ies:Incarceration sparx:guid "{06972684-050B-4f36-9393-B8790D510F5C}" . 
ies:Incarceration rdfs:comment "A LawEnforcement EndToEndActivity where a Person is incarcerated" . 
ies:Incarceration rdfs:subClassOf ies:LawEnforcement . 
ies:Incarceration rdfs:subClassOf ies:EndToEndActivity . 
ies:IncarcerationFacility rdf:type rdfs:Class . 
ies:IncarcerationFacility sparx:guid "{B5C15382-451A-4446-BBE6-C67FBDB04402}" . 
ies:IncarcerationFacility rdfs:comment "A Facility used for incarceration - e.g. a prison, detention centre, or remand facility" . 
ies:IncarcerationFacility rdfs:subClassOf ies:Facility . 
ies:inCategory rdf:type owl:ObjectProperty . 
ies:inCategory sparx:guid "{D10B4B95-5BF1-4e3f-A2A8-8F52F045C31A}" . 
ies:inCategory rdfs:comment "An rdf:type relationship that asserts a Representation belongs to a ContentCategory" . 
ies:inCategory rdfs:subPropertyOf rdf:type . 
ies:inCategory rdfs:range ies:ContentCategory . 
ies:inCategory rdfs:domain ies:Representation . 
ies:inCategory rdfs:subPropertyOf ies:relationship . 
ies:IncomingGovernment rdf:type rdfs:Class . 
ies:IncomingGovernment sparx:guid "{BC752C7E-611B-47d6-BA89-05E58CD23803}" . 
ies:IncomingGovernment rdfs:comment "The Government that took power after a ChangeOfGovernment" . 
ies:IncomingGovernment rdfs:subClassOf ies:EventParticipant . 
ies:IncumbentRepresentative rdf:type rdfs:Class . 
ies:IncumbentRepresentative sparx:guid "{5C4C2871-5F61-4704-83D0-9F8CF42890BF}" . 
ies:IncumbentRepresentative rdfs:comment "A Person in-office prior to the Election being decided" . 
ies:IncumbentRepresentative rdfs:subClassOf ies:EventParticipant . 
ies:InDisagreement rdf:type rdfs:Class . 
ies:InDisagreement sparx:guid "{F12D45EA-66D5-4016-BDF7-E1CD8F48CCF5}" . 
ies:InDisagreement rdfs:comment "An EventParticipant where a ResponsibleActor is in disagreement" . 
ies:InDisagreement rdfs:subClassOf ies:ActiveEventParticipant . 
ies:IndividualDocument rdf:type rdfs:Class . 
ies:IndividualDocument sparx:guid "{0F327324-6B4E-40b1-B96B-97A334BA5E4A}" . 
ies:IndividualDocument rdfs:comment "An Asset that is a written, photographed or drawn representation of thoughts. This might include, but not limited to, formal reports, books, legal instruments. Such documents might exist in a wide variety of forms, both printed and in electronic form.Note: this is an individual document  - i.e. physical or (rarely) a specific electronic copy (e.g. on a specific hard disk...told you it was rare). In most cases, we refer to the document in general - WorkOfDocumentation " . 
ies:IndividualDocument rdfs:subClassOf ies:Asset . 
ies:IndividualDocumentID rdf:type rdfs:Class . 
ies:IndividualDocumentID sparx:guid "{D68F4E10-957A-4e98-8447-8F2768940DA7}" . 
ies:IndividualDocumentID rdfs:comment "An Identifier used to uniquely identify an IndividualDocument" . 
ies:IndividualDocumentID rdfs:subClassOf ies:Identifier . 
ies:influencedBy rdf:type owl:ObjectProperty . 
ies:influencedBy sparx:guid "{411F5C4C-9AD0-462a-BE10-3F43958B7D66}" . 
ies:influencedBy rdfs:comment "A relationship between a ResponsibleActor and the thing that influences them" . 
ies:influencedBy rdfs:subPropertyOf ies:relationship . 
ies:influencedBy rdfs:range ies:ExchangedItem . 
ies:influencedBy rdfs:domain ies:ResponsibleActorState . 
ies:informationContent rdf:type owl:ObjectProperty . 
ies:informationContent sparx:guid "{5BEE4248-DC98-4625-8553-3BB2171A1EDE}" . 
ies:informationContent rdfs:comment "A relationship between a WebResourceState and a Representation that asserts the Representation is the content of the WebResourceNote: a state is used here as the content may change over time even though the WebResource persists" . 
ies:informationContent rdfs:subPropertyOf ies:relationship . 
ies:informationContent rdfs:domain ies:WebResourceState . 
ies:informationContent rdfs:range ies:Representation . 
ies:inGroup rdf:type owl:ObjectProperty . 
ies:inGroup sparx:guid "{C21D2CA2-6F42-4b7c-9092-8B8C5B7BAF9F}" . 
ies:inGroup rdfs:comment "A property linking an ExchangedItem to a GroupOfItems indicating that it belongs to that group.Note: An ExchangedItem may be in more than one group and a group may contain more than one ExchangedItem" . 
ies:inGroup rdfs:domain ies:ExchangedItem . 
ies:inGroup rdfs:range ies:GroupOfItems . 
ies:inLanguage rdf:type owl:ObjectProperty . 
ies:inLanguage sparx:guid "{FF902F8E-6B22-4f17-9C16-48543251D22E}" . 
ies:inLanguage rdfs:comment "An rdf:type relationship that asserts a Representation is in a particular Language" . 
ies:inLanguage rdfs:subPropertyOf rdf:type . 
ies:inLanguage rdfs:subPropertyOf ies:relationship . 
ies:inLanguage rdfs:range ies:Language . 
ies:inLanguage rdfs:domain ies:Representation . 
ies:inLocation rdf:type owl:ObjectProperty . 
ies:inLocation sparx:guid "{463F9B14-2D14-4364-B4F0-658A20DFCBFA}" . 
ies:inLocation rdfs:comment "A partOf relationship to indicate an Element is entirely within a Location" . 
ies:inLocation rdfs:subPropertyOf ies:isPartOf . 
ies:inLocation rdfs:range ies:Location . 
ies:inPeriod rdf:type owl:ObjectProperty . 
ies:inPeriod sparx:guid "{2F08EF25-A5C8-48ad-85E3-903DB008AA19}" . 
ies:inPeriod rdfs:comment "A partOf relationship to indicate an Elements lifetime is entirely within a PeriodOfTimeExample:Freds birth is in May 1978" . 
ies:inPeriod rdfs:subPropertyOf ies:isPartOf . 
ies:inPeriod rdfs:range ies:PeriodOfTime . 
ies:inPeriod rdfs:domain ies:Element . 
ies:inPossessionOf rdf:type owl:ObjectProperty . 
ies:inPossessionOf sparx:guid "{0A28624B-C5E3-461e-B84A-E55B550B5DD6}" . 
ies:inPossessionOf rdfs:comment "A Relationship between a ResponsibleActor and an Asset they have in their possession.Note: this is separate to ownership - e.g. the possessor may well be the owner (use the owns relationship) but may also be a result of borrowing, theft, temporary custodianship, " . 
ies:inPossessionOf rdfs:range ies:Asset . 
ies:inPossessionOf rdfs:subPropertyOf ies:hasAccessTo . 
ies:InPost rdf:type rdfs:Class . 
ies:InPost sparx:guid "{6C1949B5-B86B-4940-8912-9008CCD67150}" . 
ies:InPost rdfs:comment "A temporal state of a ResponsibleActor when they are in a Post" . 
ies:InPost rdfs:subClassOf ies:ResponsibleActorState . 
ies:inRepresentation rdf:type owl:ObjectProperty . 
ies:inRepresentation sparx:guid "{7238489D-6802-4733-9F7F-9B31D02B3C81}" . 
ies:inRepresentation rdfs:comment "A relationship that asserts a Representation is part of another Representation" . 
ies:inRepresentation rdfs:subPropertyOf ies:relationship . 
ies:inRepresentation rdfs:domain ies:Representation . 
ies:inRepresentation rdfs:range ies:Representation . 
ies:inScheme rdf:type owl:ObjectProperty . 
ies:inScheme sparx:guid "{7EB9FE85-127C-4918-AC56-62E1BE1DE825}" . 
ies:inScheme rdfs:comment "An rdf:type relationship that asserts a Representation is a member of a RepresentationScheme" . 
ies:inScheme rdfs:subPropertyOf rdf:type . 
ies:inScheme rdfs:domain ies:Name . 
ies:inScheme rdfs:range ies:NamingScheme . 
ies:installedSoftware rdf:type owl:ObjectProperty . 
ies:installedSoftware sparx:guid "{B37ADF66-D5D0-4144-9539-DA91BA302914}" . 
ies:installedSoftware rdfs:comment "A relationship indicating Software is installed on a Device" . 
ies:installedSoftware rdfs:domain ies:DeviceState . 
ies:installedSoftware rdfs:subPropertyOf ies:relationship . 
ies:installedSoftware rdfs:range ies:Software . 
ies:IntelligenceAgency rdf:type rdfs:Class . 
ies:IntelligenceAgency sparx:guid "{F87E3B6F-5872-47eb-89F8-6642DD7C8237}" . 
ies:IntelligenceAgency rdfs:comment "A GovernmentOrganisation that collects, analyses or disseminates intelligence" . 
ies:IntelligenceAgency rdfs:subClassOf ies:GovernmentOrganisation . 
ies:IntelligenceOperation rdf:type rdfs:Class . 
ies:IntelligenceOperation sparx:guid "{A0A9CD13-A4B4-415b-9187-64C9B72E2F4E}" . 
ies:IntelligenceOperation rdfs:comment "An OperationalEvent that involves the gathering, analysis or dissemination of intelligence" . 
ies:IntelligenceOperation rdfs:subClassOf ies:OperationalEvent . 
ies:InteractiveCommunication rdf:type rdfs:Class . 
ies:InteractiveCommunication sparx:guid "{6D5E11EE-C61A-4e38-913F-BBAF2A34A288}" . 
ies:InteractiveCommunication rdfs:comment "A Communication that occurs synchronously - e.g. a video or voice call" . 
ies:InteractiveCommunication rdfs:subClassOf ies:Communication . 
ies:Interested rdf:type rdfs:Class . 
ies:Interested sparx:guid "{B1D011F9-9585-49eb-97C4-86E82D6F0BCF}" . 
ies:Interested rdfs:comment "A ResponsibleActorState where the Actor is interested in something" . 
ies:Interested rdfs:subClassOf ies:ResponsibleActorState . 
ies:interestedIn rdf:type owl:ObjectProperty . 
ies:interestedIn sparx:guid "{7BD2B884-F02C-4da2-AF6A-21B790FBF669}" . 
ies:interestedIn rdfs:comment "A Relationship between a ResponsibleActor (or state thereof) and an Entity they are interested in." . 
ies:interestedIn rdfs:subPropertyOf ies:relationship . 
ies:interestedIn rdfs:domain ies:Interested . 
ies:interestedIn rdfs:range ies:ExchangedItem . 
ies:InternationalCoalition rdf:type rdfs:Class . 
ies:InternationalCoalition sparx:guid "{AE70547D-8E7E-474e-B7FD-F0A81F470157}" . 
ies:InternationalCoalition rdfs:comment "An Organisation formed of Nations who have agreed to pursue a particular course (e.g. a war)" . 
ies:InternationalCoalition rdfs:subClassOf ies:Organisation . 
ies:intimidatedBy rdf:type owl:ObjectProperty . 
ies:intimidatedBy sparx:guid "{39D0AC05-01DB-423a-861A-26E6125DF906}" . 
ies:intimidatedBy rdfs:comment "A Relationship between two ResponsibleActor Entities where one (range) intimidates the other (domain)." . 
ies:intimidatedBy rdfs:subPropertyOf ies:relationship . 
ies:intimidatedBy rdfs:range ies:ResponsibleActor . 
ies:intimidatedBy rdfs:domain ies:ResponsibleActorState . 
ies:Investigation rdf:type rdfs:Class . 
ies:Investigation sparx:guid "{2912E599-436D-4b79-B94F-02FA2319F201}" . 
ies:Investigation rdfs:comment "An IntelligenceOperation that researches a particular threat, or theme. " . 
ies:Investigation rdfs:subClassOf ies:OperationalEvent . 
ies:Investigation rdfs:subClassOf ies:EndToEndActivity . 
ies:Investigator rdf:type rdfs:Class . 
ies:Investigator sparx:guid "{3525F314-87ED-43c8-9A84-68EDCD203B30}" . 
ies:Investigator rdfs:comment "An Operator role where a Person is an investigator" . 
ies:Investigator rdfs:subClassOf ies:Operator . 
ies:IPAddress rdf:type rdfs:Class . 
ies:IPAddress sparx:guid "{451C4C40-4183-4130-B67C-6F746B8B8BCA}" . 
ies:IPAddress rdfs:comment "An Identifier that is an Internet Protocol address." . 
ies:IPAddress rdfs:subClassOf ies:CommunicationsIdentifier . 
ies:IPAddressRange rdf:type rdfs:Class . 
ies:IPAddressRange sparx:guid "{BEC2FDBC-6F37-4446-AEE1-3D4627DDD5F2}" . 
ies:IPAddressRange rdfs:comment "A CommunicationIdentifierRange between two IPAddress instancesIn these examples the IPv4 address range is specified using the following format:&lt;lower address&gt; - &lt;upper address&gt; using one of a number of different IPv4 address notations.The IPv4 address range is all the IPv4 addresses between the &lt;lower address&gt; and the &lt;upper address&gt; (inclusive).Both examples here represent the same address range (but in different notations).The Dot Decimal Range notation specifies the &lt;lower address&gt; and the &lt;upper address&gt; in Dot Decimal form � whereeach of these 32-bit IPv4 addresses are expressed as four octets expressed individually in decimal and separated by periods.The Dot Hexadecimal Range notation specifies the &lt;lower address&gt; and the &lt;upper address&gt; in Dot Hexadecimal form � where each of these 32-bit IPv4 addresses are expressed as four octets where each octet is prefixed with 0x, expressed individually in hexadecimal and separated by periods." . 
ies:IPAddressRange rdfs:subClassOf ies:CommunicationsIdentifierRange . 
ies:IPPhoneHandset rdf:type rdfs:Class . 
ies:IPPhoneHandset sparx:guid "{0B494F4A-9E82-4667-89AD-3D22FC9B5742}" . 
ies:IPPhoneHandset rdfs:subClassOf ies:CommunicationsDevice . 
ies:IPv4Address rdf:type rdfs:Class . 
ies:IPv4Address sparx:guid "{142D6D4D-6EF3-48aa-8B7B-86DA73690E3E}" . 
ies:IPv4Address rdfs:comment "An IPAddress conforming to v4 of the standard" . 
ies:IPv4Address rdfs:subClassOf ies:IPAddress . 
ies:IPv6Address rdf:type rdfs:Class . 
ies:IPv6Address sparx:guid "{78549D65-75F2-41c3-AC14-F0D441AD6354}" . 
ies:IPv6Address rdfs:comment "An IPAddress conforming to v6 of the standard" . 
ies:IPv6Address rdfs:subClassOf ies:IPAddress . 
ies:isAuthorisedForUseWithPassport rdf:type owl:ObjectProperty . 
ies:isAuthorisedForUseWithPassport sparx:guid "{1CA57828-3B6B-450b-B477-C59A196EAE34}" . 
ies:isAuthorisedForUseWithPassport rdfs:comment "The passport associated with the Visa.Note: if the IES data does not already contain the associated passport, a Passport instance must be created, and the appropriate passport number specified." . 
ies:isAuthorisedForUseWithPassport rdfs:subPropertyOf ies:relationship . 
ies:isAuthorisedForUseWithPassport rdfs:domain ies:TravelVisa . 
ies:isAuthorisedForUseWithPassport rdfs:range ies:Passport . 
ies:isCentroidOf rdf:type owl:ObjectProperty . 
ies:isCentroidOf sparx:guid "{44ADC197-D9FA-4889-B6AF-929C3546F4A0}" . 
ies:isCentroidOf rdfs:comment "An inLocation relationship to indicate a PointOnEarthSurface is the centroid of a Location" . 
ies:isCentroidOf rdfs:subPropertyOf ies:inLocation . 
ies:isCentroidOf rdfs:domain ies:PointOnEarthSurface . 
ies:isDisposedTo rdf:type owl:ObjectProperty . 
ies:isDisposedTo sparx:guid "{B093F8DA-AE08-4819-8E1C-F119EF212566}" . 
ies:isDisposedTo rdfs:comment "An rdf:type relationship that asserts an Element is a member of a DispositionalClass - i.e. it is disposed to (capable of, tends to, etc.) the specified disposition." . 
ies:isDisposedTo rdfs:subPropertyOf rdf:type . 
ies:isDisposedTo rdfs:subPropertyOf ies:relationship . 
ies:isDisposedTo rdfs:domain ies:Element . 
ies:isDisposedTo rdfs:range ies:DispositionalClass . 
ies:isEndOf rdf:type owl:ObjectProperty . 
ies:isEndOf sparx:guid "{EA859D48-5BA4-40b3-A52D-1465D1765262}" . 
ies:isEndOf rdfs:comment "An isStateOf that relates a BoundingState to the Element it marks the end of" . 
ies:isEndOf rdfs:subPropertyOf ies:isStateOf . 
ies:isEndOf rdfs:domain ies:BoundingState . 
ies:isIdentifiedBy rdf:type owl:ObjectProperty . 
ies:isIdentifiedBy sparx:guid "{FBA54EEF-91BF-4ba2-8B67-79C899963149}" . 
ies:isIdentifiedBy rdfs:comment "A hasName relationship that asserts an Identifier identifies an ExchangedItem" . 
ies:isIdentifiedBy rdfs:subPropertyOf ies:hasName . 
ies:isIdentifiedBy rdfs:domain ies:ExchangedItem . 
ies:isIdentifiedBy rdfs:range ies:Identifier . 
ies:isLegalTenderIn rdf:type owl:ObjectProperty . 
ies:isLegalTenderIn sparx:guid "{2415B865-3C37-4595-9F38-11075EAB5D34}" . 
ies:isLegalTenderIn rdfs:comment "The Country in which a Currency is legal tender" . 
ies:isLegalTenderIn rdfs:subPropertyOf ies:relationship . 
ies:isLegalTenderIn rdfs:domain ies:Currency . 
ies:isLegalTenderIn rdfs:range ies:Country . 
ies:ISO19125-WKT rdf:type rdfs:Class . 
ies:ISO19125-WKT sparx:guid "{22B79CFD-DEDA-42e1-8864-E8421D36CF19}" . 
ies:ISO19125-WKT rdfs:comment "A GeoRepresentation using Well-Known-Text encoding for ISO19125 simple features.Note: the WKT must include the coordinate reference system used - e.g WGS 84" . 
ies:ISO19125-WKT rdfs:subClassOf ies:GeoRepresentation . 
ies:ISO3166_1Alpha_3 rdf:type rdfs:Class . 
ies:ISO3166_1Alpha_3 sparx:guid "{B92D79E2-9E7D-4df7-8D38-3D884AA09AD2}" . 
ies:ISO3166_1Alpha_3 rdfs:comment "ISO 3166-1 alpha 3 (3-Letter Country Code)" . 
ies:ISO3166_1Alpha_3 rdfs:subClassOf ies:GeoIdentity . 
ies:ISO639-3Code rdf:type rdfs:Class . 
ies:ISO639-3Code sparx:guid "{ECFED94D-CC69-46b9-B09D-B282D5665787}" . 
ies:ISO639-3Code rdfs:comment "ISO639-3 three-letter language code" . 
ies:ISO639-3Code rdfs:subClassOf ies:Identifier . 
ies:iso8601PeriodRepresentation rdf:type owl:DatatypeProperty . 
ies:iso8601PeriodRepresentation sparx:guid "{E9372543-434E-45d3-A1F0-8D711952D10A}" . 
ies:iso8601PeriodRepresentation rdfs:comment "A ISO8601 datetime (as xsd:dateTime if possible) that represents the ParticularPeriod.Note: the representation is also encoded in the URI of the period, this is an additional required attribute to enable querying by dateTime and SPARQL temporal operations." . 
ies:iso8601PeriodRepresentation rdfs:subPropertyOf ies:attribute . 
ies:iso8601PeriodRepresentation rdfs:domain ies:ParticularPeriod . 
ies:isParticipantIn rdf:type owl:ObjectProperty . 
ies:isParticipantIn sparx:guid "{BAEA86D9-C90E-4f8d-96F5-A01BB0C49711}" . 
ies:isParticipantIn rdfs:comment "An isPartOf that relates an EventParticipant to the Event it participates in." . 
ies:isParticipantIn rdfs:subPropertyOf ies:isPartOf . 
ies:isParticipantIn rdfs:range ies:Event . 
ies:isParticipantIn rdfs:domain ies:EventParticipant . 
ies:isParticipantStateIn rdf:type owl:ObjectProperty . 
ies:isParticipantStateIn sparx:guid "{A77A19DA-2775-4dfa-A76C-41C158AC582C}" . 
ies:isParticipantStateIn rdfs:comment "An isParticipantIn and an isStateOf that relates an EventParticipant to the Event it participates, in the case where the participant has the same spatial extent as the Event for that period of time.Note: This is really just a bit of logical plumbing to enable start and end states of Events to be all of the event for a period of time." . 
ies:isParticipantStateIn rdfs:subPropertyOf ies:isStateOf . 
ies:isParticipantStateIn rdfs:subPropertyOf ies:isParticipantIn . 
ies:isParticipationOf rdf:type owl:ObjectProperty . 
ies:isParticipationOf sparx:guid "{DF9F6056-CCD4-41aa-9A86-536F6150EC25}" . 
ies:isParticipationOf rdfs:comment "An isStateOf that relates an EventParticipant to the Element that is the participant" . 
ies:isParticipationOf rdfs:subPropertyOf ies:isStateOf . 
ies:isParticipationOf rdfs:domain ies:EventParticipant . 
ies:isParticipationOf rdfs:range ies:Entity . 
ies:isPartOf rdf:type owl:ObjectProperty . 
ies:isPartOf sparx:guid "{CD85D7F7-783B-4d06-B023-56DBBDDC02DC}" . 
ies:isPartOf rdfs:comment "A relationship linking an Element to another that it is part of.Examples:London partOf UKMy Arm partOf Me" . 
ies:isPartOf rdfs:subPropertyOf ies:relationship . 
ies:isPartOf rdfs:domain ies:Element . 
ies:isPartOf rdfs:range ies:Element . 
ies:isPrimaryForOrganisation rdf:type owl:ObjectProperty . 
ies:isPrimaryForOrganisation sparx:guid "{D6974F5E-B24C-4a06-9AC1-DB6299E9BF55}" . 
ies:isPrimaryForOrganisation rdfs:comment "A relationship linking an ExchangedItem to the ResponsibleActor that prefers the use of that ExchangedItem.This is used when there are more than one state, name, etc. for a given item, and there is a requirement to specify which one is considered primary / preferred by a particular Organisation.Examples:* A primary name for a person (applied to PersonName)* A primary DoB for a person (applied to BirthState)* A primary nationality for a person (applied to the PersonState that links to the Nation)" . 
ies:isPrimaryForOrganisation rdfs:subPropertyOf ies:relationship . 
ies:isPrimaryForOrganisation rdfs:domain ies:ExchangedItem . 
ies:isPrimaryForOrganisation rdfs:range ies:Organisation . 
ies:isRepresentedAs rdf:type owl:ObjectProperty . 
ies:isRepresentedAs sparx:guid "{D106A0A9-55C4-454f-9E20-35BA54114036}" . 
ies:isRepresentedAs rdfs:comment "A relationship that asserts a Representation in someway depicts an ExchangedItem" . 
ies:isRepresentedAs rdfs:subPropertyOf ies:relationship . 
ies:isRepresentedAs rdfs:domain ies:ExchangedItem . 
ies:isRepresentedAs rdfs:range ies:Representation . 
ies:isStartOf rdf:type owl:ObjectProperty . 
ies:isStartOf sparx:guid "{D9E068B1-2A44-4523-B8FC-F9888212B35C}" . 
ies:isStartOf rdfs:comment "An isStateOf that relates a BoundingState to the Element it marks the start of" . 
ies:isStartOf rdfs:subPropertyOf ies:isStateOf . 
ies:isStartOf rdfs:domain ies:BoundingState . 
ies:isStateOf rdf:type owl:ObjectProperty . 
ies:isStateOf sparx:guid "{F7CBF87A-6ECC-4c9f-B698-FD3CF3F7980E}" . 
ies:isStateOf rdfs:comment "An isPartOf linking an Element to a temporal State of that Element Examples:You, you yesterday" . 
ies:isStateOf rdfs:subPropertyOf ies:isPartOf . 
ies:isStateOf rdfs:range ies:Element . 
ies:isStateOf rdfs:domain ies:State . 
ies:issuerIdentificationNumber rdf:type owl:DatatypeProperty . 
ies:issuerIdentificationNumber sparx:guid "{5E353B12-2503-429f-A683-F7C77E0DFBAD}" . 
ies:issuerIdentificationNumber rdfs:comment "The IIN is a number that uniquely identifies the issuer of the Bank Card.An ISO/IEC 7812 number contains a single-digit major industry identifier (MII), a six-digit issuer identification number (IIN), an individual account identification number, and a single digit checksum." . 
ies:issuerIdentificationNumber rdfs:subPropertyOf ies:attribute . 
ies:issuerIdentificationNumber rdfs:domain ies:BankCard . 
ies:issuingAgency rdf:type owl:ObjectProperty . 
ies:issuingAgency sparx:guid "{74D86486-8E18-474a-8930-B92E759BBE06}" . 
ies:issuingAgency rdfs:comment "The Organisation that issued the ticket � this might be different from the travel provider." . 
ies:issuingAgency rdfs:subPropertyOf ies:relationship . 
ies:issuingAgency rdfs:range ies:Organisation . 
ies:issuingAgency rdfs:domain ies:TravelTicket . 
ies:isTeacherOf rdf:type owl:ObjectProperty . 
ies:isTeacherOf sparx:guid "{B8650A61-3B08-4f62-8EAB-0F9D007B20CE}" . 
ies:isTeacherOf rdfs:comment "A Relationship between two ResponsibleActor Entities that indicates one teaches the other.In the case where the teaching is occasional / ad-hoc (i.e. there isnt an ongoing course) then the instance of the ResponsibleActorState should also be an instance of DiscontinuousState" . 
ies:isTeacherOf rdfs:subPropertyOf ies:relationship . 
ies:isTeacherOf rdfs:domain ies:PersonState . 
ies:isTeacherOf rdfs:range ies:Person . 
ies:JointAccount rdf:type rdfs:Class . 
ies:JointAccount sparx:guid "{AD17E3D9-CAB2-4a60-99C9-109F4496F92F}" . 
ies:JointAccount rdfs:comment "A FinancialAccount held by more than one person" . 
ies:JointAccount rdfs:subClassOf ies:FinancialAccount . 
ies:Journey rdf:type rdfs:Class . 
ies:Journey sparx:guid "{8B571665-0AA1-40be-A7A0-A35BE86B7192}" . 
ies:Journey rdfs:comment "A Movement which is made up of two or more TravelLegsNote:  this may include a number of legs to the journey (i.e. instances of TravelLeg that are part of the Journey)" . 
ies:Journey rdfs:subClassOf ies:Movement . 
ies:jurisdictionOfRights rdf:type owl:ObjectProperty . 
ies:jurisdictionOfRights sparx:guid "{62EF76B2-4AB0-4e1e-98C4-61C3A85BF980}" . 
ies:jurisdictionOfRights rdfs:comment "A Relationship between Rights and the Nation under whose laws the Rights are established" . 
ies:jurisdictionOfRights rdfs:subPropertyOf ies:relationship . 
ies:jurisdictionOfRights rdfs:domain ies:Rights . 
ies:jurisdictionOfRights rdfs:range ies:Nation . 
ies:knownAssociateOf rdf:type owl:ObjectProperty . 
ies:knownAssociateOf sparx:guid "{57F3607C-0204-4590-9442-24F372A35931}" . 
ies:knownAssociateOf rdfs:comment "A Relationship between two ResponsibleActor Entities where both are known to know each other but the extent to which they interact (e.g. friendship, work, criminal activity, etc.) is not known." . 
ies:knownAssociateOf rdfs:subPropertyOf ies:relationship . 
ies:knownAssociateOf rdfs:domain ies:ResponsibleActorState . 
ies:knownAssociateOf rdfs:range ies:ResponsibleActor . 
ies:LandlineHandset rdf:type rdfs:Class . 
ies:LandlineHandset sparx:guid "{57C9F8DF-AFE6-4374-9403-ACACAC26FCE4}" . 
ies:LandlineHandset rdfs:comment "A CommunicationsDevice that connects using fixed line telecommunications" . 
ies:LandlineHandset rdfs:subClassOf ies:CommunicationsDevice . 
ies:LandlineTelephoneAccount rdf:type rdfs:Class . 
ies:LandlineTelephoneAccount sparx:guid "{D7F83A2D-6428-4211-964D-E1E8A8089083}" . 
ies:LandlineTelephoneAccount rdfs:comment "A TelephoneAccount where the telephones in use connect using a wired network and operate only in a specific location" . 
ies:LandlineTelephoneAccount rdfs:subClassOf ies:TelephoneAccount . 
ies:Language rdf:type rdfs:Class . 
ies:Language sparx:guid "{82652FF5-258F-459c-BC7F-6DAC65E1ECA1}" . 
ies:Language rdfs:comment "A ClassOfRepresentation that is a spoken or written form of human communication" . 
ies:Language rdfs:subClassOf ies:ClassOfRepresentation . 
ies:LanguageProficiency rdf:type rdfs:Class . 
ies:LanguageProficiency sparx:guid "{EB73AB32-8232-4b58-8271-640DDDDCC7DE}" . 
ies:LanguageProficiency rdfs:comment "A ClassOfPersonState indicating the proficiency a person has in a particular language at that state in their life." . 
ies:LanguageProficiency rdfs:subClassOf ies:ClassOfPersonState . 
ies:Latitude rdf:type rdfs:Class . 
ies:Latitude sparx:guid "{BD14EF81-DDBC-4bdf-BC40-E5FAE937ADA6}" . 
ies:Latitude rdfs:comment "A GeoIdentity that is a decimal representation of an angle of latitude of a PointOnEarthSurface (WGS84)" . 
ies:Latitude rdfs:subClassOf ies:GeoIdentity . 
ies:LawEnforcement rdf:type rdfs:Class . 
ies:LawEnforcement sparx:guid "{3876B81C-E316-4e11-A6C4-8024E52F769B}" . 
ies:LawEnforcement rdfs:comment "An Event that involves the application of criminal law" . 
ies:LawEnforcement rdfs:subClassOf ies:Event . 
ies:LawEnforcementOrganisation rdf:type rdfs:Class . 
ies:LawEnforcementOrganisation sparx:guid "{15806699-2F00-4891-B2A0-8A211CEDFC10}" . 
ies:LawEnforcementOrganisation rdfs:comment "A GovernmentOrganisation that investigates crimes and brings the perpetrators to justice. Wikipedia definition: Law enforcement is any system by which some members of society act in an organized manner to enforce the law by discovering, deterring, rehabilitating, or punishing people who violate the rules and norms governing that society." . 
ies:LawEnforcementOrganisation rdfs:subClassOf ies:GovernmentOrganisation . 
ies:LeadInvestigator rdf:type rdfs:Class . 
ies:LeadInvestigator sparx:guid "{E1AF7AFE-FA2F-40f7-88A3-CA6988BC2E0D}" . 
ies:LeadInvestigator rdfs:comment "An Investigator who is charge of an Investigation" . 
ies:LeadInvestigator rdfs:subClassOf ies:Investigator . 
ies:Length rdf:type rdfs:Class . 
ies:Length sparx:guid "{5C21DE93-329F-4209-87FF-19610CB0D367}" . 
ies:Length rdfs:comment "The Measure of distance as specified by the International System of Quantities" . 
ies:Length rdfs:subClassOf ies:StandardMeasure . 
ies:LifecycleEvent rdf:type rdfs:Class . 
ies:LifecycleEvent sparx:guid "{FA07AB7A-0EE8-4258-BE8B-260F9A1192A7}" . 
ies:LifecycleEvent rdfs:comment "An Event that brings about change to its environment or another Element - e.g. creation, destruction or modification" . 
ies:LifecycleEvent rdfs:subClassOf ies:Event . 
ies:Likes rdf:type rdfs:Class . 
ies:Likes sparx:guid "{B292748F-D41E-4c3b-9335-04D4B06A1F34}" . 
ies:Likes rdfs:comment "An Interested State where a ResponsibleActor likes something" . 
ies:Likes rdfs:subClassOf ies:Interested . 
ies:LineOfAddress rdf:type rdfs:Class . 
ies:LineOfAddress sparx:guid "{E0D8895D-2230-4c80-8B06-351581C53436}" . 
ies:LineOfAddress rdfs:comment "A line in an Address. There may be any number of these." . 
ies:LineOfAddress rdfs:subClassOf ies:GeoIdentity . 
ies:LiveCast rdf:type rdfs:Class . 
ies:LiveCast sparx:guid "{ECC6E85E-CB08-464d-81A4-BA3ECDCB784C}" . 
ies:LiveCast rdfs:comment "An OnlineArtefact that is video or audio streamed online in real time.Note: the begin and end dates for a LiveCast instance mark its life online rather than the duration of the actual recording. The recording itself should be tracked using an OnlineContentCreation Event." . 
ies:LiveCast rdfs:subClassOf ies:OnlineArtefact . 
ies:Location rdf:type rdfs:Class . 
ies:Location sparx:guid "{E1A494ED-D493-44ab-8BF9-ABC6889D4D9A}" . 
ies:Location rdfs:comment "An Entity that is a geographic place which specifies a point or an area on the Earths surface or elsewhere." . 
ies:Location rdfs:subClassOf ies:Entity . 
ies:Location rdfs:subClassOf ies:LocationState . 
ies:LocationState rdf:type rdfs:Class . 
ies:LocationState sparx:guid "{7CAFACD0-94F9-400e-B20E-E4ECE31943E5}" . 
ies:LocationState rdfs:comment "A temporal state of a Location" . 
ies:LocationState rdfs:subClassOf ies:State . 
ies:Logoff rdf:type rdfs:Class . 
ies:Logoff sparx:guid "{8010625F-BA25-457a-93CF-7EC1E99261D7}" . 
ies:Logoff rdfs:comment "A OnlineEvent where an OnlineAccount logs out of an OnlineService" . 
ies:Logoff rdfs:subClassOf ies:OnlineEvent . 
ies:Logon rdf:type rdfs:Class . 
ies:Logon sparx:guid "{43CDB7F8-E77E-4eba-A92E-C6A74AF954CA}" . 
ies:Logon rdfs:comment "A OnlineEvent where an OnlineAccount logs onto an OnlineService" . 
ies:Logon rdfs:subClassOf ies:OnlineEvent . 
ies:Longitude rdf:type rdfs:Class . 
ies:Longitude sparx:guid "{B2C5522F-EA60-455a-B00F-9CC87A76E5B0}" . 
ies:Longitude rdfs:comment "The GeoIdentity that is a decimal representation of an angle of longitude of a PointOnEarthSurface (WGS84)" . 
ies:Longitude rdfs:subClassOf ies:GeoIdentity . 
ies:Loves rdf:type rdfs:Class . 
ies:Loves sparx:guid "{E543978A-06D0-4c79-BCCD-A62DE9294A85}" . 
ies:Loves rdfs:comment "A interestedIn relationship where a Person loves another Person" . 
ies:Loves rdfs:subClassOf ies:Interested . 
ies:lowerBound rdf:type owl:ObjectProperty . 
ies:lowerBound sparx:guid "{96717346-1DF4-4eae-A7CF-E389B4454B47}" . 
ies:lowerBound rdfs:comment "A relationship a MeasureRange to the Measure that is its lower bound" . 
ies:lowerBound rdfs:subPropertyOf ies:relationship . 
ies:lowerBound rdfs:range ies:Measure . 
ies:lowerBound rdfs:domain ies:MeasureRange . 
ies:LuminousIntensity rdf:type rdfs:Class . 
ies:LuminousIntensity sparx:guid "{8431C546-B6F9-406f-9ECD-383FE985D115}" . 
ies:LuminousIntensity rdfs:comment "The Measure of radiated light" . 
ies:LuminousIntensity rdfs:subClassOf ies:StandardMeasure . 
ies:MACAddress rdf:type rdfs:Class . 
ies:MACAddress sparx:guid "{DE1EDE92-142C-4c05-AD61-BE58822B2E17}" . 
ies:MACAddress rdfs:comment "A CommunicationsIdentifier that is used to identify network interface controllersVarious forms of the MAC address can be used:(a) six groups of two hexadecimal digits, separated by hyphens (-) or colons (:), in transmission order(b) three groups of four hexadecimal digits separated by dots (.) again in transmission order.2. The make &amp; model of the network interface is encoded within the MAC address." . 
ies:MACAddress rdfs:subClassOf ies:CommunicationsIdentifier . 
ies:maintains rdf:type owl:ObjectProperty . 
ies:maintains sparx:guid "{727175D4-0998-49a0-BAEE-6B8F1F1FD8D4}" . 
ies:maintains rdfs:comment "A Relationship between a ResponsibleActorState and an Entity they maintain" . 
ies:maintains rdfs:subPropertyOf ies:relationship . 
ies:maintains rdfs:range ies:Entity . 
ies:maintains rdfs:domain ies:ResponsibleActorState . 
ies:make rdf:type owl:ObjectProperty . 
ies:make sparx:guid "{E0036B31-8D73-4268-8959-6E9A5EE55BB2}" . 
ies:make rdfs:comment "A relationship from the device to its make - i.e. organisation that brands it (even if the manufacture is contracted-out)Example - an iPhone 6S has make Apple" . 
ies:make rdfs:domain ies:Asset . 
ies:make rdfs:subPropertyOf ies:relationship . 
ies:make rdfs:range ies:Organisation . 
ies:MaliciousAccountUse rdf:type rdfs:Class . 
ies:MaliciousAccountUse sparx:guid "{F0C08ADE-7EE5-4392-9877-5FD8FB4076E9}" . 
ies:MaliciousAccountUse rdfs:comment "An OnlineAccountInUse where the account is used to conduct a CriminalActivity online" . 
ies:MaliciousAccountUse rdfs:subClassOf ies:OnlineAccountInUse . 
ies:managedBy rdf:type owl:ObjectProperty . 
ies:managedBy sparx:guid "{8991D995-1915-47b7-B180-D9EBC4A1FD1F}" . 
ies:managedBy rdfs:comment "A worksFor relationship where the managed ResponsibleActorState (domain) is managed by another ResponsibleActor (range)." . 
ies:managedBy rdfs:subPropertyOf ies:worksFor . 
ies:MapGridArea rdf:type rdfs:Class . 
ies:MapGridArea sparx:guid "{18A66904-823F-471d-A465-65ECD2D69867}" . 
ies:MapGridArea rdfs:comment "A Location whose area is specified by a grid on a map.Note this is the actual area, not the map grid. " . 
ies:MapGridArea rdfs:subClassOf ies:Location . 
ies:MapGridArea rdfs:subClassOf ies:Asset . 
ies:Marriage rdf:type rdfs:Class . 
ies:Marriage sparx:guid "{9DFEDF24-1203-4341-B282-BD37C1B9CDF5}" . 
ies:Marriage rdfs:comment "An EndToEndActivity covering the entire extent of a two peoples marriage (from the ceremony to either divorce or death)Note: As IES4 does not increase the scope of IES3, Marriage also includes common-law partners and civil partnerships" . 
ies:Marriage rdfs:subClassOf ies:LawEnforcement . 
ies:Marriage rdfs:subClassOf ies:EndToEndActivity . 
ies:Married rdf:type rdfs:Class . 
ies:Married sparx:guid "{D03A0D8B-79F5-4901-97BC-2767FD46CD5F}" . 
ies:Married rdfs:comment "A State when a Person is married to another person" . 
ies:Married rdfs:subClassOf ies:PersonState . 
ies:Married rdfs:subClassOf ies:EventParticipant . 
ies:Mass rdf:type rdfs:Class . 
ies:Mass sparx:guid "{AE8FC416-9650-472d-99C6-F0A46B7359EB}" . 
ies:Mass rdfs:comment "The Measure of an Entitys resistance to acceleration as specified by the International System of Quantities" . 
ies:Mass rdfs:subClassOf ies:StandardMeasure . 
ies:Measure rdf:type rdfs:Class . 
ies:Measure sparx:guid "{6CF79FCE-E2C9-4e8b-848C-39BD8616F77D}" . 
ies:Measure rdfs:comment "An Characteristic which is measurable on a scale" . 
ies:Measure rdfs:subClassOf ies:Characteristic . 
ies:MeasureRange rdf:type rdfs:Class . 
ies:MeasureRange sparx:guid "{CCBBF963-EB27-40d5-BE9F-47CDF4D352F8}" . 
ies:MeasureRange rdfs:comment "A Measure specified by upper and lower bound Measures" . 
ies:MeasureRange rdfs:subClassOf ies:Measure . 
ies:measureUnit rdf:type owl:ObjectProperty . 
ies:measureUnit sparx:guid "{161079F3-8089-4124-A67A-5D6A7A4EA511}" . 
ies:measureUnit rdfs:comment "An rdf:type relationship that asserts a Measure is represented using a particular UnitOfMeasure" . 
ies:measureUnit rdfs:subPropertyOf rdf:type . 
ies:measureUnit rdfs:subPropertyOf ies:relationship . 
ies:measureUnit rdfs:domain ies:MeasureValue . 
ies:measureUnit rdfs:range ies:UnitOfMeasure . 
ies:MeasureValue rdf:type rdfs:Class . 
ies:MeasureValue sparx:guid "{3693B7DE-DCE7-4bf9-BC2A-A8914DA4A11E}" . 
ies:MeasureValue rdfs:comment "A Representation of the value of a MeasureNote: A UnitOfMeasure is almost always required. The reason it is not mandatory is that in some cases (due to partial reporting) we do not have complete information - e.g. we know the value was stated to be 10 but we dont know if thats metres or feet" . 
ies:MeasureValue rdfs:subClassOf ies:Representation . 
ies:MediaFile rdf:type rdfs:Class . 
ies:MediaFile sparx:guid "{CE2E2EB2-17F7-4054-9107-E8DC275B0B11}" . 
ies:MediaFile rdfs:comment "A DataObject that is a stand-alone file - e.g. a video, image or sound recording" . 
ies:MediaFile rdfs:subClassOf ies:DataObject . 
ies:Meeting rdf:type rdfs:Class . 
ies:Meeting sparx:guid "{6445E51F-3DDF-4dcf-ABDF-3ED123D53188}" . 
ies:Meeting rdfs:comment "A CoLocation where the attendees (Presence) communicate with each other" . 
ies:Meeting rdfs:subClassOf ies:CoLocation . 
ies:MeetingChair rdf:type rdfs:Class . 
ies:MeetingChair sparx:guid "{B499C172-310D-4c5f-BA92-93B1C7874EEB}" . 
ies:MeetingChair rdfs:comment "An Attendance where the Person involved is the chair of a Meeting" . 
ies:MeetingChair rdfs:subClassOf ies:Attendance . 
ies:Message rdf:type rdfs:Class . 
ies:Message sparx:guid "{70AEDFC7-2B17-43d8-BF49-B5ACF8812317}" . 
ies:Message rdfs:comment "A Communication or OnlineContentEvent where a message is sent" . 
ies:Message rdfs:subClassOf ies:Communication . 
ies:Message rdfs:subClassOf ies:OnlineContentEvent . 
ies:messageContent rdf:type owl:DatatypeProperty . 
ies:messageContent sparx:guid "{E1A85BEA-C374-4727-A189-E536BA248D98}" . 
ies:messageContent rdfs:comment "An attribute representing the content of a messageExample:messageContent = See you at Waterloo station at 18:15" . 
ies:messageContent rdfs:subPropertyOf ies:attribute . 
ies:messageContent rdfs:domain ies:Message . 
ies:MilitaryAttack rdf:type rdfs:Class . 
ies:MilitaryAttack sparx:guid "{8787BE51-8FE0-4d76-97B4-608311434F5B}" . 
ies:MilitaryAttack rdfs:comment "A MilitaryEvent where force is usedNote: was called Attack in v3.x - now called MilitaryAttack to distinguish from domestic attacks, terrorist attacks, hacking attacks, etc." . 
ies:MilitaryAttack rdfs:subClassOf ies:MilitaryEvent . 
ies:MilitaryEvent rdf:type rdfs:Class . 
ies:MilitaryEvent sparx:guid "{8EA1764B-26BE-4a72-ADEF-385C4CD657C3}" . 
ies:MilitaryEvent rdfs:comment "An OperationalEvent that involves military staff" . 
ies:MilitaryEvent rdfs:subClassOf ies:OperationalEvent . 
ies:MilitaryOrganisation rdf:type rdfs:Class . 
ies:MilitaryOrganisation sparx:guid "{492AB59A-342E-4d74-B85B-E6CA95BBC3B2}" . 
ies:MilitaryOrganisation rdfs:comment "A GovernmentOrganisation that conducts warfighting, peacekeeping and emergency civil support functions" . 
ies:MilitaryOrganisation rdfs:subClassOf ies:GovernmentOrganisation . 
ies:missionPurpose rdf:type owl:DatatypeProperty . 
ies:missionPurpose sparx:guid "{A6DED556-12B8-45b7-A69C-A6A3D813269B}" . 
ies:missionPurpose rdfs:comment "A short description of why an IntelligenceOperation was carried out used for legal justificationAgencies that work in the intelligence domain may wish to standardise these descriptions. " . 
ies:missionPurpose rdfs:subPropertyOf ies:attribute . 
ies:missionPurpose rdfs:domain ies:OperationalEvent . 
ies:MobileHandset rdf:type rdfs:Class . 
ies:MobileHandset sparx:guid "{3BF8FC71-64BD-4fb5-BEFD-D7FCB936FA12}" . 
ies:MobileHandset rdfs:comment "A CommunicationsDevice that is a portable telephone using cellular networks" . 
ies:MobileHandset rdfs:subClassOf ies:CommunicationsDevice . 
ies:MobileTelephoneAccount rdf:type rdfs:Class . 
ies:MobileTelephoneAccount sparx:guid "{9F5EDA24-5991-48e7-9303-C86E25A196CF}" . 
ies:MobileTelephoneAccount rdfs:comment "A TelephoneAccount where the telephones in use connects using a cellular network" . 
ies:MobileTelephoneAccount rdfs:subClassOf ies:TelephoneAccount . 
ies:Model rdf:type rdfs:Class . 
ies:Model sparx:guid "{7A879268-33C2-4f2b-8928-9E78AFF01E69}" . 
ies:Model rdfs:comment "An rdf:type relationship asserting the Model of a DeviceExamples:* Smartphone* Apple iPhone 6S* Ford Focus" . 
ies:Model rdfs:subClassOf ies:ClassOfDevice . 
ies:model rdf:type owl:ObjectProperty . 
ies:model sparx:guid "{98BDD06F-1BD7-42b8-B338-20A198BCF90A}" . 
ies:model rdfs:comment "A relationship from the device to the ModelOfDevice" . 
ies:model rdfs:subPropertyOf ies:relationship . 
ies:model rdfs:domain ies:Device . 
ies:model rdfs:subPropertyOf rdf:type . 
ies:model rdfs:range ies:Model . 
ies:Modifier rdf:type rdfs:Class . 
ies:Modifier sparx:guid "{21A341AE-9A38-4f45-BCB5-B29B02DC1B90}" . 
ies:Modifier rdfs:comment "An EventParticipant where a ResponsibleActor participates in a Modify event as a modifier" . 
ies:Modifier rdfs:subClassOf ies:ActiveEventParticipant . 
ies:Modify rdf:type rdfs:Class . 
ies:Modify sparx:guid "{3EF09CE4-79B0-42be-9AA1-12B97611BF2B}" . 
ies:Modify rdfs:comment "A LifecycleEvent where something is changed" . 
ies:Modify rdfs:subClassOf ies:LifecycleEvent . 
ies:MoneyTransfer rdf:type rdfs:Class . 
ies:MoneyTransfer sparx:guid "{D94ED70F-8CCA-4c6e-8AE5-65450BBA62D7}" . 
ies:MoneyTransfer rdfs:comment "A BusinessEvent where an AmountOfMoney is moved from one FinancialAccount to another.Usually a Money Transfer event will involve two accounts but we might not know both, or it might be a cash transfer � in which case only one of the participants might be specified." . 
ies:MoneyTransfer rdfs:subClassOf ies:BusinessEvent . 
ies:MoneyTransfer rdfs:subClassOf ies:TradeEvent . 
ies:Movement rdf:type rdfs:Class . 
ies:Movement sparx:guid "{95B5ACC4-956A-4b29-AB9E-BDCD12EF319F}" . 
ies:Movement rdfs:comment "An Event where an Entity moves from one place to another." . 
ies:Movement rdfs:subClassOf ies:Event . 
ies:Moving rdf:type rdfs:Class . 
ies:Moving sparx:guid "{D06C3801-F91C-436d-9D7F-DFDE29B48E5C}" . 
ies:Moving rdfs:comment "An EventParticipant in which an Entity moves from one Location to another" . 
ies:Moving rdfs:subClassOf ies:EventParticipant . 
ies:Name rdf:type rdfs:Class . 
ies:Name sparx:guid "{7D7CC966-56EB-4220-A650-A993E598F2E2}" . 
ies:Name rdfs:comment "A Representation that is used to refer to something, usually in context of a NamingSchemeExamples:GBR - the ISO Trigram for the United KingdomGB - the FIPS two-letter code for the United KingdomMichael Caine  - stage name for Maurice Micklewhite" . 
ies:Name rdfs:subClassOf ies:Representation . 
ies:NamingScheme rdf:type rdfs:Class . 
ies:NamingScheme sparx:guid "{222534A5-25C8-4ecd-BE55-27DA1534D402}" . 
ies:NamingScheme rdfs:comment "An ClassOfClassOfEntity whose instances collect together all Names that belong to a particular scheme - i.e. an organisational identity scheme, a systems primary key format, etc." . 
ies:NamingScheme rdfs:subClassOf ies:ClassOfClassOfEntity . 
ies:Nation rdf:type rdfs:Class . 
ies:Nation sparx:guid "{6AE6F8A5-F427-4ea6-BABD-5720F07430F5}" . 
ies:Nation rdfs:comment "The people of a Country (or group of Countries recognised as a Nation).Note: this is distinct to a Country which is the land mass under control by the Nation, though ISO Country codes are regularly used to also identify Nations. " . 
ies:Nation rdfs:subClassOf ies:RegionalConstituency . 
ies:NationalIdentityCard rdf:type rdfs:Class . 
ies:NationalIdentityCard sparx:guid "{843EDE77-78C4-4a09-9866-DBCC726AD5E6}" . 
ies:NationalIdentityCard rdfs:comment "An IdentityDocument issued by a Government to identify a Person" . 
ies:NationalIdentityCard rdfs:subClassOf ies:IdentityDocument . 
ies:NationalIdentityNumber rdf:type rdfs:Class . 
ies:NationalIdentityNumber sparx:guid "{F2CF8705-DA4A-4131-AB60-CF1AC33BED95}" . 
ies:NationalIdentityNumber rdfs:comment "An Identifier of a Person that is specified by a GovernmentOrganisation " . 
ies:NationalIdentityNumber rdfs:subClassOf ies:Identifier . 
ies:nationality rdf:type owl:ObjectProperty . 
ies:nationality sparx:guid "{45CDA5C1-624D-4f2f-81F6-EF19300820A9}" . 
ies:nationality rdfs:comment "A relationship to a Nation which recognises the Person (or State of Person, as it is possible to renounce a nationality) as one of their nationals." . 
ies:nationality rdfs:subPropertyOf ies:relationship . 
ies:nationality rdfs:range ies:Nation . 
ies:nationality rdfs:domain ies:PersonState . 
ies:natureOfInterest rdf:type owl:DatatypeProperty . 
ies:natureOfInterest sparx:guid "{0C0728AF-B9F2-418f-A03E-107689F0ACA0}" . 
ies:natureOfInterest rdfs:comment "NatureOfInterest is limited to the following values:� Personal� Professional� Academic" . 
ies:natureOfInterest rdfs:subPropertyOf ies:attribute . 
ies:natureOfInterest rdfs:domain ies:Interested . 
ies:nearTo rdf:type owl:ObjectProperty . 
ies:nearTo sparx:guid "{E3BB8B07-9CC5-407a-8CC7-E2B0E1B69476}" . 
ies:nearTo rdfs:comment "A relationship linking an Entity to another Entity it is proximate to in space" . 
ies:nearTo rdfs:subPropertyOf ies:relationship . 
ies:nearTo rdfs:domain ies:Entity . 
ies:nearTo rdfs:range ies:Entity . 
ies:Negotiation rdf:type rdfs:Class . 
ies:Negotiation sparx:guid "{FB2EA8AE-164A-4642-82E3-D2622DC6FCCB}" . 
ies:Negotiation rdfs:comment "An AgreementStage where parties are trying to find agreement" . 
ies:Negotiation rdfs:subClassOf ies:AgreementStage . 
ies:Negotiator rdf:type rdfs:Class . 
ies:Negotiator sparx:guid "{D4B25AAF-F083-45ba-8188-25DE9D86013D}" . 
ies:Negotiator rdfs:comment "An EventParticipant where a ResponsibleActor negotiates an agreement" . 
ies:Negotiator rdfs:subClassOf ies:ActiveEventParticipant . 
ies:nephewOrNieceOf rdf:type owl:ObjectProperty . 
ies:nephewOrNieceOf sparx:guid "{1995033D-7AF2-468c-998D-61E86FB51B16}" . 
ies:nephewOrNieceOf rdfs:comment "A Relationship between two Person Entities that indicates one is the nephew or niece of the other.Note: people can become nephews or nieces at different stages in their lives (e.g. as people marry) so PersonState should be used in cases where someone has not always been related in this way (i.e. not from birth)" . 
ies:nephewOrNieceOf rdfs:subPropertyOf ies:familiallyRelatedTo . 
ies:NetworkInterface rdf:type rdfs:Class . 
ies:NetworkInterface sparx:guid "{C544CCAC-91C5-4e82-B5D9-7A1B8D48E771}" . 
ies:NetworkInterface rdfs:comment "An Device (usually part of another Device) that provides wired or wireless access to a network.Network interfaces can often be removable. To model this, create DeviceStates of the NetworkInterface and make them part of the Device which hosts the interface for that period of time. " . 
ies:NetworkInterface rdfs:subClassOf ies:Device . 
ies:NetworkInterface rdfs:subClassOf ies:SystemState . 
ies:nextTo rdf:type owl:ObjectProperty . 
ies:nextTo sparx:guid "{F33CAAA7-85A7-4e41-B0D4-3EAC4E6F73CC}" . 
ies:nextTo rdfs:comment "A nearTo linking an Entity to another Entity it is immediately proximate to (i.e. touching) in space" . 
ies:nextTo rdfs:subPropertyOf ies:nearTo . 
ies:Nickname rdf:type rdfs:Class . 
ies:Nickname sparx:guid "{BA4B97EE-58E2-4796-949C-F62EAAAE56C9}" . 
ies:Nickname rdfs:comment "A PersonName that is an unofficial or casual nameNote:An nickname will often be applied to a State of the Person, as these tend to be non-permanent names" . 
ies:Nickname rdfs:subClassOf ies:PersonName . 
ies:NonDisclosureAgreement rdf:type rdfs:Class . 
ies:NonDisclosureAgreement sparx:guid "{672C510D-8836-4a41-8921-C732DF430278}" . 
ies:NonDisclosureAgreement rdfs:comment "An EndToEndAgreement where parties agree not to disclose certain information" . 
ies:NonDisclosureAgreement rdfs:subClassOf ies:EndToEndAgreement . 
ies:Northing rdf:type rdfs:Class . 
ies:Northing sparx:guid "{09649FE9-DDD7-4493-B9EC-7A716B0FC616}" . 
ies:Northing rdfs:comment "The GeoIdentity that is a representation of the northward componrnent of cartesian point on a map - i.e. on a 2D projection of the globe such as a mercator projection." . 
ies:Northing rdfs:subClassOf ies:GeoIdentity . 
ies:NotForProfitOrganisation rdf:type rdfs:Class . 
ies:NotForProfitOrganisation sparx:guid "{C2B4A066-E4A7-4cf5-BD1F-8381364F5D30}" . 
ies:NotForProfitOrganisation rdfs:comment "An Organisation where all income is reinvested, or distributed - i.e. no profit is made." . 
ies:NotForProfitOrganisation rdfs:subClassOf ies:Organisation . 
ies:Notify rdf:type rdfs:Class . 
ies:Notify sparx:guid "{15EF63E0-1223-4874-A2D4-43F75ACF5315}" . 
ies:Notify rdfs:comment "An OnlineContentEvent where a notification is raised - i.e.  an application-generated event (not a user-generated event)" . 
ies:Notify rdfs:subClassOf ies:OnlineContentEvent . 
ies:objectContent rdf:type owl:DatatypeProperty . 
ies:objectContent sparx:guid "{222FBD07-DCCF-40c6-BD15-4ADBC64A8AA5}" . 
ies:objectContent rdfs:comment "The content of the data object.Whenever a DataObject is exchanged it must include either the ObjectContent or an ObjectContentReference or both.The ContentStandard qualifier specifies the standard (either by name or by reference) that is applicable to the content of the DataObject.The ContentFormat qualifier specifies the format of the content of the DataObject." . 
ies:objectContent rdfs:subPropertyOf ies:representationValue . 
ies:objectContent rdfs:domain ies:DataObject . 
ies:objectContentReference rdf:type owl:DatatypeProperty . 
ies:objectContentReference sparx:guid "{6B06ABDD-05CF-485c-A483-563C5E85F189}" . 
ies:objectContentReference rdfs:comment "An ObjectContentReference is a resolvable reference to the �content� of the respective DataObject.Whenever a DataObject is exchanged it must include either the ObjectContent or an ObjectContentReference or both.The ContentStandard qualifier specifies the standard that is applicable to the content of the DataObject that is referred to by the ObjectContentReference.The ContentFormat qualifier specifies the format of the content of the DataObject that is referred to by the ObjectContentReference." . 
ies:objectContentReference rdfs:subPropertyOf ies:attribute . 
ies:objectContentReference rdfs:domain ies:DataObject . 
ies:ObjectName rdf:type rdfs:Class . 
ies:ObjectName sparx:guid "{9A372833-B327-4cb0-9950-786A2FBF7CC3}" . 
ies:ObjectName rdfs:comment "A Name given to a DataObject." . 
ies:ObjectName rdfs:subClassOf ies:Name . 
ies:Observation rdf:type rdfs:Class . 
ies:Observation sparx:guid "{8CA40CCF-A099-49fd-80CB-CA6DA733FAB4}" . 
ies:Observation rdfs:comment "An Event where an Element (Event or Entity) is observed by an Entity (i.e. a Person or Device)" . 
ies:Observation rdfs:subClassOf ies:Event . 
ies:Observed rdf:type rdfs:Class . 
ies:Observed sparx:guid "{CC05ABD0-7BAB-4484-8E8C-ED07C1AA3C93}" . 
ies:Observed rdfs:comment "An EventParticipant where an Element is Observed" . 
ies:Observed rdfs:subClassOf ies:EventParticipant . 
ies:Observer rdf:type rdfs:Class . 
ies:Observer sparx:guid "{C58A1AB4-19E2-48d0-B606-3BDFC5DD3860}" . 
ies:Observer rdfs:comment "An EventParticipant where an Entity observes another Entity or Event" . 
ies:Observer rdfs:subClassOf ies:ActiveEventParticipant . 
ies:ObserverStatus rdf:type rdfs:Class . 
ies:ObserverStatus sparx:guid "{FB2FDA67-B258-4b18-9E95-3B9DFAB8FB14}" . 
ies:ObserverStatus rdfs:comment "When a Government has observer rights at a Summit" . 
ies:ObserverStatus rdfs:subClassOf ies:EventParticipant . 
ies:OffenceCode rdf:type rdfs:Class . 
ies:OffenceCode sparx:guid "{66A24EF2-F417-46c7-A68D-D4540260F64F}" . 
ies:OffenceCode rdfs:comment "An Identifier for a ClassOfCriminalActivityThe Home Office Offence Classification Index [B] should be used wherever possible to specify the Crime Type" . 
ies:OffenceCode rdfs:subClassOf ies:Identifier . 
ies:OfferForSale rdf:type rdfs:Class . 
ies:OfferForSale sparx:guid "{1D589649-490D-4558-91D5-2D977B2B42DE}" . 
ies:OfferForSale rdfs:comment "A TradeEvent where one or more Entities of the same type (specified by an ClassOfEntity) are offered for sale or exchange" . 
ies:OfferForSale rdfs:subClassOf ies:TradeEvent . 
ies:OnJourney rdf:type rdfs:Class . 
ies:OnJourney sparx:guid "{80AFD655-A969-46be-BE72-035C053C1C4F}" . 
ies:OnJourney rdfs:comment "An EventParticipant in which an Entity is on a Journey (i.e. a multi-part journey)" . 
ies:OnJourney rdfs:subClassOf ies:Moving . 
ies:OnlineAccount rdf:type rdfs:Class . 
ies:OnlineAccount sparx:guid "{E95170B9-2599-46dc-BEDC-012B08F09D43}" . 
ies:OnlineAccount rdfs:comment "An Account that enables a person, organisation or other entity to participate within a particular online domain.Note: was called OnlineIdentifier in previous versions of IES" . 
ies:OnlineAccount rdfs:subClassOf ies:Account . 
ies:OnlineAccount rdfs:subClassOf ies:OnlineAccountState . 
ies:OnlineAccountInUse rdf:type rdfs:Class . 
ies:OnlineAccountInUse sparx:guid "{BCFD5BED-785D-4c5d-B004-2C8A5C7B40C3}" . 
ies:OnlineAccountInUse rdfs:comment "An EventParticipant where an OnlineAccount participates in an OnlineEvent" . 
ies:OnlineAccountInUse rdfs:subClassOf ies:ActiveEventParticipant . 
ies:onlineAccountProvider rdf:type owl:ObjectProperty . 
ies:onlineAccountProvider sparx:guid "{2CF1B157-A2F6-41c8-8A87-7B82EEB71F40}" . 
ies:onlineAccountProvider rdfs:comment "Relates an OnlineAccount to the OnlineService that provides and administers the account.Note:  was called Domain in previous IES versions" . 
ies:onlineAccountProvider rdfs:subPropertyOf ies:relationship . 
ies:onlineAccountProvider rdfs:domain ies:OnlineAccount . 
ies:onlineAccountProvider rdfs:range ies:OnlineService . 
ies:OnlineAccountState rdf:type rdfs:Class . 
ies:OnlineAccountState sparx:guid "{4C0D1724-B820-4a87-AD36-08C0612CE21E}" . 
ies:OnlineAccountState rdfs:comment "A temporal state of an OnlineAccount" . 
ies:OnlineAccountState rdfs:subClassOf ies:AccountState . 
ies:OnlineArtefact rdf:type rdfs:Class . 
ies:OnlineArtefact sparx:guid "{54500458-51CF-46b5-A5A3-14B1D5C7F755}" . 
ies:OnlineArtefact rdfs:comment "A WebResource which is any kind of media presented online that is more granular than a webpage, and user-generated - e.g. a blog post, tweet, facebook post, etc.Note: when applying begin and end states (and periods of time) to OnlineArtefact, the times should correspond to the life of the content, not the duration of the posting activity." . 
ies:OnlineArtefact rdfs:subClassOf ies:WebResource . 
ies:OnlineArtefactInEvent rdf:type rdfs:Class . 
ies:OnlineArtefactInEvent sparx:guid "{FE21E354-7770-4e6b-A7EA-E012F759E835}" . 
ies:OnlineArtefactInEvent rdfs:comment "An EventParticipant where an OnlineArtefact participates in an OnlineEvent" . 
ies:OnlineArtefactInEvent rdfs:subClassOf ies:EventParticipant . 
ies:OnlineArtefactInEvent rdfs:subClassOf ies:DeviceState . 
ies:OnlineComment rdf:type rdfs:Class . 
ies:OnlineComment sparx:guid "{FF216817-5B58-4db5-88C5-20AE6A466265}" . 
ies:OnlineComment rdfs:comment "An OnlineArtefact that is a comment on an existing OnlineArtefact instance" . 
ies:OnlineComment rdfs:subClassOf ies:OnlineArtefact . 
ies:onlineCommentOn rdf:type owl:ObjectProperty . 
ies:onlineCommentOn sparx:guid "{0A4C12E6-CA4C-43f1-9C6C-FBE23197975F}" . 
ies:onlineCommentOn rdfs:comment "Relates an OnlineComment to the OnlineContent that was commented on" . 
ies:onlineCommentOn rdfs:subPropertyOf ies:relationship . 
ies:onlineCommentOn rdfs:range ies:OnlineArtefact . 
ies:onlineCommentOn rdfs:domain ies:OnlineComment . 
ies:OnlineContentCreation rdf:type rdfs:Class . 
ies:OnlineContentCreation sparx:guid "{DB70D7EE-5076-4eb2-950B-63C71A3C8859}" . 
ies:OnlineContentCreation rdfs:comment "An OnlineContentEvent where a post is made.Examples:* Posting a blog* Posting a comment* Tweeting (other microblogs are available, probably)* A Facebook, LinkedIn, Instagram, etc. post" . 
ies:OnlineContentCreation rdfs:subClassOf ies:OnlineContentEvent . 
ies:OnlineContentCreation rdfs:subClassOf ies:Create . 
ies:OnlineContentEvent rdf:type rdfs:Class . 
ies:OnlineContentEvent sparx:guid "{2176DEAE-6B5A-4906-AE37-FC76B0A50C0D}" . 
ies:OnlineContentEvent rdfs:comment "An OnlineEvent where content (text, images, video, etc.) is uploaded, downloaded or viewed" . 
ies:OnlineContentEvent rdfs:subClassOf ies:OnlineEvent . 
ies:OnlineEvent rdf:type rdfs:Class . 
ies:OnlineEvent sparx:guid "{24499751-7D9B-4f2e-B880-8D5BC4FCEF30}" . 
ies:OnlineEvent rdfs:comment "An Event on the internet" . 
ies:OnlineEvent rdfs:subClassOf ies:Event . 
ies:OnlineLike rdf:type rdfs:Class . 
ies:OnlineLike sparx:guid "{5B50EECC-45FC-4e5b-933E-51BC0FEE0FCD}" . 
ies:OnlineLike rdfs:comment "OnlineArtefact that is a like of an existing OnlineArtefact instance" . 
ies:OnlineLike rdfs:subClassOf ies:OnlineArtefact . 
ies:onlineLikeOf rdf:type owl:ObjectProperty . 
ies:onlineLikeOf sparx:guid "{4A3F24C6-EEC9-48ce-93FB-26FF64E1268A}" . 
ies:onlineLikeOf rdfs:comment "Relates an OnlineLike to the OnlineContent that was liked" . 
ies:onlineLikeOf rdfs:subPropertyOf ies:relationship . 
ies:onlineLikeOf rdfs:domain ies:OnlineLike . 
ies:onlineLikeOf rdfs:range ies:OnlineArtefact . 
ies:onlinePublisher rdf:type owl:ObjectProperty . 
ies:onlinePublisher sparx:guid "{34F13F26-7C4E-451a-BDA0-62BA7738039F}" . 
ies:onlinePublisher rdfs:comment "Relates an OnlineArtefact to the ResponsibleActor that produced it." . 
ies:onlinePublisher rdfs:subPropertyOf ies:relationship . 
ies:onlinePublisher rdfs:domain ies:OnlineArtefact . 
ies:onlinePublisher rdfs:range ies:ResponsibleActor . 
ies:OnlineService rdf:type rdfs:Class . 
ies:OnlineService sparx:guid "{27BEFD0A-B30B-47db-B863-13E48D1172F9}" . 
ies:OnlineService rdfs:comment "A service provided on the internet." . 
ies:OnlineService rdfs:subClassOf ies:WebResource . 
ies:onlineServiceProvider rdf:type owl:ObjectProperty . 
ies:onlineServiceProvider sparx:guid "{DEE1404A-AAC3-4d46-9BA3-8E097A55C7F5}" . 
ies:onlineServiceProvider rdfs:comment "Relates an OnlineService to the ResponsibleActor that owns/runs it" . 
ies:onlineServiceProvider rdfs:subPropertyOf ies:relationship . 
ies:onlineServiceProvider rdfs:domain ies:OnlineService . 
ies:onlineServiceProvider rdfs:range ies:ResponsibleActor . 
ies:onlineServiceType rdf:type owl:ObjectProperty . 
ies:onlineServiceType sparx:guid "{2C9CEF7F-FA9A-4a0e-9E2C-AC3D3EB51D5C}" . 
ies:onlineServiceType rdfs:comment "The class of OnlineService" . 
ies:onlineServiceType rdfs:subPropertyOf ies:relationship . 
ies:onlineServiceType rdfs:domain ies:OnlineService . 
ies:onlineServiceType rdfs:subPropertyOf rdf:type . 
ies:onlineServiceType rdfs:range ies:ClassOfOnlineService . 
ies:OnlineShop rdf:type rdfs:Class . 
ies:OnlineShop sparx:guid "{980404C4-C512-4f36-B3B1-5088CC754DCF}" . 
ies:OnlineShop rdfs:comment "An EventParticipant where a ResponsibleActor participates in a TradeEvent as an online shop" . 
ies:OnlineShop rdfs:subClassOf ies:Retailer . 
ies:OpenAccount rdf:type rdfs:Class . 
ies:OpenAccount sparx:guid "{A8B06392-A9A3-4de4-93FB-24F08A546434}" . 
ies:OpenAccount rdfs:comment "An AccountAdminEvent where a new Account is opened" . 
ies:OpenAccount rdfs:subClassOf ies:AccountAdminEvent . 
ies:OperatingSystem rdf:type rdfs:Class . 
ies:OperatingSystem sparx:guid "{4F83D781-7E46-4ad4-B2A5-ECD27565EA49}" . 
ies:OperatingSystem rdfs:comment "Software that provides the basic access layer to hardware" . 
ies:OperatingSystem rdfs:subClassOf ies:Software . 
ies:OperationalEvent rdf:type rdfs:Class . 
ies:OperationalEvent sparx:guid "{59121C21-38E4-4224-8C2D-4D3E94A3A0D9}" . 
ies:OperationalEvent rdfs:comment "An Event conducted by military or national security actors" . 
ies:OperationalEvent rdfs:subClassOf ies:Event . 
ies:OperationalEvent ies:powertype ies:ClassOfOperationalEvent . 
ies:Operator rdf:type rdfs:Class . 
ies:Operator sparx:guid "{6730B57A-3E53-4bd2-B784-78C4FB239DBF}" . 
ies:Operator rdfs:comment "A ResponsibleActors role in an OperationalEvent where they are one of the operators " . 
ies:Operator rdfs:subClassOf ies:ActiveEventParticipant . 
ies:opposedTo rdf:type owl:ObjectProperty . 
ies:opposedTo sparx:guid "{436E6ABB-C1E3-484e-B15B-63E700B27EA8}" . 
ies:opposedTo rdfs:comment "A coupling between a ResponsibleActor (or state thereof) and an ClassOfElement to which they are opposedExamples: an organisation that is opposed to Nuclear Weapons" . 
ies:opposedTo rdfs:subPropertyOf ies:relationship . 
ies:opposedTo rdfs:domain ies:ResponsibleActorState . 
ies:opposedTo rdfs:range ies:ClassOfElement . 
ies:Organisation rdf:type rdfs:Class . 
ies:Organisation sparx:guid "{1ECB4C6E-6A30-4dc5-A4AC-9A9DF5B6A54F}" . 
ies:Organisation rdfs:comment "A ResponsibleActor that is a group of people formed for one or more of purposes � e.g. government organisations, educational organisations, terrorists organisations, religious organisations, etc." . 
ies:Organisation rdfs:subClassOf ies:ResponsibleActor . 
ies:Organisation rdfs:subClassOf ies:OrganisationState . 
ies:Organisation ies:powertype ies:ClassOfOrganisation . 
ies:OrganisationalRole rdf:type rdfs:Class . 
ies:OrganisationalRole sparx:guid "{C0B7C4B2-C067-4ca8-A9FB-E82782889250}" . 
ies:OrganisationalRole rdfs:comment "A Role that a ResponsibleActor can have in an Organisation" . 
ies:OrganisationalRole rdfs:subClassOf ies:Role . 
ies:OrganisationalRole rdfs:subClassOf ies:ClassOfResponsibleActorState . 
ies:OrganisationIdentifier rdf:type rdfs:Class . 
ies:OrganisationIdentifier sparx:guid "{13865B40-B57D-44e7-9658-00C45C8175C8}" . 
ies:OrganisationIdentifier rdfs:comment "A unique Identifier for an Organisation (more usually an OrganisationState)Example:DUNS numberVAT numberCompanies House NumberRegistered Charity Number" . 
ies:OrganisationIdentifier rdfs:subClassOf ies:Identifier . 
ies:OrganisationIdentifier rdfs:subClassOf ies:OrganisationName . 
ies:OrganisationName rdf:type rdfs:Class . 
ies:OrganisationName sparx:guid "{065C9B64-96E2-47f5-9769-E7942C1A208F}" . 
ies:OrganisationName rdfs:comment "A Name used to identify an Organisation" . 
ies:OrganisationName rdfs:subClassOf ies:Name . 
ies:OrganisationState rdf:type rdfs:Class . 
ies:OrganisationState sparx:guid "{F3DB6A59-B2DE-4743-A9A8-7DA9CCC68638}" . 
ies:OrganisationState rdfs:comment "A temporal state of an Organisation" . 
ies:OrganisationState rdfs:subClassOf ies:ResponsibleActorState . 
ies:orGroup rdf:type owl:DatatypeProperty . 
ies:orGroup sparx:guid "{71249792-E0AF-4f98-86ED-17115F1734A7}" . 
ies:orGroup rdfs:comment "The groups (if any) which the requesting user must be a member of at least one of in order to access the item. See the EDH specification for further details.Allowable Values:See EDH Standard" . 
ies:orGroup rdfs:domain ies:SecurityLabel . 
ies:originatingSystem rdf:type owl:ObjectProperty . 
ies:originatingSystem sparx:guid "{D4A003A3-7FEF-409c-8935-743CD97299E7}" . 
ies:originatingSystem rdfs:comment "The System that produced the dataset" . 
ies:originatingSystem rdfs:range ies:System . 
ies:originatingSystem rdfs:domain rdf:Statement . 
ies:originator rdf:type owl:ObjectProperty . 
ies:originator sparx:guid "{4978D7F3-E686-4b30-9356-F0C4DC7A158D}" . 
ies:originator rdfs:comment "The ResponsibleActor that produced the dataset" . 
ies:originator rdfs:range ies:ResponsibleActor . 
ies:originator rdfs:domain rdf:Statement . 
ies:OSGridReference rdf:type rdfs:Class . 
ies:OSGridReference sparx:guid "{697EAA12-8FD3-49e0-A4A2-A045B4570550}" . 
ies:OSGridReference rdfs:comment "A GeoIdentity that is an Ordnance Survey Grid Reference - i.e. pertaining to Great Britain." . 
ies:OSGridReference rdfs:subClassOf ies:GeoIdentity . 
ies:OutgoingGovernment rdf:type rdfs:Class . 
ies:OutgoingGovernment sparx:guid "{A5516CD2-940B-4827-B38A-AD86AF934E99}" . 
ies:OutgoingGovernment rdfs:comment "The Government that left power following a ChangeOfGovernment" . 
ies:OutgoingGovernment rdfs:subClassOf ies:EventParticipant . 
ies:owns rdf:type owl:ObjectProperty . 
ies:owns sparx:guid "{FDD94D9F-F343-4c1b-9688-752C896A3C7C}" . 
ies:owns rdfs:comment "A Relationship between a ResponsibleActor and an Asset they legally own" . 
ies:owns rdfs:subPropertyOf ies:relationship . 
ies:owns rdfs:domain ies:ResponsibleActorState . 
ies:owns rdfs:range ies:Asset . 
ies:parentOf rdf:type owl:ObjectProperty . 
ies:parentOf sparx:guid "{6F13083C-505A-473e-9EDB-B0E534A341FB}" . 
ies:parentOf rdfs:comment "A Relationship between two Person Entities that indicates one is the parent of the other" . 
ies:parentOf rdfs:subPropertyOf ies:ancestorOf . 
ies:parentOf rdfs:domain ies:Person . 
ies:parentOf rdfs:range ies:Person . 
ies:Parked rdf:type rdfs:Class . 
ies:Parked sparx:guid "{B6A503E5-3FC4-4a45-8DC0-994EA31A895A}" . 
ies:Parked rdfs:comment "A temporal state of a Vehicle where it is not moving. Examples:* A car parked on the roadside* A ship in dock or at anchor* An aircraft parked on the tarmac or in a hangar" . 
ies:Parked rdfs:subClassOf ies:VehicleState . 
ies:ParticularPeriod rdf:type rdfs:Class . 
ies:ParticularPeriod sparx:guid "{2173F463-524C-457c-B106-51322F64F122}" . 
ies:ParticularPeriod rdfs:comment "A PeriodOfTime that is a specific, contiguous extent of time.IMPORTANT NOTE: The URI of a ParticularPeriod shall be encoded as follows:http://iso8601.iso.org/2007-01-18T15%3A00%3A00Where the content after the / is % encoded (e.g. encodeURIComponent in javascript). In the example above, the unencoded content would be 2007-01-18T15:00:00The reason behind using a URI is that receiving systems can resolve the periods of time and de-duplicate. Examples:Tuesday 28th August 20182016December 1944" . 
ies:ParticularPeriod rdfs:subClassOf ies:PeriodOfTime . 
ies:PartNumber rdf:type rdfs:Class . 
ies:PartNumber sparx:guid "{772CD8A3-3DCA-4cc7-8BA3-17D1C57E94BC}" . 
ies:PartNumber rdfs:comment "A unique Identifier for the a ModelOfDeviceNote:  this is different to a serial number which is unique to each Device" . 
ies:PartNumber rdfs:subClassOf ies:Identifier . 
ies:PartOfFacility rdf:type rdfs:Class . 
ies:PartOfFacility sparx:guid "{3EFEA421-6B88-4e51-9B20-4FFA22E8C5CA}" . 
ies:PartOfFacility rdfs:comment "A Location that is contained within a Facility - e.g. a room, laboratory, floor, etc." . 
ies:PartOfFacility rdfs:subClassOf ies:RealEstate . 
ies:PartyInCommunication rdf:type rdfs:Class . 
ies:PartyInCommunication sparx:guid "{A5713B2C-E098-4dd2-BD46-42DA51899FEA}" . 
ies:PartyInCommunication rdfs:comment "An Event that is part of (usually one end of) a Communication Event.Sometimes, all we know about a PartyInCommunication is their CommunicationsIdentifier (phone number, e-mail address, maybe even just an IP address) so the isIdentifiedBy relationship may be applied to PartyInCommunication" . 
ies:PartyInCommunication rdfs:subClassOf ies:Event . 
ies:PartyToAgreement rdf:type rdfs:Class . 
ies:PartyToAgreement sparx:guid "{AF57E842-9BF7-4f6e-B180-DDEACB0F5386}" . 
ies:PartyToAgreement rdfs:comment "An EventParticipant where a ResponsibleActor is party to an EndToEndAgreementNote:  this includes EndToEndAgreements that were never ratified - i.e. they got to the negotiation stage but were never put into force" . 
ies:PartyToAgreement rdfs:subClassOf ies:ActiveEventParticipant . 
ies:Passenger rdf:type rdfs:Class . 
ies:Passenger sparx:guid "{D6D07656-1866-4cb4-97A7-FC4C1CB65416}" . 
ies:Passenger rdfs:comment "A PersonInTransit where the Person travelling is a Passenger on a Transit" . 
ies:Passenger rdfs:subClassOf ies:PersonInTransit . 
ies:PassengerName rdf:type rdfs:Class . 
ies:PassengerName sparx:guid "{E5C1270D-35AD-4f86-B0E4-1DC0039174E3}" . 
ies:PassengerName rdfs:comment "The Name of the Person being used for Travel - it may not be known if this is the actual Name the Person travelling, as someone else may be using their ticket." . 
ies:PassengerName rdfs:subClassOf ies:Name . 
ies:Passport rdf:type rdfs:Class . 
ies:Passport sparx:guid "{13ABC7CA-915E-4069-8EA7-FD205A5336C5}" . 
ies:Passport rdfs:comment "An IdentityDocument that confirms a Persons nationality and permits them to cross national boundaries" . 
ies:Passport rdfs:subClassOf ies:IdentityDocument . 
ies:payloadContents rdf:type owl:ObjectProperty . 
ies:payloadContents sparx:guid "{10DEB6B8-80CC-4bfc-B10F-1830B559C21F}" . 
ies:payloadContents rdfs:comment "A link from an ExchangePayload to an rdfs:Resource that is in that payload.If there is no payloadContents link, then it is assumed that all the contents of the file are in the ExchangePayload. Under this circumstance, more than one ExchangePayload would be an error. The payloadContents link will usually refer to a named graph, but it can also be used to refer to individual rdf:Statements and rdfs:Resources." . 
ies:payloadContents rdfs:domain ies:ExchangePayload . 
ies:payloadContents rdfs:range rdfs:Resource . 
ies:payloadLabel rdf:type owl:ObjectProperty . 
ies:payloadLabel sparx:guid "{259167E4-D0B3-4f03-9653-CAD778F5F6F3}" . 
ies:payloadLabel rdfs:comment "A mandatory link from an ExchangePayload to the SecurityLabel that provides the default access control for all statements in the payload.Note: individual statements may deviate from the default by applying their own SecurityLabels" . 
ies:payloadLabel rdfs:domain ies:ExchangePayload . 
ies:payloadLabel rdfs:range ies:SecurityLabel . 
ies:PaymentArtefact rdf:type rdfs:Class . 
ies:PaymentArtefact sparx:guid "{9882D901-1B22-4b89-81D1-031F840A20D0}" . 
ies:PaymentArtefact rdfs:comment "An Asset that is means of payment" . 
ies:PaymentArtefact rdfs:subClassOf ies:Asset . 
ies:paymentArtefactProvider rdf:type owl:ObjectProperty . 
ies:paymentArtefactProvider sparx:guid "{C793E699-C27B-49cc-9358-C4A0E17E609E}" . 
ies:paymentArtefactProvider rdfs:comment "The Organisation that provided the PaymentArtefact" . 
ies:paymentArtefactProvider rdfs:subPropertyOf ies:relationship . 
ies:paymentArtefactProvider rdfs:domain ies:PaymentArtefact . 
ies:paymentArtefactProvider rdfs:range ies:Organisation . 
ies:PeaceTreaty rdf:type rdfs:Class . 
ies:PeaceTreaty sparx:guid "{10FBBF98-4604-46d9-AD12-211597532B9E}" . 
ies:PeaceTreaty rdfs:comment "A Treaty that formalises the end of hostilities in a War" . 
ies:PeaceTreaty rdfs:subClassOf ies:Treaty . 
ies:PeriodOfTime rdf:type rdfs:Class . 
ies:PeriodOfTime sparx:guid "{3FDFA898-C340-4279-8B3C-275359D5B02D}" . 
ies:PeriodOfTime rdfs:comment "A PeriodOfTime is an Element whose spatial extent is everywhere, but whose temporal extent is limited. " . 
ies:PeriodOfTime rdfs:subClassOf ies:Element . 
ies:permittedNationality rdf:type owl:DatatypeProperty . 
ies:permittedNationality sparx:guid "{FA623989-B6A4-40e2-A956-B8FFEA478895}" . 
ies:permittedNationality rdfs:comment "The nationalities of those who are permitted to access the item. See the EDH specification for further details.Allowable Values:See EDH Standard" . 
ies:permittedNationality rdfs:domain ies:SecurityLabel . 
ies:permittedOrganisation rdf:type owl:DatatypeProperty . 
ies:permittedOrganisation sparx:guid "{90F3E89D-1456-41fe-9354-4E13C4D79564}" . 
ies:permittedOrganisation rdfs:comment "The organisations who are permitted to access the item. See the EDH specification for further details.Allowable Values:See EDH Standard" . 
ies:permittedOrganisation rdfs:domain ies:SecurityLabel . 
ies:Perpetrator rdf:type rdfs:Class . 
ies:Perpetrator sparx:guid "{D625B538-7D72-4d7d-BA50-D79712A264ED}" . 
ies:Perpetrator rdfs:comment "An Actor where the ResponsibleActor conducts a CriminalActivity" . 
ies:Perpetrator rdfs:subClassOf ies:ActiveEventParticipant . 
ies:Person rdf:type rdfs:Class . 
ies:Person sparx:guid "{5D5C5B9B-5E90-4100-8353-8EE9F3D772E2}" . 
ies:Person rdfs:comment "A human being, living or dead. This also includes what may appear to be a person, but is in fact an Alias" . 
ies:Person rdfs:subClassOf ies:ResponsibleActor . 
ies:Person rdfs:subClassOf ies:PersonState . 
ies:PersonalRadioHandset rdf:type rdfs:Class . 
ies:PersonalRadioHandset sparx:guid "{9D84921F-87A3-4ee9-8A3D-A88F564295FA}" . 
ies:PersonalRadioHandset rdfs:comment "A CommunicationsDevice for portable radio communications - e.g. a walkie-talkie" . 
ies:PersonalRadioHandset rdfs:subClassOf ies:CommunicationsDevice . 
ies:PersonHeight rdf:type rdfs:Class . 
ies:PersonHeight sparx:guid "{57060AD9-A6D7-496d-A2BF-22B930400EEE}" . 
ies:PersonHeight rdfs:comment "The Length that is the height of a PersonState" . 
ies:PersonHeight rdfs:subClassOf ies:Length . 
ies:PersonInCommunication rdf:type rdfs:Class . 
ies:PersonInCommunication sparx:guid "{0383D09B-8C40-417d-8C1A-75220EAF496E}" . 
ies:PersonInCommunication rdfs:comment "A PersonState (and an EventParticipant) when a Person is involved in communicating. " . 
ies:PersonInCommunication rdfs:subClassOf ies:EventParticipant . 
ies:PersonInCommunication rdfs:subClassOf ies:PersonState . 
ies:PersonInTransit rdf:type rdfs:Class . 
ies:PersonInTransit sparx:guid "{9888A3F3-7E9B-4806-BD4E-2FC4D87A5902}" . 
ies:PersonInTransit rdfs:comment "An EntityInTransit where the Entity is a Person" . 
ies:PersonInTransit rdfs:subClassOf ies:EntityInTransit . 
ies:PersonName rdf:type rdfs:Class . 
ies:PersonName sparx:guid "{F114F86C-3BA8-4be7-A686-A1D80002DF28}" . 
ies:PersonName rdfs:comment "A Name used to identify / refer to a PersonNote: this is the full name as known to the organisation managing the NamingScheme. For first names, surnames, etc. use a subtype of PersonNameA PersonName may be composed of Surname, GivenName, etc. using the inRepresentation relationship" . 
ies:PersonName rdfs:subClassOf ies:Name . 
ies:PersonState rdf:type rdfs:Class . 
ies:PersonState sparx:guid "{38F8B795-0BCE-4945-8C69-8678ED935C1A}" . 
ies:PersonState rdfs:comment "A temporal state of a Person" . 
ies:PersonState rdfs:subClassOf ies:ResponsibleActorState . 
ies:PersonTitle rdf:type rdfs:Class . 
ies:PersonTitle sparx:guid "{CA36058B-835C-48ef-944A-2507708ADA71}" . 
ies:PersonTitle rdfs:comment "The title associated with the name of the person." . 
ies:PersonTitle rdfs:subClassOf ies:PersonName . 
ies:PlaceName rdf:type rdfs:Class . 
ies:PlaceName sparx:guid "{37DB1A2C-9382-4dac-8AE8-9DEC5A337E16}" . 
ies:PlaceName rdfs:comment "A Name that is used to refer to a Location.Note:  the naming pattern is used here as different parties (even standards bodies !) may have different names for the same Location" . 
ies:PlaceName rdfs:subClassOf ies:Name . 
ies:PointOnEarthSurface rdf:type rdfs:Class . 
ies:PointOnEarthSurface sparx:guid "{A11A426E-ED15-4aaf-B9A5-02A4060533AA}" . 
ies:PointOnEarthSurface rdfs:comment "A Location that is a point (mathematically speaking, of vanishing area) on the surface of the WGS84 spheroid" . 
ies:PointOnEarthSurface rdfs:subClassOf ies:GeoPoint . 
ies:PolicyAnnouncement rdf:type rdfs:Class . 
ies:PolicyAnnouncement sparx:guid "{345E8F46-AC41-452b-B2F9-694DBED556FD}" . 
ies:PolicyAnnouncement rdfs:comment "A PoliticalAnnouncement about policy" . 
ies:PolicyAnnouncement rdfs:subClassOf ies:PoliticalAnnouncement . 
ies:PoliticalAgreement rdf:type rdfs:Class . 
ies:PoliticalAgreement sparx:guid "{686C8BFB-6CB2-4185-9FCF-89D2D4BB3051}" . 
ies:PoliticalAgreement rdfs:comment "A PoliticalEvent that is also an EndToEndAgreementNote: was called Agreement in IES 3.x, but that was confusing for business agreements, personal agreements, etc." . 
ies:PoliticalAgreement rdfs:subClassOf ies:PoliticalEvent . 
ies:PoliticalAgreement rdfs:subClassOf ies:EndToEndAgreement . 
ies:PoliticalAnnouncement rdf:type rdfs:Class . 
ies:PoliticalAnnouncement sparx:guid "{53D5957B-E4B6-4cbb-8CE9-887F7152820F}" . 
ies:PoliticalAnnouncement rdfs:comment "A PoliticalEvent where information is released to the publicNote: was called Announcement in IES 3.x, but that was confusing for business announcements , personal announcements , etc." . 
ies:PoliticalAnnouncement rdfs:subClassOf ies:PoliticalEvent . 
ies:PoliticalEvent rdf:type rdfs:Class . 
ies:PoliticalEvent sparx:guid "{3A0E6FDD-5B3B-4092-9549-C05E8A5FED41}" . 
ies:PoliticalEvent rdfs:comment "An Event related to democratic processes or party politics" . 
ies:PoliticalEvent rdfs:subClassOf ies:Event . 
ies:Port rdf:type rdfs:Class . 
ies:Port sparx:guid "{57860A04-0128-4c7e-9BFD-83D3BA432F8C}" . 
ies:Port rdfs:comment "A Facility which is a recognised terminus for international travel" . 
ies:Port rdfs:subClassOf ies:Facility . 
ies:PossibleWorld rdf:type rdfs:Class . 
ies:PossibleWorld sparx:guid "{15E93B86-6969-47f2-8036-0B7B96E9BDA2}" . 
ies:PossibleWorld rdfs:comment "An Element that encompasses a number of Events, Entities and States that may occur / have occurred. A PossibleWorld is used for scenario planning and forensics.  This is a very simple placeholder for an area of IES that is likely to grow in the future. For now, it can be used to group together a number of elements (using isPartOf relationship) to assert that they share the same truth - i.e. in one possible scenario, all of them were true. The same Element may exist in more than one PossibleWorld - i.e. scenarios may share elements. For version 4.1.0 of IES, PossibleWorld is to be used with AssessToBeTrue in order to specify a level of confidence or probability. More work is needed on this in later IES versions. " . 
ies:PossibleWorld rdfs:subClassOf ies:Element . 
ies:Post rdf:type rdfs:Class . 
ies:Post sparx:guid "{7C28E83C-1895-4901-ABF8-9D78C9C12C62}" . 
ies:Post rdfs:comment "A part of an Organisation that has particular responsibilities" . 
ies:Post rdfs:subClassOf ies:ResponsibleActor . 
ies:Post rdfs:subClassOf ies:PostState . 
ies:PostalCode rdf:type rdfs:Class . 
ies:PostalCode sparx:guid "{6A0385E2-3FB1-4a42-A254-BC382D92E27A}" . 
ies:PostalCode rdfs:comment "A GeoIdentity used to (partially) identify and address" . 
ies:PostalCode rdfs:subClassOf ies:GeoIdentity . 
ies:postModificationState rdf:type owl:ObjectProperty . 
ies:postModificationState sparx:guid "{2B02EF33-E12A-42ec-B047-533F6D8F159D}" . 
ies:postModificationState rdfs:comment "A partOf relationship to indicate a State of an Entity just after the Modify eventNote: For BORO purists, this means the post State is part of the Modify Event (i.e. the extent of the Modify Event includes the State)" . 
ies:postModificationState rdfs:subPropertyOf ies:isStateOf . 
ies:postModificationState rdfs:domain ies:Modify . 
ies:postModificationState rdfs:range ies:State . 
ies:PostState rdf:type rdfs:Class . 
ies:PostState sparx:guid "{DB51B007-E3E8-431f-9C23-3C0A7E83FB11}" . 
ies:PostState rdfs:comment "A temporal state of a Post" . 
ies:PostState rdfs:subClassOf ies:ResponsibleActorState . 
ies:powertype rdf:type owl:ObjectProperty . 
ies:powertype sparx:guid "{D4BD48E8-76B8-4d3c-AB83-E653DB89170D}" . 
ies:powertype rdfs:comment "An rdf:type relationship that asserts one Class is the powerset of the other (see Cantors theorem)." . 
ies:powertype rdfs:subPropertyOf rdf:type . 
ies:preModificationState rdf:type owl:ObjectProperty . 
ies:preModificationState sparx:guid "{4E954855-D50A-42ab-9401-4B1C890542AD}" . 
ies:preModificationState rdfs:comment "A partOf relationship to indicate a State of an Entity just prior to the Modify eventNote: For BORO purists, this means the pre State is part of the Modify Event (i.e. the extent of the Modify Event includes the State)" . 
ies:preModificationState rdfs:subPropertyOf ies:isStateOf . 
ies:preModificationState rdfs:domain ies:Modify . 
ies:preModificationState rdfs:range ies:State . 
ies:Presence rdf:type rdfs:Class . 
ies:Presence sparx:guid "{8404464D-3904-4c59-AE0E-B3FAFB46AC4E}" . 
ies:Presence rdfs:comment "An EventParticipant where an Entity is CoLocated with other Entities of interest" . 
ies:Presence rdfs:subClassOf ies:EventParticipant . 
ies:Prisoner rdf:type rdfs:Class . 
ies:Prisoner sparx:guid "{885EA1C2-29D7-4b7c-B479-D43E4F77B5BD}" . 
ies:Prisoner rdfs:comment "A persons role when incarcerated" . 
ies:Prisoner rdfs:subClassOf ies:EventParticipant . 
ies:Prisoner rdfs:subClassOf ies:PersonState . 
ies:Prosecution rdf:type rdfs:Class . 
ies:Prosecution sparx:guid "{024133FE-9D0B-4e5d-A97D-A34B5EA01C41}" . 
ies:Prosecution rdfs:comment "A LawEnforcement Event that is the trial of a suspect" . 
ies:Prosecution rdfs:subClassOf ies:LawEnforcement . 
ies:Prosecutor rdf:type rdfs:Class . 
ies:Prosecutor sparx:guid "{ABDC5FD5-3281-4cd5-A9B0-188292D8C6B7}" . 
ies:Prosecutor rdfs:comment "A persons role as a prosecutor in a trial" . 
ies:Prosecutor rdfs:subClassOf ies:ActiveEventParticipant . 
ies:Prosecutor rdfs:subClassOf ies:ResponsibleActorState . 
ies:protectiveMarking rdf:type owl:DatatypeProperty . 
ies:protectiveMarking sparx:guid "{7E5590F8-B142-49d8-8FB0-414716CF9F16}" . 
ies:protectiveMarking rdfs:comment "The classification applied to the respective item. This is equivalent to the Classification field within the EDHAllowable Values:OFFICIALOFFICIAL-SENSITIVESECRETTOP SECRET" . 
ies:protectiveMarking rdfs:domain ies:SecurityLabel . 
ies:publicationDate rdf:type owl:ObjectProperty . 
ies:publicationDate sparx:guid "{CD6E380B-7AD4-43d6-A128-9C666ABD8223}" . 
ies:publicationDate rdfs:comment "The date of publication of the respective document." . 
ies:publicationDate rdfs:subPropertyOf ies:relationship . 
ies:publicationDate rdfs:domain ies:WorkOfDocumentation . 
ies:publicationDate rdfs:range ies:ParticularPeriod . 
ies:Purchase rdf:type rdfs:Class . 
ies:Purchase sparx:guid "{0A9A9F7D-A6F1-4629-BD2B-7990D2D36493}" . 
ies:Purchase rdfs:comment "A TradeEvent where an Entity is bought" . 
ies:Purchase rdfs:subClassOf ies:TradeEvent . 
ies:Purchaser rdf:type rdfs:Class . 
ies:Purchaser sparx:guid "{B10A694D-31AA-456c-8C51-B7B5F101A39F}" . 
ies:Purchaser rdfs:comment "An EventParticipant where a ResponsibleActor participates in a TradeEvent as a purchaserNote: in the case of a RequestForQuotation, the purchaser is the person or organisation issuing the RfQNote: in the case of an online purchase where the buyer is unknown, the participant may be an OnlineIdentifier" . 
ies:Purchaser rdfs:subClassOf ies:EventParticipant . 
ies:quantityDelivered rdf:type owl:DatatypeProperty . 
ies:quantityDelivered sparx:guid "{7550DA0F-DF0E-4c61-9198-5DE767677A3A}" . 
ies:quantityDelivered rdfs:comment "The number of Entities (of the same type) that were delivered" . 
ies:quantityDelivered rdfs:subPropertyOf ies:attribute . 
ies:quantityDelivered rdfs:domain ies:Delivery . 
ies:quantityOffered rdf:type owl:DatatypeProperty . 
ies:quantityOffered sparx:guid "{AEC476A1-AE39-4a9e-9EE3-DD45B50B0F26}" . 
ies:quantityOffered rdfs:comment "The number of Entities (of the same type) that are being offered for sale" . 
ies:quantityOffered rdfs:subPropertyOf ies:attribute . 
ies:quantityOffered rdfs:domain ies:OfferForSale . 
ies:quantityPurchased rdf:type owl:DatatypeProperty . 
ies:quantityPurchased sparx:guid "{0D2231E8-6AF1-4e59-B8FA-86A26334CC71}" . 
ies:quantityPurchased rdfs:comment "The number of Entities (of the same type) that were purchased" . 
ies:quantityPurchased rdfs:subPropertyOf ies:attribute . 
ies:quantityPurchased rdfs:domain ies:Purchase . 
ies:radioCoverage rdf:type owl:ObjectProperty . 
ies:radioCoverage sparx:guid "{3B5E5043-30C2-4e67-86C8-F59F55AEBA90}" . 
ies:radioCoverage rdfs:comment "A relationship linking a RadioMast to its RadioCoverageArea" . 
ies:radioCoverage rdfs:subPropertyOf ies:relationship . 
ies:radioCoverage rdfs:domain ies:RadioMast . 
ies:radioCoverage rdfs:range ies:RadioCoverageArea . 
ies:RadioCoverageArea rdf:type rdfs:Class . 
ies:RadioCoverageArea sparx:guid "{7A2CC7C7-6B82-4751-BDBE-A770B3AFBBEB}" . 
ies:RadioCoverageArea rdfs:comment "A Location whose area is that in which a RadioMast hast viable communications coverage.Note: The RadioMast itself may not be part of this area, as often the immediate area around the base of a RadioMast is a deadspot. Note: Most radio area coverage is complex in shape, and the preferred representation in IES4 is GeoJSON. No attempt is made here to differentiate between signal strength zones. To do this, create multople RadioCoverAreas for the same RadioMast and label them appropriately. " . 
ies:RadioCoverageArea rdfs:subClassOf ies:Location . 
ies:RadioCoverageArea rdfs:subClassOf ies:Asset . 
ies:RadioMast rdf:type rdfs:Class . 
ies:RadioMast sparx:guid "{F02CFF55-12A7-4308-9A60-E2353DE5BE58}" . 
ies:RadioMast rdfs:comment "An Device that is placed in a Location to provide either a link from a wired to wireless connection, or to relay between two wireless endpoints." . 
ies:RadioMast rdfs:subClassOf ies:Device . 
ies:RadioMast rdfs:subClassOf ies:SystemState . 
ies:Ratification rdf:type rdfs:Class . 
ies:Ratification sparx:guid "{31977608-5432-4d6f-AEE0-19838197C813}" . 
ies:Ratification rdfs:comment "An AgreementStage where parties have arrived at a consensus and approve the agreement" . 
ies:Ratification rdfs:subClassOf ies:AgreementStage . 
ies:RealEstate rdf:type rdfs:Class . 
ies:RealEstate sparx:guid "{8E0DF17F-34EE-43c6-8DA4-30F698384FD3}" . 
ies:RealEstate rdfs:comment "A Location (and an Asset) that has been defined or constructed for the purpose of ownership" . 
ies:RealEstate rdfs:subClassOf ies:Location . 
ies:RealEstate rdfs:subClassOf ies:Asset . 
ies:ReceivingAccount rdf:type rdfs:Class . 
ies:ReceivingAccount sparx:guid "{25965198-3FE0-4bb9-BCA9-808E15A3EE49}" . 
ies:ReceivingAccount rdfs:comment "An EventParticipant where a FinancialAccount receives money" . 
ies:ReceivingAccount rdfs:subClassOf ies:EventParticipant . 
ies:Recipient rdf:type rdfs:Class . 
ies:Recipient sparx:guid "{AAC709FB-0B88-4517-B5BB-FE2320992073}" . 
ies:Recipient rdfs:comment "An PartyInCommunication where the communicating party is the recipient of a message" . 
ies:Recipient rdfs:subClassOf ies:PartyInCommunication . 
ies:Reconnaisance rdf:type rdfs:Class . 
ies:Reconnaisance sparx:guid "{88E8F5E6-AFE5-4376-8112-EC294A673923}" . 
ies:Reconnaisance rdfs:comment "An IntelligenceOperation where an Entity or Event is observed for the purposes of planning" . 
ies:Reconnaisance rdfs:subClassOf ies:IntelligenceOperation . 
ies:recurrentPeriodRepresentation rdf:type owl:DatatypeProperty . 
ies:recurrentPeriodRepresentation sparx:guid "{442AC7F0-AE57-4090-88D6-55A3825ECEAA}" . 
ies:recurrentPeriodRepresentation rdfs:comment "A modified ISO8601 format (hence use of xsd:string) where elements of the time/date are blanked with ?? characters. The purpose of this is to be able to specify e.g.  a time of day with no date - i.e. all recurrences of that time of day." . 
ies:recurrentPeriodRepresentation rdfs:subPropertyOf ies:attribute . 
ies:recurrentPeriodRepresentation rdfs:domain ies:RecurringPeriod . 
ies:RecurringPeriod rdf:type rdfs:Class . 
ies:RecurringPeriod sparx:guid "{986E66AC-9092-410b-88AD-30B86EFC32DD}" . 
ies:RecurringPeriod rdfs:comment "A PeriodOfTime that is composed of regularly recurring periods of time.ISO8601 is used to represent these periods (recurrentPeriod property), using the blanking technique (e.g. blanking the date to give a daily time). The recurrence can be limited using the recurringFrom and recurringUntil properties Examples:Every Tuesday from 28th August 2018 to 2 October 201813:00 to 14:00 on every day from 27th June 2016 to 2 October 2024" . 
ies:RecurringPeriod rdfs:subClassOf ies:ArbitraryPeriod . 
ies:ReferenceNumber rdf:type rdfs:Class . 
ies:ReferenceNumber sparx:guid "{A0DC70DD-9237-480b-A712-F5381C5FFA1A}" . 
ies:ReferenceNumber rdfs:comment "An Identifier used to uniquely identity a document." . 
ies:ReferenceNumber rdfs:subClassOf ies:Identifier . 
ies:RegionalConstituency rdf:type rdfs:Class . 
ies:RegionalConstituency sparx:guid "{FC55D479-07C4-4d98-B48C-5032190E493D}" . 
ies:RegionalConstituency rdfs:comment "The people residing (or entitled to reside / vote in) a particular Location." . 
ies:RegionalConstituency rdfs:subClassOf ies:Organisation . 
ies:regionCountry rdf:type owl:ObjectProperty . 
ies:regionCountry sparx:guid "{B3B6D7F3-F5B0-49d6-886F-F5AF7C56F041}" . 
ies:regionCountry rdfs:comment "An inLocation relationship to indicate a RegionOfCountry is in a Country" . 
ies:regionCountry rdfs:subPropertyOf ies:inLocation . 
ies:regionCountry rdfs:range ies:Country . 
ies:regionCountry rdfs:domain ies:RegionOfCountry . 
ies:RegionOfCountry rdf:type rdfs:Class . 
ies:RegionOfCountry sparx:guid "{65D869DB-19EE-4886-98BA-E579C39C4A68}" . 
ies:RegionOfCountry rdfs:comment "A Location that is a general subdivision of a Countrye.g. cities, towns, counties, states, etc." . 
ies:RegionOfCountry rdfs:subClassOf ies:Location . 
ies:RegionOfWorld rdf:type rdfs:Class . 
ies:RegionOfWorld sparx:guid "{18C405CE-CC09-4e02-A44D-0FB00C6F6B37}" . 
ies:RegionOfWorld rdfs:comment "A Location that is a general subdivision of the world - e.g. continents, sub-continents, economic areas, etc.Regions of the world may sometimes be spatially separated (e.g. economic areas)" . 
ies:RegionOfWorld rdfs:subClassOf ies:Location . 
ies:RegistrationNumber rdf:type rdfs:Class . 
ies:RegistrationNumber sparx:guid "{1E784B9C-1A5D-4035-B134-67A758FB869D}" . 
ies:RegistrationNumber rdfs:comment "The registration number for the respective Vehicle (with or without spaces).For road vehicles this is often referred to as the VRN (vehicle registration number).For aircraft the tail number is often used as a means of identification and/or registration." . 
ies:RegistrationNumber rdfs:subClassOf ies:Identifier . 
ies:relationship rdf:type owl:ObjectProperty . 
ies:relationship sparx:guid "{DCE662F5-7BDB-457e-AE7E-2E5FE43DBA1A}" . 
ies:relationship rdfs:comment "A relationship represents an association between two Entities" . 
ies:relationship rdfs:range ies:ExchangedItem . 
ies:relationship rdfs:domain ies:ExchangedItem . 
ies:Religion rdf:type rdfs:Class . 
ies:Religion sparx:guid "{BD538820-CE91-4b9a-ADB8-C105FE0F2E7B}" . 
ies:Religion rdfs:comment "An Entity whose extent is all the people (PersonState) who share the same belief.Religions may be part of other religions - e.g. Christianity being made up of Catholic, Protestant, Orthodox, etc. 1. The religion �practiced� by the respective Person..2. The religion may be qualified to identity a particular sect.3. The Metropolitan Police standard [F] shall be used as the reference data standard" . 
ies:Religion rdfs:subClassOf ies:Entity . 
ies:Religion rdfs:subClassOf ies:ReligionState . 
ies:ReligionState rdf:type rdfs:Class . 
ies:ReligionState sparx:guid "{E7B02F98-C52E-4db0-AF32-3D5131710EE7}" . 
ies:ReligionState rdfs:comment "A temporal state of an Religion" . 
ies:ReligionState rdfs:subClassOf ies:State . 
ies:ReligiousOrganisation rdf:type rdfs:Class . 
ies:ReligiousOrganisation sparx:guid "{2978340B-C4AA-4331-A68D-54A158798DAC}" . 
ies:ReligiousOrganisation rdfs:comment "An Organisation formed around a particular religious belief" . 
ies:ReligiousOrganisation rdfs:subClassOf ies:Organisation . 
ies:RentalAgreement rdf:type rdfs:Class . 
ies:RentalAgreement sparx:guid "{F38D2E58-C29A-4e3c-93BF-C33800969720}" . 
ies:RentalAgreement rdfs:comment "An EndToEndAgreement where one Party rents an Entity to another" . 
ies:RentalAgreement rdfs:subClassOf ies:EndToEndAgreement . 
ies:RentalProvider rdf:type rdfs:Class . 
ies:RentalProvider sparx:guid "{8ECC64A4-CED0-4122-AB54-64EA870837FC}" . 
ies:RentalProvider rdfs:comment "A PartyToAgreement where a ResponsibleActor provides an Entity to rent" . 
ies:RentalProvider rdfs:subClassOf ies:PartyToAgreement . 
ies:Rented rdf:type rdfs:Class . 
ies:Rented sparx:guid "{E5C65CAB-65BE-4502-8B46-5C5CC3C73B00}" . 
ies:Rented rdfs:comment "An EventParticipant where an Entity is rented" . 
ies:Rented rdfs:subClassOf ies:EventParticipant . 
ies:Renter rdf:type rdfs:Class . 
ies:Renter sparx:guid "{E2FC3A09-EC9D-4ab9-B273-A526CB511B5A}" . 
ies:Renter rdfs:comment "A PartyToAgreement where a ResponsibleActor rents an Entity from another party" . 
ies:Renter rdfs:subClassOf ies:PartyToAgreement . 
ies:Report rdf:type rdfs:Class . 
ies:Report sparx:guid "{8D510CB0-C9BF-4de3-A442-9070ABB15732}" . 
ies:Report rdfs:comment "A WorkOfDocumentation that offers one or more persons view on a particular topic. " . 
ies:Report rdfs:subClassOf ies:WorkOfDocumentation . 
ies:Representation rdf:type rdfs:Class . 
ies:Representation sparx:guid "{675A5C23-0746-43d0-96D0-AF0DF72CD697}" . 
ies:Representation rdfs:comment "An ClassOfEntity whose instances are representations of things in the real worldExamples:* an identifier used for a Person* a document (though not an individual copy of a document)" . 
ies:Representation rdfs:subClassOf ies:ClassOfEntity . 
ies:representationValue rdf:type owl:DatatypeProperty . 
ies:representationValue sparx:guid "{AE00F1DE-F42B-4fc0-B07B-21F754F16FD4}" . 
ies:representationValue rdfs:comment "The examplar text, number, etc. of a Representation" . 
ies:representationValue rdfs:subPropertyOf ies:attribute . 
ies:representationValue rdfs:domain ies:Representation . 
ies:RequestDocument rdf:type rdfs:Class . 
ies:RequestDocument sparx:guid "{C0273975-049B-40f0-817C-DFBFA4A3E5CE}" . 
ies:RequestDocument rdfs:comment "A WorkOfDocumentation that requests permission" . 
ies:RequestDocument rdfs:subClassOf ies:WorkOfDocumentation . 
ies:requestedActivityType rdf:type owl:ObjectProperty . 
ies:requestedActivityType sparx:guid "{132AFC03-7A64-45fa-9F87-93171BBFBE3D}" . 
ies:requestedActivityType rdfs:comment "A relationship linking an AuthorisationRequest to a AuthorisedEventClass that the request requires authorisation to do.For example, someone making request authorisation to travel" . 
ies:requestedActivityType rdfs:subPropertyOf ies:relationship . 
ies:requestedActivityType rdfs:range ies:AuthorisedEventClass . 
ies:requestedActivityType rdfs:domain ies:AuthorisationRequest . 
ies:RequestForQuotation rdf:type rdfs:Class . 
ies:RequestForQuotation sparx:guid "{300203EC-607A-4d77-AE6F-7EAE7FA44DF2}" . 
ies:RequestForQuotation rdfs:comment "A TradeEvent where one or more Entities are is required" . 
ies:RequestForQuotation rdfs:subClassOf ies:TradeEvent . 
ies:Reservation rdf:type rdfs:Class . 
ies:Reservation sparx:guid "{CDF94674-D458-4996-9A99-6CBFFF3907EB}" . 
ies:Reservation rdfs:comment "Rights where the rights holder has reserved some future event - e.g. hotel reservation, travel reservation, delivery, etc." . 
ies:Reservation rdfs:subClassOf ies:Rights . 
ies:residesIn rdf:type owl:ObjectProperty . 
ies:residesIn sparx:guid "{6BC3DDD8-477E-4c8a-B85D-E637CF9DB6DF}" . 
ies:residesIn rdfs:comment "A Relationship between a ResponsibleActorState and a Location at which they registered as a resident.Note this is legal / administrative construct. See also StaysAt" . 
ies:residesIn rdfs:subPropertyOf ies:relationship . 
ies:residesIn rdfs:domain ies:ResponsibleActorState . 
ies:residesIn rdfs:range ies:Location . 
ies:respectfulOf rdf:type owl:ObjectProperty . 
ies:respectfulOf sparx:guid "{EEBCE0A4-4882-4c95-9C2D-93CE5EB7A275}" . 
ies:respectfulOf rdfs:comment "A Relationship between two ResponsibleActor Entities where one respects the other.Note: this should not be considered a bi-directional relationship. Just because one person respects another person does not necessarily mean the feeling is reciprocated. " . 
ies:respectfulOf rdfs:subPropertyOf ies:relationship . 
ies:respectfulOf rdfs:range ies:ResponsibleActor . 
ies:respectfulOf rdfs:domain ies:ResponsibleActorState . 
ies:ResponsibleActor rdf:type rdfs:Class . 
ies:ResponsibleActor sparx:guid "{D09EDE21-E862-4ec1-BC0F-045CCE5454A9}" . 
ies:ResponsibleActor rdfs:comment "An Actor that can be held legally responsible for their actions - generally a Person or an Organisation. This also includes Posts which may be filled by people or organisations.Note: there are many situations (mostly due to the law) where a Person or Organisation can be the subject of a relationship or Event interchangeably. Hence the need for a parent class in the IES ontology. " . 
ies:ResponsibleActor rdfs:subClassOf ies:Actor . 
ies:ResponsibleActor rdfs:subClassOf ies:ResponsibleActorState . 
ies:ResponsibleActor ies:powertype ies:ClassOfResponsibleActor . 
ies:ResponsibleActorState rdf:type rdfs:Class . 
ies:ResponsibleActorState sparx:guid "{100B93CD-937E-4fdd-8851-02D1DC07F5B6}" . 
ies:ResponsibleActorState rdfs:comment "A temporal state of a ResponsibleActorNote:  this is the superclass of ResponsibleActor (the whole life person or organisation) because the whole-life state is just a special case of a ResponsibleActorState. This pattern is true for all states. " . 
ies:ResponsibleActorState rdfs:subClassOf ies:ActorState . 
ies:Retailer rdf:type rdfs:Class . 
ies:Retailer sparx:guid "{BA2472AB-56F0-462e-9460-F0192ABCD979}" . 
ies:Retailer rdfs:comment "An EventParticipant where a ResponsibleActor participates in a TradeEvent as a retailer" . 
ies:Retailer rdfs:subClassOf ies:Supplier . 
ies:Rights rdf:type rdfs:Class . 
ies:Rights sparx:guid "{487778E0-4BD7-4d9a-B7F7-63731478E1A2}" . 
ies:Rights rdfs:comment "An Asset which encompasses the legal rights to an Element Strictly speaking, all property (therefore most Assets) are a question of rights. No-one actually owns something, they have a legal right of that thing. In most cases, we can deal with this just using Asset. However in more complex cases, rights can be bought and sold (and of course owned) to things which arent generally viewed as assets - e.g. paying a delivery cost, owning the leasehold to a property, etc. Examples:* The performance rights to a Song* The rights to purchase currency at a pre-agreed rate in the future" . 
ies:Rights rdfs:subClassOf ies:Asset . 
ies:rightsTo rdf:type owl:ObjectProperty . 
ies:rightsTo sparx:guid "{04A80EF0-8E34-4bdb-8A8E-31D89028F9B6}" . 
ies:rightsTo rdfs:comment "A Relationship between Rights and the Element to which the Rights apply Example:* Rights to travel on a particular service (a travel reservation)* Rights to a parcel of land" . 
ies:rightsTo rdfs:subPropertyOf ies:relationship . 
ies:rightsTo rdfs:domain ies:Rights . 
ies:rightsTo rdfs:range ies:Element . 
ies:RoadVehicle rdf:type rdfs:Class . 
ies:RoadVehicle sparx:guid "{830B2164-E880-4bef-A62C-B38CEB6A824D}" . 
ies:RoadVehicle rdfs:comment "A Vehicle that travels by road (surprisingly enough)" . 
ies:RoadVehicle rdfs:subClassOf ies:Vehicle . 
ies:Role rdf:type rdfs:Class . 
ies:Role sparx:guid "{0066A327-D497-42e0-9F50-D988F522F4A5}" . 
ies:Role rdfs:comment "An ClassOfState that is the role an Entity has in context (as part of) an Element- e.g. Manager, " . 
ies:Role rdfs:subClassOf ies:ClassOfState . 
ies:RoomNumber rdf:type rdfs:Class . 
ies:RoomNumber sparx:guid "{0B2564A8-9A95-4164-BB49-01900DD530AD}" . 
ies:RoomNumber rdfs:comment "A GeoIdentity used to identify a PartOfFacility" . 
ies:RoomNumber rdfs:subClassOf ies:GeoIdentity . 
ies:Sailing rdf:type rdfs:Class . 
ies:Sailing sparx:guid "{803AF0E7-01EC-4123-B888-3FB6369C840F}" . 
ies:Sailing rdfs:comment "A TravelService by sea" . 
ies:Sailing rdfs:subClassOf ies:Transit . 
ies:SatellitePhoneHandset rdf:type rdfs:Class . 
ies:SatellitePhoneHandset sparx:guid "{3634DBF3-AA3A-402e-9D08-906C06FAFEDB}" . 
ies:SatellitePhoneHandset rdfs:comment "A CommunicationsDevice that communicates via satellite. " . 
ies:SatellitePhoneHandset rdfs:subClassOf ies:CommunicationsDevice . 
ies:scheduledArrivalPort rdf:type owl:ObjectProperty . 
ies:scheduledArrivalPort sparx:guid "{6BC73189-2B25-4e1c-A935-EDA8106F3EB3}" . 
ies:scheduledArrivalPort rdfs:comment "The Port from which the TravelService is scheduled to arrive" . 
ies:scheduledArrivalPort rdfs:subPropertyOf ies:relationship . 
ies:scheduledArrivalPort rdfs:domain ies:TravelService . 
ies:scheduledArrivalPort rdfs:range ies:Port . 
ies:scheduledArrivalTime rdf:type owl:DatatypeProperty . 
ies:scheduledArrivalTime sparx:guid "{DB3878D9-FF24-4069-A8DD-C24F5D074C0C}" . 
ies:scheduledArrivalTime rdfs:comment "The date/time on which the service was scheduled to arriveThe format of this attribute is a restricted string based upon the ISO 8601 Extended Format." . 
ies:scheduledArrivalTime rdfs:subPropertyOf ies:attribute . 
ies:scheduledArrivalTime rdfs:domain ies:TravelService . 
ies:scheduledDeparturePort rdf:type owl:ObjectProperty . 
ies:scheduledDeparturePort sparx:guid "{1312D263-F609-4df3-A1DB-AA0557B3B94B}" . 
ies:scheduledDeparturePort rdfs:comment "The Port from which the TravelService is scheduled to depart" . 
ies:scheduledDeparturePort rdfs:subPropertyOf ies:relationship . 
ies:scheduledDeparturePort rdfs:domain ies:TravelService . 
ies:scheduledDeparturePort rdfs:range ies:Port . 
ies:scheduledDepartureTime rdf:type owl:DatatypeProperty . 
ies:scheduledDepartureTime sparx:guid "{340CF0CC-BA75-40b7-8B8A-167CD65C1830}" . 
ies:scheduledDepartureTime rdfs:comment "The date/time on which the service was scheduled to departThe format of this attribute is a restricted string based upon the ISO 8601 Extended Format." . 
ies:scheduledDepartureTime rdfs:subPropertyOf ies:attribute . 
ies:scheduledDepartureTime rdfs:domain ies:TravelService . 
ies:SchemaObject rdf:type rdfs:Class . 
ies:SchemaObject sparx:guid "{D3375BB5-6773-40e1-8CA2-B393DD02B98C}" . 
ies:SchemaObject rdfs:comment "A DataObject that is a standardised plan or outline for something.e.g. Bristol City Street Furniture Schema" . 
ies:SchemaObject rdfs:subClassOf ies:DataObject . 
ies:schemeMasteredIn rdf:type owl:ObjectProperty . 
ies:schemeMasteredIn sparx:guid "{C2C5FF87-189C-478a-B3BF-4706D798087F}" . 
ies:schemeMasteredIn rdfs:comment "A relationship that asserts a NamingScheme is owned by a System that is the master for its names / identifiers - i.e. the uniqueness of the name/identifier is limited to the system." . 
ies:schemeMasteredIn rdfs:subPropertyOf ies:relationship . 
ies:schemeMasteredIn rdfs:domain ies:NamingScheme . 
ies:schemeMasteredIn rdfs:range ies:System . 
ies:schemeOwner rdf:type owl:ObjectProperty . 
ies:schemeOwner sparx:guid "{8D42B4A8-30D3-459d-A729-F5C8FE16D418}" . 
ies:schemeOwner rdfs:comment "A relationship that asserts a RepresentationScheme is governed and used by a ResponsibleActor " . 
ies:schemeOwner rdfs:subPropertyOf ies:relationship . 
ies:schemeOwner rdfs:range ies:ResponsibleActor . 
ies:schemeOwner rdfs:domain ies:NamingScheme . 
ies:ScreenName rdf:type rdfs:Class . 
ies:ScreenName sparx:guid "{8C1321B7-8686-4a21-B99A-6C4A98B411A7}" . 
ies:ScreenName rdfs:comment "A display Name used by the account which may be non-unique, and may not be the same as the username" . 
ies:ScreenName rdfs:subClassOf ies:Name . 
ies:SeatNumber rdf:type rdfs:Class . 
ies:SeatNumber sparx:guid "{03D1711E-F9A7-41b1-B82F-B442FDF82EBF}" . 
ies:SeatNumber rdfs:comment "The number of the seat that the Passenger should be travelling in. Whilst this partially identifies the Passenger, there is no guarantee that people have not swapped seats. " . 
ies:SeatNumber rdfs:subClassOf ies:Identifier . 
ies:SecurityLabel rdf:type rdfs:Class . 
ies:SecurityLabel sparx:guid "{CED628E4-8641-486b-BCD7-CB4E147E7AE6}" . 
ies:SecurityLabel rdfs:comment "A SecurityLabel may be assigned at the statement (triple) level or to the entire ExchangePayload. They provide a mechanism to specify access restrictions and handling instructions for specific triples.Note: In any given IES exchange, a SecurityLabel must be applied to the ExchangePayload. Individual SecurityLabels at the statement level are used to indicate where individual statements deviate from the overall payload SecurityLabel" . 
ies:Sender rdf:type rdfs:Class . 
ies:Sender sparx:guid "{44C93DB5-8DFA-4585-9060-EEC789E0A5AC}" . 
ies:Sender rdfs:comment "An PartyInCommunication where the communicating party is the sender of a message" . 
ies:Sender rdfs:subClassOf ies:PartyInCommunication . 
ies:SendingAccount rdf:type rdfs:Class . 
ies:SendingAccount sparx:guid "{F7172876-85F6-4d29-B11F-A1B36616416A}" . 
ies:SendingAccount rdfs:comment "An EventParticipant where a FinancialAccount sends money" . 
ies:SendingAccount rdfs:subClassOf ies:EventParticipant . 
ies:SerialNumber rdf:type rdfs:Class . 
ies:SerialNumber sparx:guid "{51F79BC9-9BB5-47d6-973B-6F86F289B5FB}" . 
ies:SerialNumber rdfs:comment "An Identifier for Device that has been assigned at manufacture.Example Value:123ABC456DEF" . 
ies:SerialNumber rdfs:subClassOf ies:Identifier . 
ies:ServiceName rdf:type rdfs:Class . 
ies:ServiceName sparx:guid "{8F8428BA-8586-4e34-9C75-FBA7A647B8EA}" . 
ies:ServiceName rdfs:comment "The Name of the OnlineServiceThis should not be confused with a webpage (see the Webpage entity type). The Online Service may be provided via a webpage." . 
ies:ServiceName rdfs:subClassOf ies:Name . 
ies:ServiceProvider rdf:type rdfs:Class . 
ies:ServiceProvider sparx:guid "{496683C9-EB89-46ac-87D0-4864F1B54ED4}" . 
ies:ServiceProvider rdfs:comment "The role of an Organisation in providing a Service (e.g. a TeleConference)" . 
ies:ServiceProvider rdfs:subClassOf ies:EventParticipant . 
ies:Ship rdf:type rdfs:Class . 
ies:Ship sparx:guid "{14098560-1FF3-4599-B9A5-41167861538B}" . 
ies:Ship rdfs:comment "A Vehicle that travels on water" . 
ies:Ship rdfs:subClassOf ies:Vehicle . 
ies:siblingOf rdf:type owl:ObjectProperty . 
ies:siblingOf sparx:guid "{A0D40C4F-B513-4c9f-8D4A-79D0FA7CEF50}" . 
ies:siblingOf rdfs:comment "A Relationship between two Person Entities that indicates one is the sibling of the other" . 
ies:siblingOf rdfs:subPropertyOf ies:familiallyRelatedTo . 
ies:siblingOf rdfs:domain ies:Person . 
ies:siblingOf rdfs:range ies:Person . 
ies:Signatory rdf:type rdfs:Class . 
ies:Signatory sparx:guid "{C55A12C9-CF85-4b7c-B422-1D41054E9570}" . 
ies:Signatory rdfs:comment "An EventParticipant where a ResponsibleActor ratifies an agreement" . 
ies:Signatory rdfs:subClassOf ies:ActiveEventParticipant . 
ies:SIMCard rdf:type rdfs:Class . 
ies:SIMCard sparx:guid "{3244F6B1-8636-4895-B3B1-283CF057F826}" . 
ies:SIMCard rdfs:comment "A CommunicationsDevice that holds data about a IMSI" . 
ies:SIMCard rdfs:subClassOf ies:CommunicationsDevice . 
ies:SimilarEntities rdf:type rdfs:Class . 
ies:SimilarEntities sparx:guid "{A4B13044-00FD-4868-8147-1A3C9E84DAAB}" . 
ies:SimilarEntities rdfs:comment "An ClassOfEntity whose instances are considered similar" . 
ies:SimilarEntities rdfs:subClassOf ies:ClassOfEntity . 
ies:similarEntity rdf:type owl:ObjectProperty . 
ies:similarEntity sparx:guid "{333E73AD-563F-443c-A9B3-CA122FDF75B9}" . 
ies:similarEntity rdfs:comment "An rdf:type relationship that asserts an Entity is similar to other Entities that are also related to the same SimilarEntities class." . 
ies:similarEntity rdfs:subPropertyOf rdf:type . 
ies:similarEntity rdfs:domain ies:Entity . 
ies:similarEntity rdfs:range ies:SimilarEntities . 
ies:SMS rdf:type rdfs:Class . 
ies:SMS sparx:guid "{4C19E163-710B-4ccb-9F1C-569F8E348BDC}" . 
ies:SMS rdfs:comment "A Message (text and images) sent over a cellular network" . 
ies:SMS rdfs:subClassOf ies:Message . 
ies:socialisesAt rdf:type owl:ObjectProperty . 
ies:socialisesAt sparx:guid "{1D9F0978-EFD2-4e27-9242-219637C574EF}" . 
ies:socialisesAt rdfs:comment "A visits relationship between a ResponsibleActor and a Location they socialise in.Note: more often than not, this will be a statement of occasional socialising, so the instance of the ResponsibleActorState should also be an instance of DiscontinuousState. In rarer occasions, it may be used to highlight a single, continuous visit, but in that case, inLocation would generally be used." . 
ies:socialisesAt rdfs:subPropertyOf ies:visits . 
ies:SocialMediaPage rdf:type rdfs:Class . 
ies:SocialMediaPage sparx:guid "{3DC012C3-E273-4ec2-A462-CEDEB27262C1}" . 
ies:SocialMediaPage rdfs:comment "An OnlineArtefact that is user-created - e.g. a facebook timeline, twitter feed, etc. " . 
ies:SocialMediaPage rdfs:subClassOf ies:OnlineArtefact . 
ies:SocialMediaPost rdf:type rdfs:Class . 
ies:SocialMediaPost sparx:guid "{4B3AE19C-6369-49d0-B7B5-949714FFFC95}" . 
ies:SocialMediaPost rdfs:comment "An OnlineArtefact that is part of a SocialMediaPageNote: the content may be created by a different account to the one which created the SocialMediaPage" . 
ies:SocialMediaPost rdfs:subClassOf ies:OnlineArtefact . 
ies:SocialServicesIdentifier rdf:type rdfs:Class . 
ies:SocialServicesIdentifier sparx:guid "{DF17458A-3BB8-4851-B88A-1E08C2EFA697}" . 
ies:SocialServicesIdentifier rdfs:comment "An NationalIdentityNumber used for managing a citizens access to social servicesIn UK, this would be an NI number, in the US, it would be the social security number" . 
ies:SocialServicesIdentifier rdfs:subClassOf ies:NationalIdentityNumber . 
ies:Software rdf:type rdfs:Class . 
ies:Software sparx:guid "{B6014BB6-FD82-4748-8DFF-65401770515C}" . 
ies:Software rdfs:comment "A ClassOfAsset that is programmatic instructions that control or affect the behaviour of an Asset (usually a Device). Note that Software is a class, as the same Software may be installed in multiple locations." . 
ies:Software rdfs:subClassOf ies:ClassOfAsset . 
ies:spokenLanguage rdf:type owl:ObjectProperty . 
ies:spokenLanguage sparx:guid "{FA149043-EA61-4497-A036-589DA1FD312E}" . 
ies:spokenLanguage rdfs:comment "The language in which someone is proficient" . 
ies:spokenLanguage rdfs:range ies:Language . 
ies:spokenLanguage rdfs:subPropertyOf ies:relationship . 
ies:spokenLanguage rdfs:domain ies:LanguageProficiency . 
ies:Stalking rdf:type rdfs:Class . 
ies:Stalking sparx:guid "{9B232210-27A3-410a-A713-EFDE7922C61C}" . 
ies:Stalking rdfs:comment "A CriminalActivity involving the malicious surveillance of a person, often in threatening manner" . 
ies:Stalking rdfs:subClassOf ies:CriminalActivity . 
ies:StandardMeasure rdf:type rdfs:Class . 
ies:StandardMeasure sparx:guid "{C441DE5B-739A-4a83-BE87-96BC63A530B3}" . 
ies:StandardMeasure rdfs:comment "A Measure specified in the International system of quantities" . 
ies:StandardMeasure rdfs:subClassOf ies:Measure . 
ies:StandardMeasureValue rdf:type rdfs:Class . 
ies:StandardMeasureValue sparx:guid "{773272F0-DBAB-4c47-8E21-01171FC82245}" . 
ies:StandardMeasureValue rdfs:comment "A MeasureValue that is expressed in SI units" . 
ies:StandardMeasureValue rdfs:subClassOf ies:MeasureValue . 
ies:startsIn rdf:type owl:DatatypeProperty . 
ies:startsIn sparx:guid "{861E3D08-3659-489a-B100-0E943CF3F3F0}" . 
ies:startsIn rdfs:comment "An xsd:DateTime for the start of the period" . 
ies:startsIn rdfs:subPropertyOf ies:attribute . 
ies:startsIn rdfs:domain ies:ArbitraryPeriod . 
ies:State rdf:type rdfs:Class . 
ies:State sparx:guid "{47301D66-CBD5-4d10-9481-B66966A3F3A2}" . 
ies:State rdfs:comment "A temporal state of an ElementNote: IES requires that any State must be related to its whole-life Element. In some cases, the identity of the whole-life element may be unknown (or of unknown type) but a whole-life element must still be created and related to the State.Note: When Events are decomposed into temporal parts, those parts are often Events themselves. The exception is when the temporal part is arbitrary (e.g. the 11th second of a meeting) when a State should be used. These are rare though." . 
ies:State rdfs:subClassOf ies:Element . 
ies:State ies:powertype ies:ClassOfState . 
ies:statementLabel rdf:type owl:ObjectProperty . 
ies:statementLabel sparx:guid "{7EC7FCEE-7C60-4233-8938-D6320BD951F2}" . 
ies:statementLabel rdfs:comment "A link from an rdf:Statement (see W3C guidance on RDF reification) to the SecurityLabel that provides the access control for that statement.Note: All exchanges should have a default payloadLabel specified. The use of statementLabel is required when individual statements deviate from the default in terms of their access control." . 
ies:statementLabel rdfs:domain rdf:Statement . 
ies:statementLabel rdfs:range ies:SecurityLabel . 
ies:staysAt rdf:type owl:ObjectProperty . 
ies:staysAt sparx:guid "{90332C00-0188-4773-8A71-F9ED15F5ED33}" . 
ies:staysAt rdfs:comment "A visits relationship between a ResponsibleActor and a Location where the person stays at the Location. This should not be confused with residesIn which is an assertion of legal residence. Note: more often than not, this will be a statement of regular/occasional stays, so the instance of the ResponsibleActorState should also be an instance of DiscontinuousState. In rarer occasions, it may be used to highlight a single, continuous visit, but in that case, inLocation would generally be used." . 
ies:staysAt rdfs:subPropertyOf ies:visits . 
ies:StoreCard rdf:type rdfs:Class . 
ies:StoreCard sparx:guid "{686293F8-123B-478f-9A67-A6074937B528}" . 
ies:StoreCard rdfs:comment "A PaymentArtefact issued by a retail Organisation that can only be used to pay for items supplied by that Organisation. " . 
ies:StoreCard rdfs:subClassOf ies:PaymentArtefact . 
ies:storedIn rdf:type owl:ObjectProperty . 
ies:storedIn sparx:guid "{2E33B6DC-54D5-4e5e-9894-B2801F174B00}" . 
ies:storedIn rdfs:comment "A Relationship between an AssetState and a Location where the Asset is/was stored" . 
ies:storedIn rdfs:subPropertyOf ies:isPartOf . 
ies:storedIn rdfs:domain ies:AssetState . 
ies:storedIn rdfs:range ies:Location . 
ies:strengthOfInterest rdf:type owl:DatatypeProperty . 
ies:strengthOfInterest sparx:guid "{49B3D340-AADC-4fcd-80CC-283AE0FC85DF}" . 
ies:strengthOfInterest rdfs:comment "StrengthOfInterest is used in its most general sense and is limited to the following values:� Weak� Strong� Fanatical" . 
ies:strengthOfInterest rdfs:subPropertyOf ies:attribute . 
ies:strengthOfInterest rdfs:domain ies:Interested . 
ies:SubjectOfInterest rdf:type rdfs:Class . 
ies:SubjectOfInterest sparx:guid "{BFFBC847-AD87-458e-9A86-690D659EB48F}" . 
ies:SubjectOfInterest rdfs:comment "A State during which an Element is of interest to an investigation" . 
ies:SubjectOfInterest rdfs:subClassOf ies:State . 
ies:SubjectOfOperation rdf:type rdfs:Class . 
ies:SubjectOfOperation sparx:guid "{11F2A275-650F-407d-8E86-F99DDEF4AAAF}" . 
ies:SubjectOfOperation rdfs:comment "An EventParticipant where an Entity is the subject of an OperationalEventExamples:* person / organisation under investigation* recond location* subject of surveillance" . 
ies:SubjectOfOperation rdfs:subClassOf ies:EventParticipant . 
ies:successorTo rdf:type owl:ObjectProperty . 
ies:successorTo sparx:guid "{BEC84E4F-F407-4a20-BC68-AD1723A3F860}" . 
ies:successorTo rdfs:comment "An after relationship linking two Elements where one ends and the other comes after as a replacement" . 
ies:successorTo rdfs:subPropertyOf ies:after . 
ies:Summit rdf:type rdfs:Class . 
ies:Summit sparx:guid "{78D65599-BCBB-491a-8C34-75B9F7AB60D5}" . 
ies:Summit rdfs:comment "A PoliticalEvent where senior leaders assemble to discuss and agree policy or treaties" . 
ies:Summit rdfs:subClassOf ies:PoliticalEvent . 
ies:Supplier rdf:type rdfs:Class . 
ies:Supplier sparx:guid "{E4D44720-DBEE-434e-A61E-35FE8B66A4BE}" . 
ies:Supplier rdfs:comment "An EventParticipant where a ResponsibleActor participates in a TradeEvent as a supplier" . 
ies:Supplier rdfs:subClassOf ies:EventParticipant . 
ies:supplierTo rdf:type owl:ObjectProperty . 
ies:supplierTo sparx:guid "{4F013D3F-E237-489a-96D5-5E9E54C6A388}" . 
ies:supplierTo rdfs:comment "A worksFor relationship where the supplier (domain) is contracted to deliver goods or services to client (range)" . 
ies:supplierTo rdfs:subPropertyOf ies:worksFor . 
ies:Surname rdf:type rdfs:Class . 
ies:Surname sparx:guid "{B5A0C08A-39B3-4bd1-9D19-CE87E0F7DEBB}" . 
ies:Surname rdfs:comment "A PersonName that is their inherited or married nameNote:A surname will often be applied to a State of the Person, as names tend to change over time" . 
ies:Surname rdfs:subClassOf ies:PersonName . 
ies:Surveillance rdf:type rdfs:Class . 
ies:Surveillance sparx:guid "{AD0F575E-5C28-4594-B346-50E9F22C2A8E}" . 
ies:Surveillance rdfs:comment "An IntelligenceOperation that involves the continued observation of a Person or Location" . 
ies:Surveillance rdfs:subClassOf ies:IntelligenceOperation . 
ies:SurveillanceWarrant rdf:type rdfs:Class . 
ies:SurveillanceWarrant sparx:guid "{A86EC717-55AF-456c-BEC4-E1BA295D0227}" . 
ies:SurveillanceWarrant rdfs:comment "Relates a Surveillance Event to a Document that is the warrant for the Surveillance" . 
ies:SurveillanceWarrant rdfs:subClassOf ies:EventParticipant . 
ies:System rdf:type rdfs:Class . 
ies:System sparx:guid "{F682A265-1AFE-4287-A9CD-0D4C83F54C52}" . 
ies:System rdfs:comment "An Device  comprising software and hardware brought together for a purpose. The Devices may or may not be removable / replaceable" . 
ies:System rdfs:subClassOf ies:Device . 
ies:System rdfs:subClassOf ies:SystemState . 
ies:SystemState rdf:type rdfs:Class . 
ies:SystemState sparx:guid "{056DDAD3-9315-48a8-8598-3DD4F783C5CF}" . 
ies:SystemState rdfs:comment "A temporal state of a System" . 
ies:SystemState rdfs:subClassOf ies:State . 
ies:takesplaceIn rdf:type owl:ObjectProperty . 
ies:takesplaceIn sparx:guid "{5D13DE13-CAAC-4879-9237-D20A6846F4D8}" . 
ies:takesplaceIn rdfs:comment "An inLocation relationship to indicate an EventParticipant takes place within a Location" . 
ies:takesplaceIn rdfs:subPropertyOf ies:inLocation . 
ies:takesplaceIn rdfs:domain ies:EventParticipant . 
ies:takesplaceIn rdfs:range ies:Location . 
ies:TargetLocation rdf:type rdfs:Class . 
ies:TargetLocation sparx:guid "{9BEF1C80-3823-4611-9349-AA1E11E41BE7}" . 
ies:TargetLocation rdfs:comment "Relates an MilitaryAttack to the location specified for the attack" . 
ies:TargetLocation rdfs:subClassOf ies:EventParticipant . 
ies:Team rdf:type rdfs:Class . 
ies:Team sparx:guid "{7B20EC37-6D66-4cd9-97DF-2A30B324C421}" . 
ies:Team rdfs:comment "An Organisation formed around a particular pursuit or task" . 
ies:Team rdfs:subClassOf ies:Organisation . 
ies:TeleConference rdf:type rdfs:Class . 
ies:TeleConference sparx:guid "{6EAC8930-3D16-4e44-9706-989BDF6564A5}" . 
ies:TeleConference rdfs:comment "An InteractiveCommunication where 2 or more parties communicate using audio" . 
ies:TeleConference rdfs:subClassOf ies:InteractiveCommunication . 
ies:TelephoneAccount rdf:type rdfs:Class . 
ies:TelephoneAccount sparx:guid "{593AE684-C2E9-4e40-A7FD-549BFA64900D}" . 
ies:TelephoneAccount rdfs:comment "A CommunicationsAccount that is used to administer the use of one or more telephone numbers." . 
ies:TelephoneAccount rdfs:subClassOf ies:CommunicationsAccount . 
ies:TelephoneCountryCode rdf:type rdfs:Class . 
ies:TelephoneCountryCode sparx:guid "{79C84EC1-83EC-45a8-A3CE-F88CFFBF9434}" . 
ies:TelephoneCountryCode rdfs:comment "The dialing code for a country as specified by the ITU" . 
ies:TelephoneCountryCode rdfs:subClassOf ies:CommunicationsIdentifier . 
ies:TelephoneNumber rdf:type rdfs:Class . 
ies:TelephoneNumber sparx:guid "{168D7B01-CD70-4f83-A414-19B6ABEB961C}" . 
ies:TelephoneNumber rdfs:comment "A CommunicationsIdentifier that enables calls to be directed to particular handset" . 
ies:TelephoneNumber rdfs:subClassOf ies:CommunicationsIdentifier . 
ies:TelephoneNumberRange rdf:type rdfs:Class . 
ies:TelephoneNumberRange sparx:guid "{007F88AD-9CDF-4aa1-BE73-18C688DA8C05}" . 
ies:TelephoneNumberRange rdfs:comment "A CommunicationsIdentifierRange of TelehoneNumbers" . 
ies:TelephoneNumberRange rdfs:subClassOf ies:CommunicationsIdentifierRange . 
ies:Temperature rdf:type rdfs:Class . 
ies:Temperature sparx:guid "{3FEB0BB0-F127-431a-B117-CC986B11D61A}" . 
ies:Temperature rdfs:comment "The Measure of the thermodynamic temperature of an Element" . 
ies:Temperature rdfs:subClassOf ies:StandardMeasure . 
ies:Tendency rdf:type rdfs:Class . 
ies:Tendency sparx:guid "{2B451601-EC1D-4bd4-A782-6E0B7E0D416D}" . 
ies:Tendency rdfs:comment "A DispositionalClass where all the instances share the same tendencyExample: People who tend to violence" . 
ies:Tendency rdfs:subClassOf ies:DispositionalClass . 
ies:TerrorAttack rdf:type rdfs:Class . 
ies:TerrorAttack sparx:guid "{F8454637-80DD-44a7-AD91-6DECE44F0171}" . 
ies:TerrorAttack rdfs:comment "A CriminalActivity that is politically motivated and designed to cause terror" . 
ies:TerrorAttack rdfs:subClassOf ies:CriminalActivity . 
ies:TerroristOrganisation rdf:type rdfs:Class . 
ies:TerroristOrganisation sparx:guid "{6467A4EF-46BA-401c-A5C7-668BAFB6E228}" . 
ies:TerroristOrganisation rdfs:comment "An OrganisationState that is assessed to be conducting acts of terror to achieve a political or religious goal." . 
ies:TerroristOrganisation rdfs:subClassOf ies:OrganisationState . 
ies:TheatreTicket rdf:type rdfs:Class . 
ies:TheatreTicket sparx:guid "{5CD50268-582A-426b-B4CC-F6EE308B84A3}" . 
ies:TheatreTicket rdfs:comment "An EntertainmentTicket for a theatre show" . 
ies:TheatreTicket rdfs:subClassOf ies:EntertainmentTicket . 
ies:Ticket rdf:type rdfs:Class . 
ies:Ticket sparx:guid "{0BC61540-2AFB-42e6-A845-79771EE0268D}" . 
ies:Ticket rdfs:comment "Documented authority (paid-for or otherwise) entitling the bearer to some specified activity." . 
ies:Ticket rdfs:subClassOf ies:IndividualDocument . 
ies:ticketArrivalLocation rdf:type owl:ObjectProperty . 
ies:ticketArrivalLocation sparx:guid "{A4906B5E-8718-404e-8EEF-20AE29106383}" . 
ies:ticketArrivalLocation rdfs:comment "The arrival location as stated on the ticket." . 
ies:ticketArrivalLocation rdfs:subPropertyOf ies:relationship . 
ies:ticketArrivalLocation rdfs:range ies:Port . 
ies:ticketArrivalLocation rdfs:domain ies:TravelTicket . 
ies:ticketDepartureLocation rdf:type owl:ObjectProperty . 
ies:ticketDepartureLocation sparx:guid "{952E5981-257F-429e-9F22-8D2E3B9282C7}" . 
ies:ticketDepartureLocation rdfs:comment "The departure location as stated on the ticket." . 
ies:ticketDepartureLocation rdfs:subPropertyOf ies:relationship . 
ies:ticketDepartureLocation rdfs:range ies:Port . 
ies:ticketDepartureLocation rdfs:domain ies:TravelTicket . 
ies:TicketUsedInCheckIn rdf:type rdfs:Class . 
ies:TicketUsedInCheckIn sparx:guid "{92470C59-DFA6-47f7-A525-50CDABC8F852}" . 
ies:TicketUsedInCheckIn rdfs:comment "An EventParticipant where a Ricket is used in a CheckIn evente.g. a London Underground ticket being used at a barrier, or a concert ticket being scanned on arrival at the venue" . 
ies:TicketUsedInCheckIn rdfs:subClassOf ies:EventParticipant . 
ies:TimeBoundedClass rdf:type rdfs:Class . 
ies:TimeBoundedClass sparx:guid "{E7A659A5-9059-4ea5-8FAB-8A29AFC47D9A}" . 
ies:TimeBoundedClass rdfs:comment "A ClassOfElement whose instances all begin and end within the bounds specified for the Class. In other words, a class that is defined by the temporal extent of its members. Note, if either the begin or end bound are missing, it is taken to be indeterminate. For example, if the begin bound is 1st Jan 2018, the class has instances that all started after that date, and their end is irrelevant. Example:Everything that began and ended in the year 1900 - this would include all activities that took place within that year (but did not extend beyond it), everything created and destroyed within that time, and everything that was born and died during the period. " . 
ies:TimeBoundedClass rdfs:subClassOf ies:ClassOfElement . 
ies:Title rdf:type rdfs:Class . 
ies:Title sparx:guid "{30F5944F-75C3-4f12-A315-4E94ABCA809E}" . 
ies:Title rdfs:comment "The title of the respective document." . 
ies:Title rdfs:subClassOf ies:Name . 
ies:TOID rdf:type rdfs:Class . 
ies:TOID sparx:guid "{79D9049D-E63F-4c94-B348-49506A75B9F8}" . 
ies:TOID rdfs:comment "TOIDs (TOpographic IDentifiers) are unique and persistent identifiers created and managed by Ordnance Survey Great Britain to identify topographic objects in OS datasets. Example: the TOID for the Tower of London is osgb1000006032892." . 
ies:TOID rdfs:subClassOf ies:GeoIdentity . 
ies:TradeAgreement rdf:type rdfs:Class . 
ies:TradeAgreement sparx:guid "{54A4E900-7E8E-49fd-91F4-23ADDDF2DA60}" . 
ies:TradeAgreement rdfs:comment "A PoliticalAgreement that sets tariffs and standards for trade between nations. " . 
ies:TradeAgreement rdfs:subClassOf ies:PoliticalAgreement . 
ies:TradedAsset rdf:type rdfs:Class . 
ies:TradedAsset sparx:guid "{57ADBC97-C089-4d1a-A334-A9C44EAEC38A}" . 
ies:TradedAsset rdfs:comment "An EventParticipant where an Asset is participant in a TradeEventThis could be a specific Asset (e.g. serial numbered item) being offered for sale (as opposed to a type of Asset) or an Asset being delivered, withdrawn from sale, etc." . 
ies:TradedAsset rdfs:subClassOf ies:EventParticipant . 
ies:tradedItemType rdf:type owl:ObjectProperty . 
ies:tradedItemType sparx:guid "{A92F03F0-CB9E-4667-B985-25377303416A}" . 
ies:tradedItemType rdfs:comment "The type of entity involved in the TradeEvente.g. Dyson Animal Mk3Note: there may be no more than one itemType for a given TradeEvent - i.e. a new TradeEvent must be instantiated for each ClassOfEntity sold, offered, delivered, etc.Note: was ItemType in IES 3.2" . 
ies:tradedItemType rdfs:subPropertyOf ies:relationship . 
ies:tradedItemType rdfs:domain ies:TradeEvent . 
ies:tradedItemType rdfs:range ies:ClassOfEntity . 
ies:TradeEvent rdf:type rdfs:Class . 
ies:TradeEvent sparx:guid "{CA86862B-DA7E-487c-907B-26FA5D0564CD}" . 
ies:TradeEvent rdfs:comment "An Event where something is offered, bought or exchanged" . 
ies:TradeEvent rdfs:subClassOf ies:Event . 
ies:TrainTicket rdf:type rdfs:Class . 
ies:TrainTicket sparx:guid "{A8715447-3583-45d0-9550-625CF96B3E2E}" . 
ies:TrainTicket rdfs:comment "A Ticket that is used to travel by rail" . 
ies:TrainTicket rdfs:subClassOf ies:TravelTicket . 
ies:TrainTravel rdf:type rdfs:Class . 
ies:TrainTravel sparx:guid "{F2D6CFE4-BCE9-4bce-ADB0-075656038A55}" . 
ies:TrainTravel rdfs:comment "A TravelService by rail" . 
ies:TrainTravel rdfs:subClassOf ies:Transit . 
ies:transferType rdf:type owl:ObjectProperty . 
ies:transferType sparx:guid "{9574377B-6752-4317-94DC-E075C408442D}" . 
ies:transferType rdfs:comment "An rdf:type relationship from a MoneyTransfer to a ClassOfMoneyTransfer" . 
ies:transferType rdfs:subPropertyOf ies:relationship . 
ies:transferType rdfs:domain ies:MoneyTransfer . 
ies:transferType rdfs:subPropertyOf rdf:type . 
ies:transferType rdfs:range ies:ClassOfMoneyTransfer . 
ies:transferValue rdf:type owl:ObjectProperty . 
ies:transferValue sparx:guid "{A9D01DAB-281E-48ae-BB33-8518701ABBDE}" . 
ies:transferValue rdfs:comment "A relationship from a MoneyTransfer to the AmountOfMoney transferred." . 
ies:transferValue rdfs:subPropertyOf ies:relationship . 
ies:transferValue rdfs:domain ies:MoneyTransfer . 
ies:transferValue rdfs:range ies:AmountOfMoney . 
ies:Transit rdf:type rdfs:Class . 
ies:Transit sparx:guid "{7693D2C9-0F06-4005-BB8D-B5B572B2281A}" . 
ies:Transit rdfs:comment "A Movement that is an individual transportation - e.g. an individual flight, sailing, etc." . 
ies:Transit rdfs:subClassOf ies:Movement . 
ies:TravelBooking rdf:type rdfs:Class . 
ies:TravelBooking sparx:guid "{76DC9A0C-F6E8-4ff4-ADD6-072DC1EBE3AB}" . 
ies:TravelBooking rdfs:comment "The Purchase of planned travel arrangements.3. Travel Bookings may include bookings for Flights, Ferry Crossings, Train Journeys (i.e Travel Services), and also Hotels, Hire Cars etc. when these have been modelled. These will be included on the booking as relationships to the appropriate other entities." . 
ies:TravelBooking rdfs:subClassOf ies:Purchase . 
ies:TravelCard rdf:type rdfs:Class . 
ies:TravelCard sparx:guid "{E1D8A09D-C260-4dd8-B6FF-C2FA8968A00B}" . 
ies:TravelCard rdfs:comment "A PaymentArtefact that permits travel on public transport" . 
ies:TravelCard rdfs:subClassOf ies:PaymentArtefact . 
ies:TravelLeg rdf:type rdfs:Class . 
ies:TravelLeg sparx:guid "{55384377-146A-47c9-8706-18A1343A219C}" . 
ies:TravelLeg rdfs:comment "An EventParticipant in which a Entity travels. That travel may be part of a Journey.The TravelLeg may be part of a Journey (i.e. the Journey has one of more legs)." . 
ies:TravelLeg rdfs:subClassOf ies:Moving . 
ies:TravelReservation rdf:type rdfs:Class . 
ies:TravelReservation sparx:guid "{8B290363-239E-415e-9F2D-8267D1BA2ECB}" . 
ies:TravelReservation rdfs:comment "A TradedAsset where the asset is a Reservation" . 
ies:TravelReservation rdfs:subClassOf ies:TradedAsset . 
ies:TravelService rdf:type rdfs:Class . 
ies:TravelService sparx:guid "{3D0FC30A-CF82-44f2-970E-BFD04EADBA74}" . 
ies:TravelService rdfs:comment "A transportation service, often provided as a public service � e.g. a scheduled flight, rail journey, ferry crossing, etc." . 
ies:TravelService rdfs:subClassOf ies:Event . 
ies:TravelServiceIdentifier rdf:type rdfs:Class . 
ies:TravelServiceIdentifier sparx:guid "{680FD822-C1F6-4d09-94D5-5D586C947DE1}" . 
ies:TravelServiceIdentifier rdfs:comment "The Identifier for the respective Travel Service � this is how humans would usually refer to the service Note however that often this identifier does not, on its own, uniquely identify any given instance of a travel service � e.g. Flight BA0010 is reused on a daily basis to refer to the flight between London Heathrow and Los Angeles. As such, to uniquely identify any given instance of a Travel Service you would need to combine it with other attributes � typically departure date/time.For Flights, this will be the Flight Number.For Ferry Sailings this is typically the name of the vessel that is scheduled to make that sailing and, when combined with the departure date/time can be used to uniquely identify that sailing. Note that if the actual vessel that makes the sailing is different to that which was scheduled (e.g. as result of the scheduled vessel being out of commission), this identifier is not modified." . 
ies:TravelServiceIdentifier rdfs:subClassOf ies:Identifier . 
ies:TravelTicket rdf:type rdfs:Class . 
ies:TravelTicket sparx:guid "{6C669BEF-9267-4612-9F29-B28918B203F5}" . 
ies:TravelTicket rdfs:comment "A Ticket that permits travel on a particular route or set of routes" . 
ies:TravelTicket rdfs:subClassOf ies:Ticket . 
ies:TravelVisa rdf:type rdfs:Class . 
ies:TravelVisa sparx:guid "{C066EEB4-91AF-4ee6-BB02-44A49087946B}" . 
ies:TravelVisa rdfs:comment "An IdentityDocument, usually attached to a Passport, which allows a Person to remain in a Country for a set period of time. " . 
ies:TravelVisa rdfs:subClassOf ies:IdentityDocument . 
ies:Treaty rdf:type rdfs:Class . 
ies:Treaty sparx:guid "{59599C4B-F3DE-49a0-B76F-BE4CB1293CBA}" . 
ies:Treaty rdfs:comment "An EndToEndAgreement that is between Nations and subject to international law" . 
ies:Treaty rdfs:subClassOf ies:PoliticalAgreement . 
ies:trusts rdf:type owl:ObjectProperty . 
ies:trusts sparx:guid "{37CEEA2E-93E7-446d-A181-A55A091C3B22}" . 
ies:trusts rdfs:comment "A Relationship between two ResponsibleActor Entities where one trusts the other.Note: this should not be considered a bi-directional relationship. Just because one person trusts another person does not necessarily mean the feeling is reciprocated. " . 
ies:trusts rdfs:subPropertyOf ies:relationship . 
ies:trusts rdfs:range ies:ResponsibleActor . 
ies:trusts rdfs:domain ies:ResponsibleActorState . 
ies:typeOfCriminality rdf:type owl:ObjectProperty . 
ies:typeOfCriminality sparx:guid "{07BDCB73-1CDA-4057-9D7E-EC088D304B04}" . 
ies:typeOfCriminality rdfs:comment "A link to the ClassOfCriminalActivity conducted" . 
ies:typeOfCriminality rdfs:subPropertyOf ies:relationship . 
ies:typeOfCriminality rdfs:subPropertyOf rdf:type . 
ies:typeOfCriminality rdfs:range ies:ClassOfCriminalActivity . 
ies:typeOfCriminality rdfs:domain ies:CriminalActivity . 
ies:typicallyTargets rdf:type owl:ObjectProperty . 
ies:typicallyTargets sparx:guid "{AE6D5097-F555-48af-AFBA-88ECAA31BFF3}" . 
ies:typicallyTargets rdfs:comment "A relationship linking a ClassOfOperationalEvent to a ClassOfCriminalActivity where the operations are intended to counter or target certain criminal activities.Example: counter-narcotics operations typically target drug dealing" . 
ies:typicallyTargets rdfs:subPropertyOf ies:relationship . 
ies:typicallyTargets rdfs:domain ies:ClassOfOperationalEvent . 
ies:typicallyTargets rdfs:range ies:ClassOfCriminalActivity . 
ies:UN_LOCODE rdf:type rdfs:Class . 
ies:UN_LOCODE sparx:guid "{AEA785BB-B625-41aa-8738-FB0F3726A281}" . 
ies:UN_LOCODE rdfs:comment "A GeoIdentity that is a United Nations Code for Trade and Transport Locations" . 
ies:UN_LOCODE rdfs:subClassOf ies:GeoIdentity . 
ies:UnitOfMeasure rdf:type rdfs:Class . 
ies:UnitOfMeasure sparx:guid "{9F2DE0F4-58B1-46b7-B25A-545D765381A8}" . 
ies:UnitOfMeasure rdfs:comment "A ClassOfMeasureValue that is used to quantify a Measure on a standard scale" . 
ies:UnitOfMeasure rdfs:subClassOf ies:ClassOfMeasureValue . 
ies:UpdateAccount rdf:type rdfs:Class . 
ies:UpdateAccount sparx:guid "{E2D19BE1-B1BF-4e0b-8D44-AFFD739756BA}" . 
ies:UpdateAccount rdfs:comment "An AccountAdminEvent where an Account is modified" . 
ies:UpdateAccount rdfs:subClassOf ies:AccountAdminEvent . 
ies:upperBound rdf:type owl:ObjectProperty . 
ies:upperBound sparx:guid "{D700FE64-4100-4ade-93CE-6219A7BC0BCB}" . 
ies:upperBound rdfs:comment "A relationship a MeasureRange to the Measure that is its upper bound" . 
ies:upperBound rdfs:subPropertyOf ies:relationship . 
ies:upperBound rdfs:domain ies:MeasureRange . 
ies:upperBound rdfs:range ies:Measure . 
ies:uriScheme rdf:type owl:DatatypeProperty . 
ies:uriScheme sparx:guid "{D97141BD-F6CF-4b10-B4E5-B1ECF6DF5178}" . 
ies:uriScheme rdfs:comment "URI scheme is the top level of the uniform resource identifier (URI) naming structure. All URIs and absolute URI references are formed with a scheme name, followed by a colon character (:), and the remainder of the URI called the scheme-specific part." . 
ies:uriScheme rdfs:subPropertyOf ies:attribute . 
ies:uriScheme rdfs:domain ies:WebResourceState . 
ies:uriSchemeName rdf:type owl:DatatypeProperty . 
ies:uriSchemeName sparx:guid "{AAA8DE3D-31D8-4c1e-B114-72E8B37D6CAA}" . 
ies:uriSchemeName rdfs:comment "URI scheme is the top level of the uniform resource identifier (URI) naming structure. All URIs and absolute URI references are formed with a scheme name, followed by a colon character (:), and the remainder of the URI called the scheme-specific part.A list of official IANA-registered URI schemes can be found at:http://en.wikipedia.org/wiki/URI_scheme#Official_IANAregistered_schemes" . 
ies:uriSchemeName rdfs:subPropertyOf ies:attribute . 
ies:uriSchemeName rdfs:domain ies:WebResourceState . 
ies:URL rdf:type rdfs:Class . 
ies:URL sparx:guid "{C23AB49C-0734-45b7-A383-8EEA305CDBE4}" . 
ies:URL rdfs:comment "An Identifier for a WebResource" . 
ies:URL rdfs:subClassOf ies:Identifier . 
ies:Username rdf:type rdfs:Class . 
ies:Username sparx:guid "{9D703CE2-DED0-4aba-BE21-474781670297}" . 
ies:Username rdfs:comment "The Identity for an account registered with an internet-based service.An email address can be used as an online identifier for a specific domain (like Facebook). Where this is the case it can be considered to be both an instance of an email address and an instance of a username for an online identity." . 
ies:Username rdfs:subClassOf ies:Identifier . 
ies:userOf rdf:type owl:ObjectProperty . 
ies:userOf sparx:guid "{01984617-C96D-48b3-ACDE-25F525719AEF}" . 
ies:userOf rdfs:comment "A hasAccessTo relationship between a ResponsibleActor and an Asset they use.Note: more often than not, this will be a statement of occasional use, so the instance of the ResponsibleActorState should also be an instance of DiscontinuousState. In rarer occasions, it may be used to highlight a single, continuous use, but generally this would be modelled with the appropriate type of Event and EventParticipants" . 
ies:userOf rdfs:range ies:Asset . 
ies:userOf rdfs:subPropertyOf ies:hasAccessTo . 
ies:usesServicesAt rdf:type owl:ObjectProperty . 
ies:usesServicesAt sparx:guid "{958E4D57-8A19-4855-B9B3-6BB2F93F77B7}" . 
ies:usesServicesAt rdfs:comment "A visits relationship between a ResponsibleActor and a Location where they use services - e.g. banking, shopping, etc..Note: more often than not, this will be a statement of regular/occasional use, so the instance of the ResponsibleActorState should also be an instance of DiscontinuousState. In rarer occasions, it may be used to highlight a single, continuous visit, but in that case, inLocation would generally be used." . 
ies:usesServicesAt rdfs:subPropertyOf ies:visits . 
ies:UsuallyParked rdf:type rdfs:Class . 
ies:UsuallyParked sparx:guid "{FCE0D994-4838-48fa-A274-57DB092A2960}" . 
ies:UsuallyParked rdfs:comment "A temporal state of a Vehicle which is the fusion of all its Parked statesExamples:* A car that is usually parked in Acacia Avenue* A ship that regularly docks at Dover* An aircraft that regularly resides in a private hangar" . 
ies:UsuallyParked rdfs:subClassOf ies:VehicleState . 
ies:UsuallyParked rdfs:subClassOf ies:DiscontinuousState . 
ies:vafNumber rdf:type owl:DatatypeProperty . 
ies:vafNumber sparx:guid "{6DEB5776-59E6-4645-9566-65EC62A36330}" . 
ies:vafNumber rdfs:comment "The Visa Application Form (VAF) number." . 
ies:vafNumber rdfs:subPropertyOf ies:attribute . 
ies:vafNumber rdfs:domain ies:TravelVisa . 
ies:validFromDate rdf:type owl:ObjectProperty . 
ies:validFromDate sparx:guid "{6ACC2ACC-46F2-4a02-A3E7-D16BE8EB723B}" . 
ies:validFromDate rdfs:comment "The date that the respective IdentityDocument or Ticket is valid from." . 
ies:validFromDate rdfs:subPropertyOf ies:relationship . 
ies:validFromDate rdfs:domain ies:IdentityDocument . 
ies:validFromDate rdfs:domain ies:PaymentArtefact . 
ies:validFromDate rdfs:domain ies:TravelTicket . 
ies:validFromDate rdfs:range ies:ParticularPeriod . 
ies:validToDate rdf:type owl:ObjectProperty . 
ies:validToDate sparx:guid "{680F737D-A8AB-4410-9F1D-FAD7BDC98447}" . 
ies:validToDate rdfs:comment "The date that the respective IdentityDocument or Ticket is valid to." . 
ies:validToDate rdfs:subPropertyOf ies:relationship . 
ies:validToDate rdfs:domain ies:IdentityDocument . 
ies:validToDate rdfs:domain ies:PaymentArtefact . 
ies:validToDate rdfs:domain ies:TravelTicket . 
ies:validToDate rdfs:range ies:ParticularPeriod . 
ies:ValueInAmperes rdf:type rdfs:Class . 
ies:ValueInAmperes sparx:guid "{0C682BA6-23AB-459c-B8FF-A114AA27650B}" . 
ies:ValueInAmperes rdfs:comment "A StandardMeasureValue for ElectricCurrent in amperes" . 
ies:ValueInAmperes rdfs:subClassOf ies:StandardMeasureValue . 
ies:ValueInCandela rdf:type rdfs:Class . 
ies:ValueInCandela sparx:guid "{391F91E4-768F-406c-A344-CC3331ABE2AC}" . 
ies:ValueInCandela rdfs:comment "A StandardMeasureValue for LuminousIntensity in candela" . 
ies:ValueInCandela rdfs:subClassOf ies:StandardMeasureValue . 
ies:ValueInKelvin rdf:type rdfs:Class . 
ies:ValueInKelvin sparx:guid "{32097C4D-A0FB-4024-BDB8-8E899DDCF217}" . 
ies:ValueInKelvin rdfs:comment "A StandardMeasureValue for Temperature in kelvin" . 
ies:ValueInKelvin rdfs:subClassOf ies:StandardMeasureValue . 
ies:ValueInKilograms rdf:type rdfs:Class . 
ies:ValueInKilograms sparx:guid "{E7A9BC2D-85E2-4999-90DC-B76C9CB57C42}" . 
ies:ValueInKilograms rdfs:comment "A StandardMeasureValue for Mass in kilograms" . 
ies:ValueInKilograms rdfs:subClassOf ies:StandardMeasureValue . 
ies:ValueInMetres rdf:type rdfs:Class . 
ies:ValueInMetres sparx:guid "{C8D4C3CB-16C2-44a7-B709-35CEBF219BF0}" . 
ies:ValueInMetres rdfs:comment "A StandardMeasureValue for Length in metres" . 
ies:ValueInMetres rdfs:subClassOf ies:StandardMeasureValue . 
ies:ValueInMoles rdf:type rdfs:Class . 
ies:ValueInMoles sparx:guid "{943CA047-F259-4181-BF04-F6D54065AAD4}" . 
ies:ValueInMoles rdfs:comment "A StandardMeasureValue for AmountOfSubstance in moles" . 
ies:ValueInMoles rdfs:subClassOf ies:StandardMeasureValue . 
ies:ValueInSeconds rdf:type rdfs:Class . 
ies:ValueInSeconds sparx:guid "{E485D394-B9D7-40b6-BD44-E5970B2118BD}" . 
ies:ValueInSeconds rdfs:comment "A StandardMeasureValue for Duration in seconds" . 
ies:ValueInSeconds rdfs:subClassOf ies:StandardMeasureValue . 
ies:Vehicle rdf:type rdfs:Class . 
ies:Vehicle sparx:guid "{3B916F09-F3F4-43e9-9C84-99009C685396}" . 
ies:Vehicle rdfs:comment "An Asset that is a means of transportation � e.g. car, aircraft, ship." . 
ies:Vehicle rdfs:subClassOf ies:Device . 
ies:Vehicle rdfs:subClassOf ies:VehicleState . 
ies:VehicleController rdf:type rdfs:Class . 
ies:VehicleController sparx:guid "{93A816A9-EB7B-4250-8A1A-8919488029A7}" . 
ies:VehicleController rdfs:comment "A PersonInTransit where the Person is in control of the Transite.g. driver of a car, pilot of plane, captain of a ship" . 
ies:VehicleController rdfs:subClassOf ies:PersonInTransit . 
ies:VehicleIdentificationNumber rdf:type rdfs:Class . 
ies:VehicleIdentificationNumber sparx:guid "{AC9AB7B0-6C38-4b08-B2B9-CAA8486F0F4B}" . 
ies:VehicleIdentificationNumber rdfs:comment "VIN � Vehicle Identification Number.For road vehicles this is often directly referred to as the VIN, but this can also be applied in a generic fashion to other vehicle types.ISO 3833 for road vehicles (17-digits)" . 
ies:VehicleIdentificationNumber rdfs:subClassOf ies:Identifier . 
ies:VehicleName rdf:type rdfs:Class . 
ies:VehicleName sparx:guid "{9D24B4BE-2AD4-42d6-A906-8F6EFDA23EC5}" . 
ies:VehicleName rdfs:comment "The Name of the respective Vehicle (if applicable) � often this only applies to ships/boats. Examples:The Saucy SueThe Bountiful Blumpkin" . 
ies:VehicleName rdfs:subClassOf ies:Identifier . 
ies:VehicleState rdf:type rdfs:Class . 
ies:VehicleState sparx:guid "{D3275233-7381-483e-B2D2-77F13D73A52E}" . 
ies:VehicleState rdfs:comment "A temporal state of a Vehicle" . 
ies:VehicleState rdfs:subClassOf ies:AssetState . 
ies:VehicleUsed rdf:type rdfs:Class . 
ies:VehicleUsed sparx:guid "{2202F5B0-DF49-4db5-A8F9-31FC2CC89005}" . 
ies:VehicleUsed rdfs:comment "An EventParticipant in which a Vehicle is used to transport Entities" . 
ies:VehicleUsed rdfs:subClassOf ies:EventParticipant . 
ies:venueStatedOnTicket rdf:type owl:ObjectProperty . 
ies:venueStatedOnTicket sparx:guid "{3345AECA-925E-4bfc-820E-2294D5921E71}" . 
ies:venueStatedOnTicket rdfs:comment "The venue of the event the Ticket is for.Note: venues change, and the actual event may not run at the stated venue. " . 
ies:venueStatedOnTicket rdfs:subPropertyOf ies:relationship . 
ies:venueStatedOnTicket rdfs:domain ies:EntertainmentTicket . 
ies:venueStatedOnTicket rdfs:range ies:Facility . 
ies:VersionNumber rdf:type rdfs:Class . 
ies:VersionNumber sparx:guid "{E4C44F5B-5D57-4283-B985-5A2DA87BF212}" . 
ies:VersionNumber rdfs:comment "The number or code that identifies a VersionOfDocument." . 
ies:VersionNumber rdfs:subClassOf ies:Identifier . 
ies:versionOf rdf:type owl:ObjectProperty . 
ies:versionOf sparx:guid "{C01F47A2-F545-4fac-A707-469AD32FBF94}" . 
ies:versionOf rdfs:comment "A relationship between a VersionOfDocument and the WorkOfDocumentation it is a version of." . 
ies:versionOf rdfs:subPropertyOf rdfs:subClassOf . 
ies:versionOf rdfs:subPropertyOf ies:relationship . 
ies:versionOf rdfs:range ies:WorkOfDocumentation . 
ies:versionOf rdfs:domain ies:VersionOfDocument . 
ies:VersionOfDocument rdf:type rdfs:Class . 
ies:VersionOfDocument sparx:guid "{ADB16761-4981-4476-BC53-2843587D1C02}" . 
ies:VersionOfDocument rdfs:comment "A WorkOfDocumentation and a TimeBoundedClass that is a versionOf a WorkOfDocumentation" . 
ies:VersionOfDocument rdfs:subClassOf ies:WorkOfDocumentation . 
ies:VersionOfDocument rdfs:subClassOf ies:TimeBoundedClass . 
ies:Victim rdf:type rdfs:Class . 
ies:Victim sparx:guid "{3B47FCD0-E7D1-4b2b-BC07-C96D3F07ABC3}" . 
ies:Victim rdfs:comment "An EventParticipant where a ResponsibleActor is the victim of a CriminalActivity" . 
ies:Victim rdfs:subClassOf ies:EventParticipant . 
ies:VideoConference rdf:type rdfs:Class . 
ies:VideoConference sparx:guid "{1ED09A3D-7EE9-4b7a-8F0B-8590023C9F81}" . 
ies:VideoConference rdfs:comment "A TeleConference where parties communicate over video (with audio)" . 
ies:VideoConference rdfs:subClassOf ies:TeleConference . 
ies:visaType rdf:type owl:ObjectProperty . 
ies:visaType sparx:guid "{2ED602C6-C93C-41f3-8A02-10F0CAD0D64A}" . 
ies:visaType rdfs:comment "The type of the TravelVisaExamples:B1/B2VISA TIER 4" . 
ies:visaType rdfs:subPropertyOf ies:relationship . 
ies:visaType rdfs:domain ies:TravelVisa . 
ies:visaType rdfs:subPropertyOf rdf:type . 
ies:visaType rdfs:range ies:ClassOfTravelVisa . 
ies:visits rdf:type owl:ObjectProperty . 
ies:visits sparx:guid "{92FC2C35-D40B-4393-BA0B-88849743FEB6}" . 
ies:visits rdfs:comment "A Relationship and in inLocation between a ResponsibleActor and a Location they visit.Note: more often than not, this will be a statement of occasional visiting, so the instance of the ResponsibleActorState should also be an instance of DiscontinuousState. In rarer occasions, it may be used to highlight a single, continuous visit, but in that case, inLocation would generally be used." . 
ies:visits rdfs:subPropertyOf ies:inLocation . 
ies:visits rdfs:range ies:Location . 
ies:visits rdfs:domain ies:ResponsibleActorState . 
ies:VoiceCall rdf:type rdfs:Class . 
ies:VoiceCall sparx:guid "{F186E39F-A251-4b84-85E9-577C7290F6D9}" . 
ies:VoiceCall rdfs:comment "An InteractiveCommunication by voice" . 
ies:VoiceCall rdfs:subClassOf ies:InteractiveCommunication . 
ies:VoipAccount rdf:type rdfs:Class . 
ies:VoipAccount sparx:guid "{2DB8231F-0673-4788-AE41-3F52A3702A2B}" . 
ies:VoipAccount rdfs:comment "A TelephoneAccount where the voice communication is over IP. This may also include video communication, screen sharing, etc. " . 
ies:VoipAccount rdfs:subClassOf ies:TelephoneAccount . 
ies:VoipAccount rdfs:subClassOf ies:OnlineAccount . 
ies:VotingAttendee rdf:type rdfs:Class . 
ies:VotingAttendee sparx:guid "{B94FF143-3681-41eb-8264-D3E85C558EFC}" . 
ies:VotingAttendee rdfs:comment "When a Government has voting rights at a Summit" . 
ies:VotingAttendee rdfs:subClassOf ies:EventParticipant . 
ies:War rdf:type rdfs:Class . 
ies:War sparx:guid "{D4F568F5-7BC4-489d-94BC-AE1305E5C0C2}" . 
ies:War rdfs:comment "A Disagreement where at least one party has declared war" . 
ies:War rdfs:subClassOf ies:Disagreement . 
ies:War rdfs:subClassOf ies:EndToEndActivity . 
ies:Warrant rdf:type rdfs:Class . 
ies:Warrant sparx:guid "{4CAD884A-1EA7-473d-9881-8B76EBF8526F}" . 
ies:Warrant rdfs:comment "An AuthorisationDocument that provides legal permission, usually for something that would be considered illegal or intrusive otherwise" . 
ies:Warrant rdfs:subClassOf ies:AuthorisationDocument . 
ies:Warrantry rdf:type rdfs:Class . 
ies:Warrantry sparx:guid "{CA2023C6-1677-4d24-A1E6-22BC4D595E6F}" . 
ies:Warrantry rdfs:comment "An EndToEndAuthorisation where the process involves legal warrants. " . 
ies:Warrantry rdfs:subClassOf ies:EndToEndAuthorisation . 
ies:wasAuthorisedBy rdf:type owl:ObjectProperty . 
ies:wasAuthorisedBy sparx:guid "{7A58C9AD-C198-4a61-8244-DE5BBC591416}" . 
ies:wasAuthorisedBy rdfs:comment "A relationship to the Organisation that was the authorising agency for the IdentityDocument" . 
ies:wasAuthorisedBy rdfs:subPropertyOf ies:relationship . 
ies:wasAuthorisedBy rdfs:domain ies:IdentityDocument . 
ies:wasAuthorisedBy rdfs:range ies:Organisation . 
ies:WeaponLocation rdf:type rdfs:Class . 
ies:WeaponLocation sparx:guid "{B513F0D8-E527-4548-8453-D905775E3A4F}" . 
ies:WeaponLocation rdfs:comment "Relates an MilitaryAttack to the location of the attacking weapon system" . 
ies:WeaponLocation rdfs:subClassOf ies:EventParticipant . 
ies:Webpage rdf:type rdfs:Class . 
ies:Webpage sparx:guid "{79098C74-E063-4c45-886D-D0B88A48E954}" . 
ies:Webpage rdfs:comment "An OnlineArtefact that is a page on the web." . 
ies:Webpage rdfs:subClassOf ies:OnlineArtefact . 
ies:WebResource rdf:type rdfs:Class . 
ies:WebResource sparx:guid "{46D508B4-F1CC-45d7-9E4B-BA8A3C88D82A}" . 
ies:WebResource rdfs:comment "Any http presence on the web" . 
ies:WebResource rdfs:subClassOf ies:Entity . 
ies:WebResource rdfs:subClassOf ies:WebResourceState . 
ies:WebResourceState rdf:type rdfs:Class . 
ies:WebResourceState sparx:guid "{3BE61CCF-DCD0-411d-9D43-5DEABF8381F2}" . 
ies:WebResourceState rdfs:comment "A temporal state of an WebResource" . 
ies:WebResourceState rdfs:subClassOf ies:State . 
ies:What3words rdf:type rdfs:Class . 
ies:What3words sparx:guid "{B2262900-BF01-4691-8DE1-46A726A6D1CB}" . 
ies:What3words rdfs:comment "A GeoIdentity that is a what3words Location specifier(see what3words.com)" . 
ies:What3words rdfs:subClassOf ies:GeoIdentity . 
ies:WinningCandidate rdf:type rdfs:Class . 
ies:WinningCandidate sparx:guid "{9FC35E2C-3D28-4f21-8FF7-3BAA51860958}" . 
ies:WinningCandidate rdfs:comment "The Person who won the Election" . 
ies:WinningCandidate rdfs:subClassOf ies:ElectoralCandidate . 
ies:WithdrawFromSale rdf:type rdfs:Class . 
ies:WithdrawFromSale sparx:guid "{9416F72A-9BF9-4c99-839C-76905F02B63B}" . 
ies:WithdrawFromSale rdfs:comment "A TradeEvent where a type of entity is withdrawn from sale" . 
ies:WithdrawFromSale rdfs:subClassOf ies:TradeEvent . 
ies:Witness rdf:type rdfs:Class . 
ies:Witness sparx:guid "{9C9ED058-4BB5-43d0-A311-FF7A532ED6D6}" . 
ies:Witness rdfs:comment "A Persons role as a witness in a trial" . 
ies:Witness rdfs:subClassOf ies:ActiveEventParticipant . 
ies:Witness rdfs:subClassOf ies:PersonState . 
ies:WorkOfDocumentation rdf:type rdfs:Class . 
ies:WorkOfDocumentation sparx:guid "{F0B48978-D4E4-45a4-8238-091A5B714D82}" . 
ies:WorkOfDocumentation rdfs:comment "A Representation that is the general case of a document - i.e. War and Peace as opposed to My copy of War and Peace" . 
ies:WorkOfDocumentation rdfs:subClassOf ies:ClassOfIndividualDocument . 
ies:worksAt rdf:type owl:ObjectProperty . 
ies:worksAt sparx:guid "{55161540-8869-4af9-B159-51857E0B0BDB}" . 
ies:worksAt rdfs:comment "A visits relationship between a ResponsibleActor and a Location they work in.Note: more often than not, this will be a statement of occasional presence, so the instance of the ResponsibleActorState should also be an instance of DiscontinuousState. In rarer occasions, it may be used to highlight a single, continuous presence, but in that case, inLocation would generally be used." . 
ies:worksAt rdfs:subPropertyOf ies:visits . 
ies:worksFor rdf:type owl:ObjectProperty . 
ies:worksFor sparx:guid "{181AAC84-26CE-4531-AC32-A73B8FD8B858}" . 
ies:worksFor rdfs:comment "A Relationship between a ResponsibleActor (range - employer) and a ResponsibleActorState (domain- employed) that indicates one works for the other.In the case where the work is occasional / ad-hoc (i.e. there isnt an ongoing work contract) then the instance of the ResponsibleActorState should also be an instance of DiscontinuousState" . 
ies:worksFor rdfs:subPropertyOf ies:relationship . 
ies:worksFor rdfs:domain ies:ResponsibleActorState . 
ies:worksFor rdfs:range ies:ResponsibleActor . 
ies:worksWith rdf:type owl:ObjectProperty . 
ies:worksWith sparx:guid "{25DD07E3-2500-4b9b-AF50-446EEC927AD2}" . 
ies:worksWith rdfs:comment "A Relationship between two ResponsibleActor Entities that indicates one works with the other.In the case where the work is occasional / ad-hoc (i.e. there isnt an ongoing job) then the instance of the ResponsibleActorState should also be an instance of DiscontinuousStateNote: this relationship should only be used when it is not known who the two people work for (in which case create an organisation and used employedBy) or when the working relationship is rather loose - e.g. in cases of criminal cooperation." . 
ies:worksWith rdfs:subPropertyOf ies:relationship . 
ies:worksWith rdfs:range ies:Person . 
ies:worksWith rdfs:domain ies:PersonState . 
ies:worshipsAt rdf:type owl:ObjectProperty . 
ies:worshipsAt sparx:guid "{475617C7-BEE3-4c5e-8749-9386B68A8DA5}" . 
ies:worshipsAt rdfs:comment "A visits relationship between a ResponsibleActor and a Location where they undertake religious worshipNote: more often than not, this will be a statement of regular/occasional worship, so the instance of the ResponsibleActorState should also be an instance of DiscontinuousState. In rarer occasions, it may be used to highlight a single, continuous visit, but in that case, inLocation would generally be used." . 
ies:worshipsAt rdfs:subPropertyOf ies:visits . 
ies:recognisesExistenceOf		rdf:type				owl:ObjectProperty .
ies:recognisesExistenceOf		rdfs:subPropertyOf		ies:Relationship .
ies:recognisesExistenceOf		rdfs:domain			ies:ResponsibleActorState .
ies:recognisesExistenceOf		rdfs:range			rdfs:Class .
ies:Vessel rdfs:subClassOf ies:Vehicle .
ies:Vessel rdf:type rdfs:Class .
ies:VesselState rdfs:subClassOf ies:VehicleState .
ies:VesselState rdf:type rdfs:Class .
ies:ObservedTarget rdfs:subClassOf ies:Observed .
ies:ObservedTarget rdf:type rdfs:Class .
ies:ObservedLocation rdfs:subClassOf ies:Observed .
ies:ObservedLocation rdf:type rdfs:Class .
ies:ClassOfLocation rdfs:subClassOf ies:ClassOfEntity .
ies:ClassOfLocation rdf:type rdfs:Class .
ies:ClassOfLocation ies:powertype ies:Entity .
ies:SetOfGeoMarginsOfError rdfs:subClassOf ies:ClassOfLocation .
ies:SetOfGeoMarginsOfError rdf:type rdfs:Class .
ies:LocationTransponder rdf:type rdfs:Class .
ies:LocationTransponder rdfs:subClassOf ies:CommunicationsDevice .
ies:LocationObservation rdf:type rdfs:Class .
ies:LocationObservation rdfs:subClassOf ies:Observation .
ies:ObservedLocation rdf:type rdfs:Class .
ies:ObservedLocation rdfs:subClassOf ies:Observed .
ies:ObservedTarget rdf:type rdfs:Class .
ies:ObservedTarget rdfs:subClassOf ies:Observed .